<?xml version="1.0"?>
<rdf:RDF xmlns="https://intforout.github.io/outdoorPressure"
     xml:base="https://intforout.github.io/outdoorPressure"
     xmlns:dc="http://purl.org/dc/elements/1.1/"
     xmlns:ns="http://creativecommons.org/ns#"
     xmlns:geo="http://www.opengis.net/ont/geosparql#"
     xmlns:guf="http://www.opengis.net/guf/1.0"
     xmlns:oor="http://purl.org/choucas.ign.fr/oor#"
     xmlns:org="http://www.w3.org/ns/org#"
     xmlns:owl="http://www.w3.org/2002/07/owl#"
     xmlns:pav="http://purl.org/pav/"
     xmlns:rdf="http://www.w3.org/1999/02/22-rdf-syntax-ns#"
     xmlns:www="http://purl.org/www.umr-lastig.fr/"
     xmlns:xml="http://www.w3.org/XML/1998/namespace"
     xmlns:xsd="http://www.w3.org/2001/XMLSchema#"
     xmlns:adms="http://www.w3.org/ns/adms#"
     xmlns:bibo="http://purl.org/ontology/bibo/"
     xmlns:core="http://purl.org/vocab/frbr/core#"
     xmlns:dcam="https://www.dublincore.org/specifications/dublin-core/dcmi-terms/"
     xmlns:dcat="http://www.w3.org/ns/dcat#"
     xmlns:foaf="http://xmlns.com/foaf/0.1/"
     xmlns:prov="http://www.w3.org/ns/prov#"
     xmlns:rdfs="http://www.w3.org/2000/01/rdf-schema#"
     xmlns:skos="http://www.w3.org/2004/02/skos/core#"
     xmlns:time="http://www.w3.org/2006/time#"
     xmlns:vann="http://purl.org/vocab/vann/"
     xmlns:dcam1="http://purl.org/dc/dcam/"
     xmlns:terms="http://purl.org/dc/terms/"
     xmlns:vocab="http://www.w3.org/1999/xhtml/vocab#"
     xmlns:schema="http://schema.org/"
     xmlns:geodata="http://purl.org/www.umr-lastig.fr/geodata#"
     xmlns:datacite="http://purl.org/spar/datacite/"
     xmlns:outdoorPressure="https://intforout.github.io/outdoorPressure#">
    <owl:Ontology rdf:about="https://intforout.github.io/outdoorPressure">
        <owl:imports rdf:resource="http://purl.org/www.umr-lastig.fr/geodata"/>
        <ns:licence rdf:resource="http://creativecommons.org/licenses/by/4.0/"/>
        <dc:creator>Bénédicte Bucher</dc:creator>
        <dc:creator>Marie-Dominique Van Damme</dc:creator>
        <dc:title xml:lang="en">Mountain outdoor pressure KG</dc:title>
        <rdfs:comment xml:lang="en">Sets of classes, properties and instances useful to study and mitigate ecological pressure generated by human outdoor activities in mountain</rdfs:comment>
        <rdfs:label xml:lang="en">Mountain outdoor pressure knowledge graph</rdfs:label>
    </owl:Ontology>
    


    <!-- 
    ///////////////////////////////////////////////////////////////////////////////////////
    //
    // Annotation properties
    //
    ///////////////////////////////////////////////////////////////////////////////////////
     -->

    


    <!-- http://creativecommons.org/ns#licence -->

    <owl:AnnotationProperty rdf:about="http://creativecommons.org/ns#licence"/>
    


    <!-- http://purl.org/dc/elements/1.1/creator -->

    <owl:AnnotationProperty rdf:about="http://purl.org/dc/elements/1.1/creator"/>
    


    <!-- http://purl.org/dc/elements/1.1/description -->

    <owl:AnnotationProperty rdf:about="http://purl.org/dc/elements/1.1/description"/>
    


    <!-- http://purl.org/dc/elements/1.1/publisher -->

    <owl:AnnotationProperty rdf:about="http://purl.org/dc/elements/1.1/publisher"/>
    


    <!-- http://purl.org/dc/elements/1.1/title -->

    <owl:AnnotationProperty rdf:about="http://purl.org/dc/elements/1.1/title"/>
    


    <!-- http://purl.org/dc/terms/bibliographicCitation -->

    <owl:AnnotationProperty rdf:about="http://purl.org/dc/terms/bibliographicCitation"/>
    


    <!-- http://purl.org/dc/terms/conformsTo -->

    <owl:AnnotationProperty rdf:about="http://purl.org/dc/terms/conformsTo"/>
    


    <!-- http://purl.org/dc/terms/creator -->

    <owl:AnnotationProperty rdf:about="http://purl.org/dc/terms/creator"/>
    


    <!-- http://purl.org/dc/terms/hasPart -->

    <owl:AnnotationProperty rdf:about="http://purl.org/dc/terms/hasPart"/>
    


    <!-- http://purl.org/dc/terms/identifier -->

    <owl:AnnotationProperty rdf:about="http://purl.org/dc/terms/identifier"/>
    


    <!-- http://purl.org/dc/terms/isPartOf -->

    <owl:AnnotationProperty rdf:about="http://purl.org/dc/terms/isPartOf"/>
    


    <!-- http://purl.org/dc/terms/issued -->

    <owl:AnnotationProperty rdf:about="http://purl.org/dc/terms/issued"/>
    


    <!-- http://purl.org/dc/terms/language -->

    <owl:AnnotationProperty rdf:about="http://purl.org/dc/terms/language"/>
    


    <!-- http://purl.org/dc/terms/license -->

    <owl:AnnotationProperty rdf:about="http://purl.org/dc/terms/license"/>
    


    <!-- http://purl.org/dc/terms/publisher -->

    <owl:AnnotationProperty rdf:about="http://purl.org/dc/terms/publisher"/>
    


    <!-- http://purl.org/dc/terms/spatial -->

    <owl:AnnotationProperty rdf:about="http://purl.org/dc/terms/spatial"/>
    


    <!-- http://purl.org/dc/terms/type -->

    <owl:AnnotationProperty rdf:about="http://purl.org/dc/terms/type"/>
    


    <!-- http://purl.org/spar/datacite/firstPage -->

    <owl:AnnotationProperty rdf:about="http://purl.org/spar/datacite/firstPage"/>
    


    <!-- http://purl.org/spar/datacite/lastPage -->

    <owl:AnnotationProperty rdf:about="http://purl.org/spar/datacite/lastPage"/>
    


    <!-- http://purl.org/spar/datacite/number -->

    <owl:AnnotationProperty rdf:about="http://purl.org/spar/datacite/number"/>
    


    <!-- http://purl.org/spar/datacite/publicationYear -->

    <owl:AnnotationProperty rdf:about="http://purl.org/spar/datacite/publicationYear"/>
    


    <!-- http://purl.org/spar/datacite/relatedIdentifier -->

    <owl:AnnotationProperty rdf:about="http://purl.org/spar/datacite/relatedIdentifier"/>
    


    <!-- http://purl.org/spar/datacite/resourceType -->

    <owl:AnnotationProperty rdf:about="http://purl.org/spar/datacite/resourceType"/>
    


    <!-- http://purl.org/spar/datacite/subject -->

    <owl:AnnotationProperty rdf:about="http://purl.org/spar/datacite/subject"/>
    


    <!-- http://purl.org/spar/datacite/volume -->

    <owl:AnnotationProperty rdf:about="http://purl.org/spar/datacite/volume"/>
    


    <!-- http://purl.org/www.umr-lastig.fr/geodata#target -->

    <owl:AnnotationProperty rdf:about="http://purl.org/www.umr-lastig.fr/geodata#target"/>
    


    <!-- http://schema.org/address -->

    <owl:AnnotationProperty rdf:about="http://schema.org/address"/>
    


    <!-- http://www.w3.org/1999/02/22-rdf-syntax-ns#comment -->

    <owl:AnnotationProperty rdf:about="http://www.w3.org/1999/02/22-rdf-syntax-ns#comment"/>
    


    <!-- http://www.w3.org/2000/01/rdf-schema#description -->

    <owl:AnnotationProperty rdf:about="http://www.w3.org/2000/01/rdf-schema#description"/>
    


    <!-- http://www.w3.org/ns/dcat#accessService -->

    <owl:AnnotationProperty rdf:about="http://www.w3.org/ns/dcat#accessService"/>
    


    <!-- http://www.w3.org/ns/dcat#accessURL -->

    <owl:AnnotationProperty rdf:about="http://www.w3.org/ns/dcat#accessURL"/>
    


    <!-- http://www.w3.org/ns/dcat#conformsTo -->

    <owl:AnnotationProperty rdf:about="http://www.w3.org/ns/dcat#conformsTo"/>
    


    <!-- http://www.w3.org/ns/dcat#dataset -->

    <owl:AnnotationProperty rdf:about="http://www.w3.org/ns/dcat#dataset"/>
    


    <!-- http://www.w3.org/ns/dcat#format -->

    <owl:AnnotationProperty rdf:about="http://www.w3.org/ns/dcat#format"/>
    


    <!-- http://www.w3.org/ns/dcat#hasPart -->

    <owl:AnnotationProperty rdf:about="http://www.w3.org/ns/dcat#hasPart"/>
    


    <!-- http://www.w3.org/ns/dcat#identifier -->

    <owl:AnnotationProperty rdf:about="http://www.w3.org/ns/dcat#identifier"/>
    


    <!-- http://www.w3.org/ns/dcat#isPartOf -->

    <owl:AnnotationProperty rdf:about="http://www.w3.org/ns/dcat#isPartOf"/>
    


    <!-- http://www.w3.org/ns/dcat#issued -->

    <owl:AnnotationProperty rdf:about="http://www.w3.org/ns/dcat#issued"/>
    


    <!-- http://www.w3.org/ns/dcat#keyword -->

    <owl:AnnotationProperty rdf:about="http://www.w3.org/ns/dcat#keyword"/>
    


    <!-- http://www.w3.org/ns/dcat#record -->

    <owl:AnnotationProperty rdf:about="http://www.w3.org/ns/dcat#record"/>
    


    <!-- http://www.w3.org/ns/dcat#servesDataset -->

    <owl:AnnotationProperty rdf:about="http://www.w3.org/ns/dcat#servesDataset"/>
    


    <!-- http://www.w3.org/ns/dcat#service -->

    <owl:AnnotationProperty rdf:about="http://www.w3.org/ns/dcat#service"/>
    


    <!-- http://www.w3.org/ns/dcat#theme -->

    <owl:AnnotationProperty rdf:about="http://www.w3.org/ns/dcat#theme"/>
    


    <!-- http://www.w3.org/ns/prov#endedAtTime -->

    <owl:AnnotationProperty rdf:about="http://www.w3.org/ns/prov#endedAtTime"/>
    


    <!-- http://www.w3.org/ns/prov#generated -->

    <owl:AnnotationProperty rdf:about="http://www.w3.org/ns/prov#generated"/>
    


    <!-- http://www.w3.org/ns/prov#quotedAs -->

    <owl:AnnotationProperty rdf:about="http://www.w3.org/ns/prov#quotedAs"/>
    


    <!-- http://www.w3.org/ns/prov#startedAtTime -->

    <owl:AnnotationProperty rdf:about="http://www.w3.org/ns/prov#startedAtTime"/>
    


    <!-- http://www.w3.org/ns/prov#used -->

    <owl:AnnotationProperty rdf:about="http://www.w3.org/ns/prov#used"/>
    


    <!-- http://www.w3.org/ns/prov#wasAssociatedWith -->

    <owl:AnnotationProperty rdf:about="http://www.w3.org/ns/prov#wasAssociatedWith"/>
    


    <!-- http://www.w3.org/ns/prov#wasAttributedTo -->

    <owl:AnnotationProperty rdf:about="http://www.w3.org/ns/prov#wasAttributedTo"/>
    


    <!-- http://www.w3.org/ns/prov#wasGeneratedBy -->

    <owl:AnnotationProperty rdf:about="http://www.w3.org/ns/prov#wasGeneratedBy"/>
    


    <!-- http://www.w3.org/ns/prov#wasInfluencedBy -->

    <owl:AnnotationProperty rdf:about="http://www.w3.org/ns/prov#wasInfluencedBy"/>
    


    <!-- http://www.w3.org/ns/prov#wasQuotedFrom -->

    <owl:AnnotationProperty rdf:about="http://www.w3.org/ns/prov#wasQuotedFrom"/>
    


    <!-- http://xmlns.com/foaf/0.1/homePage -->

    <owl:AnnotationProperty rdf:about="http://xmlns.com/foaf/0.1/homePage"/>
    


    <!-- http://xmlns.com/foaf/0.1/name -->

    <owl:AnnotationProperty rdf:about="http://xmlns.com/foaf/0.1/name"/>
    


    <!-- http://xmlns.com/foaf/0.1/primaryTopic -->

    <owl:AnnotationProperty rdf:about="http://xmlns.com/foaf/0.1/primaryTopic"/>
    


    <!-- 
    ///////////////////////////////////////////////////////////////////////////////////////
    //
    // Datatypes
    //
    ///////////////////////////////////////////////////////////////////////////////////////
     -->

    


    <!-- http://www.w3.org/2001/XMLSchema#date -->

    <rdfs:Datatype rdf:about="http://www.w3.org/2001/XMLSchema#date"/>
    


    <!-- http://www.w3.org/2001/XMLSchema#gYearMonth -->

    <rdfs:Datatype rdf:about="http://www.w3.org/2001/XMLSchema#gYearMonth"/>
    


    <!-- xsd:date -->

    <rdfs:Datatype rdf:about="xsd:date"/>
    


    <!-- 
    ///////////////////////////////////////////////////////////////////////////////////////
    //
    // Object Properties
    //
    ///////////////////////////////////////////////////////////////////////////////////////
     -->

    


    <!-- https://intforout.github.io/outdoorPressure#affords -->

    <owl:ObjectProperty rdf:about="https://intforout.github.io/outdoorPressure#affords">
        <rdfs:domain rdf:resource="https://intforout.github.io/outdoorPressure#LandEntity"/>
        <rdfs:range rdf:resource="https://intforout.github.io/outdoorPressure#Activity"/>
        <rdfs:comment xml:lang="en">Capacity of a place, or land, to support a given activity, effectively or potentially</rdfs:comment>
    </owl:ObjectProperty>
    


    <!-- https://intforout.github.io/outdoorPressure#hasProfile -->

    <owl:ObjectProperty rdf:about="https://intforout.github.io/outdoorPressure#hasProfile">
        <rdfs:domain rdf:resource="http://www.w3.org/ns/dcat#Dataset"/>
        <rdfs:range rdf:resource="http://purl.org/dc/terms/URI"/>
        <rdfs:comment xml:lang="en">Profilage de la source -ou du jeu- partagé sous forme d&apos;un document référencé par une URL</rdfs:comment>
    </owl:ObjectProperty>
    


    <!-- https://intforout.github.io/outdoorPressure#locatedIn -->

    <owl:ObjectProperty rdf:about="https://intforout.github.io/outdoorPressure#locatedIn">
        <rdfs:domain rdf:resource="https://intforout.github.io/outdoorPressure#Population"/>
        <rdfs:range rdf:resource="https://intforout.github.io/outdoorPressure#LandEntity"/>
    </owl:ObjectProperty>
    


    <!-- 
    ///////////////////////////////////////////////////////////////////////////////////////
    //
    // Classes
    //
    ///////////////////////////////////////////////////////////////////////////////////////
     -->

    


    <!-- http://purl.org/dc/terms/URI -->

    <owl:Class rdf:about="http://purl.org/dc/terms/URI"/>
    


    <!-- https://intforout.github.io/outdoorPressure#Activity -->

    <owl:Class rdf:about="https://intforout.github.io/outdoorPressure#Activity">
        <rdfs:comment xml:lang="en">Activity of a living creature, or of a group or of a population, different from prov:Activity in the sense that the purpose of the Activity is not to yield an output.</rdfs:comment>
        <rdfs:label xml:lang="en">Activity</rdfs:label>
    </owl:Class>
    


    <!-- https://intforout.github.io/outdoorPressure#AireCampingCar -->

    <owl:Class rdf:about="https://intforout.github.io/outdoorPressure#AireCampingCar">
        <rdfs:subClassOf rdf:resource="https://intforout.github.io/outdoorPressure#LandEntity"/>
    </owl:Class>
    


    <!-- https://intforout.github.io/outdoorPressure#AireDeDetente -->

    <owl:Class rdf:about="https://intforout.github.io/outdoorPressure#AireDeDetente">
        <rdfs:subClassOf rdf:resource="https://intforout.github.io/outdoorPressure#LandEntity"/>
    </owl:Class>
    


    <!-- https://intforout.github.io/outdoorPressure#AireProtegee -->

    <owl:Class rdf:about="https://intforout.github.io/outdoorPressure#AireProtegee">
        <rdfs:subClassOf rdf:resource="https://intforout.github.io/outdoorPressure#LandEntity"/>
        <rdfs:comment xml:lang="fr">Une aire protégée (AP) (de l&apos;anglais protected area, PA) est, selon la définition de l&apos;Union internationale pour la conservation de la nature (UICN), « un espace géographique clairement défini, reconnu, consacré et géré, par tout moyen efficace, juridique ou autre, afin d&apos;assurer à long terme la conservation de la nature, des services écosystémiques et des valeurs culturelles qui lui sont associés »</rdfs:comment>
        <rdfs:label xml:lang="fr">Aire protégée</rdfs:label>
    </owl:Class>
    


    <!-- https://intforout.github.io/outdoorPressure#AnimalActivity -->

    <owl:Class rdf:about="https://intforout.github.io/outdoorPressure#AnimalActivity">
        <rdfs:subClassOf rdf:resource="https://intforout.github.io/outdoorPressure#Activity"/>
    </owl:Class>
    


    <!-- https://intforout.github.io/outdoorPressure#AnimalTrack -->

    <owl:Class rdf:about="https://intforout.github.io/outdoorPressure#AnimalTrack">
        <rdfs:subClassOf rdf:resource="https://intforout.github.io/outdoorPressure#Track"/>
        <rdfs:comment xml:lang="en">An animal trace is a digital trace corresponding to the path left by an animal tracked using an interoperable connected device and following a defined data collection protocol.</rdfs:comment>
        <rdfs:comment xml:lang="fr">La trace animale est une trace numérique correspondant à la trace laissée par un animal suivi au moyen d un dispositif connecté interopérable et selon un protocole de collecte défini.</rdfs:comment>
    </owl:Class>
    


    <!-- https://intforout.github.io/outdoorPressure#Cycling -->

    <owl:Class rdf:about="https://intforout.github.io/outdoorPressure#Cycling">
        <rdfs:subClassOf rdf:resource="https://intforout.github.io/outdoorPressure#HumanActivity"/>
    </owl:Class>
    


    <!-- https://intforout.github.io/outdoorPressure#EncounteringZone -->

    <owl:Class rdf:about="https://intforout.github.io/outdoorPressure#EncounteringZone">
        <rdfs:subClassOf rdf:resource="https://intforout.github.io/outdoorPressure#LandEntity"/>
        <rdfs:comment xml:lang="en">Area where different activities of different creatures take place, which can potentially imply a conflict of land use rather than harmonious land sharing.</rdfs:comment>
        <rdfs:label xml:lang="en">Encountering zone</rdfs:label>
    </owl:Class>
    


    <!-- https://intforout.github.io/outdoorPressure#FastHiking -->

    <owl:Class rdf:about="https://intforout.github.io/outdoorPressure#FastHiking">
        <rdfs:subClassOf rdf:resource="https://intforout.github.io/outdoorPressure#Hiking"/>
        <rdfs:comment xml:lang="fr">Le Fast hiking est une randonnée rapide qui se pratique à allure soutenue en toute autonomie sur un parcours présentant du dénivelé et/ou des difficultés techniques.
	        Il s’agit d’une discipline plus sportive et plus dynamique que la randonnée classique.</rdfs:comment>
    </owl:Class>
    


    <!-- https://intforout.github.io/outdoorPressure#FilteredTrack -->

    <owl:Class rdf:about="https://intforout.github.io/outdoorPressure#FilteredTrack">
        <rdfs:subClassOf rdf:resource="https://intforout.github.io/outdoorPressure#Track"/>
        <rdfs:comment xml:lang="en">Filtered traces represent a set of unstructured traces assumed to follow the network and used for a specific case study. They result from a user-defined filtering process (spatial, temporal, activity type, etc.).</rdfs:comment>
        <rdfs:comment xml:lang="fr">Les traces filtrées représentent un ensemble de traces non structurées, présumées suivre le réseau et utilisées pour un cas d étude spécifique. Elles résultent d un processus de filtrage défini par l utilisateur (spatial, temporel, type d activité, etc.).</rdfs:comment>
    </owl:Class>
    


    <!-- https://intforout.github.io/outdoorPressure#Hiking -->

    <owl:Class rdf:about="https://intforout.github.io/outdoorPressure#Hiking">
        <rdfs:subClassOf rdf:resource="https://intforout.github.io/outdoorPressure#HumanActivity"/>
        <rdfs:comment xml:lang="fr">activité de plein air consistant à se promener de façon ludique ou sportive</rdfs:comment>
        <rdfs:label xml:lang="en">Hiking</rdfs:label>
        <rdfs:label xml:lang="fr">Randonnée pédestre</rdfs:label>
    </owl:Class>
    


    <!-- https://intforout.github.io/outdoorPressure#HumanActivity -->

    <owl:Class rdf:about="https://intforout.github.io/outdoorPressure#HumanActivity">
        <rdfs:subClassOf rdf:resource="https://intforout.github.io/outdoorPressure#Activity"/>
        <rdfs:comment xml:lang="en">Human activity taking place outdoor</rdfs:comment>
    </owl:Class>
    


    <!-- https://intforout.github.io/outdoorPressure#HumanTrack -->

    <owl:Class rdf:about="https://intforout.github.io/outdoorPressure#HumanTrack">
        <rdfs:subClassOf rdf:resource="https://intforout.github.io/outdoorPressure#Track"/>
        <rdfs:comment xml:lang="en">A human trace is a digital trace corresponding to the path left by a person during outdoor activities using interoperable connected devices (GPS watches, apps, smartphones).</rdfs:comment>
        <rdfs:comment xml:lang="fr">La trace humaine est une trace numérique correspondant à la trace laissée par un humain lors d une activité de plein air, à l aide de dispositifs connectés interopérables (montres GPS, applications, smartphones).</rdfs:comment>
    </owl:Class>
    


    <!-- https://intforout.github.io/outdoorPressure#LandEntity -->

    <owl:Class rdf:about="https://intforout.github.io/outdoorPressure#LandEntity">
        <rdfs:comment xml:lang="en">An entity located in land : an area, a land, a parcel, a footprint, an observation.</rdfs:comment>
    </owl:Class>
    


    <!-- https://intforout.github.io/outdoorPressure#Landmark -->

    <owl:Class rdf:about="https://intforout.github.io/outdoorPressure#Landmark">
        <rdfs:subClassOf rdf:resource="https://intforout.github.io/outdoorPressure#LandEntity"/>
    </owl:Class>
    


    <!-- https://intforout.github.io/outdoorPressure#LivingCreature -->

    <owl:Class rdf:about="https://intforout.github.io/outdoorPressure#LivingCreature">
        <rdfs:comment>Living creature, animal or human</rdfs:comment>
    </owl:Class>
    


    <!-- https://intforout.github.io/outdoorPressure#MergedAccurateTrack -->

    <owl:Class rdf:about="https://intforout.github.io/outdoorPressure#MergedAccurateTrack">
        <rdfs:subClassOf rdf:resource="https://intforout.github.io/outdoorPressure#MergedTrack"/>
        <rdfs:comment xml:lang="en">An accurate merged trace is a merged trace that optimizes a quality criterion Q with respect to the ground truth GT (Van Damme et al., 2024).</rdfs:comment>
        <rdfs:comment xml:lang="fr">La trace fusionnée exacte est une trace fusionnée qui optimise un critère de qualité Q par rapport à la vérité terrain VT (Van Damme et al., 2024).</rdfs:comment>
    </owl:Class>
    


    <!-- https://intforout.github.io/outdoorPressure#MergedTrack -->

    <owl:Class rdf:about="https://intforout.github.io/outdoorPressure#MergedTrack">
        <rdfs:subClassOf rdf:resource="https://intforout.github.io/outdoorPressure#Track"/>
    </owl:Class>
    


    <!-- https://intforout.github.io/outdoorPressure#NamedRoute -->

    <owl:Class rdf:about="https://intforout.github.io/outdoorPressure#NamedRoute">
        <rdfs:subClassOf rdf:resource="https://intforout.github.io/outdoorPressure#Route"/>
        <rdfs:comment xml:lang="en">A named route is a known route with a name and a detailed linear geometry, listed in an authoritative or collaborative database (e.g., Visorando). 
	            Example: “Le chemin du Roy”.</rdfs:comment>
        <rdfs:comment xml:lang="fr">Un itinéraire nommé est un itinéraire connu ayant un titre et une géométrie linéraire détaillée,  répertorié dans une base de données d autorité ou collaborative (par ex. Visorando). 
	            Exemple : « Le chemin du Roy ».</rdfs:comment>
    </owl:Class>
    


    <!-- https://intforout.github.io/outdoorPressure#Observation -->

    <owl:Class rdf:about="https://intforout.github.io/outdoorPressure#Observation">
        <rdfs:subClassOf rdf:resource="https://intforout.github.io/outdoorPressure#Activity"/>
        <rdfs:comment>An observation is an act associated with a discrete time instant or period through which a number, term or other symbol is assigned to a phenomenon.</rdfs:comment>
        <rdfs:label>Observation or SurveyProcess</rdfs:label>
    </owl:Class>
    


    <!-- https://intforout.github.io/outdoorPressure#PlandEau -->

    <owl:Class rdf:about="https://intforout.github.io/outdoorPressure#PlandEau">
        <rdfs:subClassOf rdf:resource="https://intforout.github.io/outdoorPressure#LandEntity"/>
    </owl:Class>
    


    <!-- https://intforout.github.io/outdoorPressure#Population -->

    <owl:Class rdf:about="https://intforout.github.io/outdoorPressure#Population">
        <rdfs:comment xml:lang="en">Ensemble of individuals of a species in an land entity.</rdfs:comment>
        <rdfs:seeAlso>http://www.wikidata.org/entity/Q2625603</rdfs:seeAlso>
    </owl:Class>
    


    <!-- https://intforout.github.io/outdoorPressure#PopulationFootprint -->

    <owl:Class rdf:about="https://intforout.github.io/outdoorPressure#PopulationFootprint">
        <rdfs:subClassOf rdf:resource="https://intforout.github.io/outdoorPressure#LandEntity"/>
    </owl:Class>
    


    <!-- https://intforout.github.io/outdoorPressure#ReservesNaturelles -->

    <owl:Class rdf:about="https://intforout.github.io/outdoorPressure#ReservesNaturelles">
        <rdfs:subClassOf rdf:resource="https://intforout.github.io/outdoorPressure#LandEntity"/>
        <rdfs:comment>Zone naturelle sensible où l&apos;environnement est vulnérable à certaines activités humaines. Créé en 2018 et imaginé par la Ligue de Protection des Oiseaux Isère, introduit dans les api des services des parcs régionaux et nationaux. Ce concept permet d&apos;introduire les zones réglementaires et les zones sensibles, de renseigner les zones d’arrêtés de protection du biotope : emplacement, période de régulation, description associée, espèce, typologie de pratique, etc..</rdfs:comment>
        <rdfs:label>Réserves naturelles</rdfs:label>
    </owl:Class>
    


    <!-- https://intforout.github.io/outdoorPressure#ResilientRoute -->

    <owl:Class rdf:about="https://intforout.github.io/outdoorPressure#ResilientRoute">
        <rdfs:subClassOf rdf:resource="https://intforout.github.io/outdoorPressure#Route"/>
        <rdfs:comment xml:lang="en">A resilient itinerary is a route that minimizes its environmental impact, exerting no pressure on wildlife or vegetation.</rdfs:comment>
        <rdfs:comment xml:lang="fr">Un itinéraire résilient est un itinéraire qui n exerce pas de pression sur la faune et la flore.</rdfs:comment>
    </owl:Class>
    


    <!-- https://intforout.github.io/outdoorPressure#Route -->

    <owl:Class rdf:about="https://intforout.github.io/outdoorPressure#Route">
        <rdfs:subClassOf rdf:resource="https://intforout.github.io/outdoorPressure#LandEntity"/>
        <rdfs:comment xml:lang="en">A route represents a path to follow, which may rely (or not) on a physical support such as a road network (Teulade-Denantes et al., 2015). It is characterized by an origin, a destination, a set of waypoints, and a descriptive element.</rdfs:comment>
        <rdfs:comment xml:lang="fr">Un itinéraire représente un trajet à suivre qui s appuie (ou non) sur un support physique défini par un réseau routier (Teulade-Denantes et al., 2015). Il est caractérisé par une origine, une destination, un ensemble de points de passage et une description.</rdfs:comment>
    </owl:Class>
    


    <!-- https://intforout.github.io/outdoorPressure#SensitiveArea -->

    <owl:Class rdf:about="https://intforout.github.io/outdoorPressure#SensitiveArea">
        <rdfs:subClassOf rdf:resource="https://intforout.github.io/outdoorPressure#LandEntity"/>
        <rdfs:comment>Zone naturelle sensible où l&apos;environnement est vulnérable à certaines activités humaines. Créé en 2018 et imaginé par la Ligue de Protection des Oiseaux Isère, introduit dans les api des services des parcs régionaux et nationaux. Ce concept permet d&apos;introduire les zones réglementaires et les zones sensibles, de renseigner les zones d’arrêtés de protection du biotope : emplacement, période de régulation, description associée, espèce, typologie de pratique, etc..</rdfs:comment>
    </owl:Class>
    


    <!-- https://intforout.github.io/outdoorPressure#Sentier -->

    <owl:Class rdf:about="https://intforout.github.io/outdoorPressure#Sentier">
        <rdfs:subClassOf rdf:resource="https://intforout.github.io/outdoorPressure#LandEntity"/>
    </owl:Class>
    


    <!-- https://intforout.github.io/outdoorPressure#Track -->

    <owl:Class rdf:about="https://intforout.github.io/outdoorPressure#Track">
        <rdfs:comment xml:lang="en">A track is defined as an ordered set of points, each characterized by a position (x, y) and a timestamp (Van Damme et al., 2024).</rdfs:comment>
        <rdfs:comment xml:lang="fr">La trace est définie par un ensemble de points ordonnés, chaque point étant caractérisé par une position (x, y) et un temps (timestamp) (Van Damme et al., 2024). C&apos;est un résultat d&apos;une procédure : soit d&apos;une Observation par un Sensor, capteur gps porté par un objet mobile (Platform), soit d&apos;un retraitement d&apos;une trace brute, soit d&apos;une simulation.</rdfs:comment>
    </owl:Class>
    


    <!-- https://intforout.github.io/outdoorPressure#Trajectory -->

    <owl:Class rdf:about="https://intforout.github.io/outdoorPressure#Trajectory">
        <rdfs:subClassOf rdf:resource="https://intforout.github.io/outdoorPressure#LandEntity"/>
    </owl:Class>
    


    <!-- 
    ///////////////////////////////////////////////////////////////////////////////////////
    //
    // Individuals
    //
    ///////////////////////////////////////////////////////////////////////////////////////
     -->

    


    <!-- http://purl.org/www.umr-lastig.fr/geodata#BD_TOPO_V3 -->

    <owl:NamedIndividual rdf:about="http://purl.org/www.umr-lastig.fr/geodata#BD_TOPO_V3">
        <rdf:type rdf:resource="http://www.w3.org/ns/dcat#DatasetSeries"/>
        <schema:alternateName>BD TOPO® description vectorielle 3D (</schema:alternateName>
        <schema:creator rdf:resource="http://njh.me/contact.geoservices@ign.fr"/>
        <schema:dateCreated rdf:datatype="http://schema.org/Date">2002-12-15</schema:dateCreated>
        <schema:datePublished rdf:datatype="http://schema.org/Date">2025-06-15</schema:datePublished>
        <schema:description>La BD TOPO® version 3.5 contient une description vectorielle 3D (structurée en objets) des éléments du territoire et de ses infrastructures, de précision métrique.

	    Les objets de la BD TOPO® sont structurés en thèmes : 
	     - l&apos;administratif ; 
	     - le bâti ; 
	     - l&apos;hydrographie ; 
	     - les lieux nommés ; 
	     - l&apos;occupation du sol ; 
	     - les services et activités ; 
	     - le transport ; 
	     - les zones réglementées. 

	    Le processus de production 3D permet de fournir l&apos;altimétrie des objets, ainsi que la hauteur des bâtiments. 

	    Le relief est décrit sous forme de modèles numériques de terrain (MNT). 

	    Depuis la version 3.0, tous les objets possèdent un identifiant unique et stable dans le temps.

	    Le produit **BDTOPO® Express** est l’édition hebdomadaire de la BDTOPO® si vous avez besoin de travailler sur de la donnée topographique à haute fréquence (disponible depuis mai 2025). 

	    Le produit **Différentiel BD TOPO®** contient les différences géométriques et sémantiques sur l&apos;ensemble du contenu BD TOPO® entre deux éditions trimestrielles successives BD TOPO®. 

	    Plus précisément, l&apos;édition N du Différentiel BD TOPO® en vigueur contient tout objet de la BD TOPO® dont la date de modification, la date de création ou la date de suppression en base est postérieure à la date de prédiffusion de la précédente édition trimestrielle (N-1), équivalent à une activité de mise à jour par l&apos;IGN d&apos;une durée de 3 mois.</schema:description>
        <schema:encodingFormat>GPKG</schema:encodingFormat>
        <schema:encodingFormat>PostGreSQL</schema:encodingFormat>
        <schema:encodingFormat>SHP</schema:encodingFormat>
        <schema:encodingFormat>TMS</schema:encodingFormat>
        <schema:encodingFormat>WFS</schema:encodingFormat>
        <schema:encodingFormat>WMS</schema:encodingFormat>
        <schema:encodingFormat>WMTS</schema:encodingFormat>
        <schema:keywords>Altitude</schema:keywords>
        <schema:keywords>Bâtiments</schema:keywords>
        <schema:keywords>Dénominations géographiques</schema:keywords>
        <schema:keywords>Hydrographie</schema:keywords>
        <schema:keywords>Mobilité</schema:keywords>
        <schema:keywords>Réseaux de transport</schema:keywords>
        <schema:keywords>activités</schema:keywords>
        <schema:keywords>données ouvertes</schema:keywords>
        <schema:keywords>eau</schema:keywords>
        <schema:keywords>forêts</schema:keywords>
        <schema:keywords>haies</schema:keywords>
        <schema:keywords>routes</schema:keywords>
        <schema:keywords>toponymie</schema:keywords>
        <schema:keywords>transports</schema:keywords>
        <schema:keywords>végétation</schema:keywords>
        <schema:name>BD TOPO®</schema:name>
        <rdfs:comment xml:lang="en">BD TOPO covers whole French territory, is captured at scale 1/ 10 000, exists since 1990 and aims to provide reference data for mapping and spatial analysis.</rdfs:comment>
        <rdfs:label xml:lang="en">BD TOPO® V3.</rdfs:label>
        <dcat:language>fr-FR</dcat:language>
        <dcat:title xml:lang="fr">BD TOPO® V3. La BD TOPO® permet de couvrir de manière cohérente l&apos;ensemble des entités géographiques et administratives du territoire national. La BD TOPO® fournit une information de référence à tous les acteurs de la gestion, de l&apos;aménagement et de l&apos;observation du territoire pour analyser, situer, représenter des données dans leur réalité géographique</dcat:title>
    </owl:NamedIndividual>
    


    <!-- http://purl.org/www.umr-lastig.fr/geodata#CameraTrapSurveyCMB20242025 -->

    <owl:NamedIndividual rdf:about="http://purl.org/www.umr-lastig.fr/geodata#CameraTrapSurveyCMB20242025">
        <rdf:type rdf:resource="https://intforout.github.io/outdoorPressure#Observation"/>
        <rdfs:comment xml:lang="en">Including the locations of each eco-counter.</rdfs:comment>
        <rdfs:label xml:lang="en">Camera trap survey from Chamonix Community of Communes in 2024-2025.</rdfs:label>
        <prov:endedAtTime rdf:datatype="http://www.w3.org/2001/XMLSchema#gYearMonth">2024-02</prov:endedAtTime>
        <prov:generated rdf:resource="https://intforout.github.io/outdoorPressure#EcoCompteurCMBDataset"/>
        <prov:startedAtTime rdf:datatype="http://www.w3.org/2001/XMLSchema#gYearMonth">2025-11</prov:startedAtTime>
        <prov:used rdf:resource="ttp://purl.org/www.umr-lastig.fr/geodata#PyroEvo"/>
    </owl:NamedIndividual>
    


    <!-- http://purl.org/www.umr-lastig.fr/geodata#mgarel -->

    <owl:NamedIndividual rdf:about="http://purl.org/www.umr-lastig.fr/geodata#mgarel"/>
    


    <!-- http://purl.org/www.umr-lastig.fr/geodata#pmarchand -->

    <owl:NamedIndividual rdf:about="http://purl.org/www.umr-lastig.fr/geodata#pmarchand"/>
    


    <!-- https://api.camptocamp.org/ -->

    <owl:NamedIndividual rdf:about="https://api.camptocamp.org/"/>
    


    <!-- https://entrepot.recherche.data.gouv.fr/file.xhtml?persistentId=doi:10.57745/NSMUWN&amp;version=1.0 -->

    <owl:NamedIndividual rdf:about="https://entrepot.recherche.data.gouv.fr/file.xhtml?persistentId=doi:10.57745/NSMUWN&amp;version=1.0"/>
    


    <!-- https://entrepot.recherche.data.gouv.fr/file.xhtml?persistentId=doi:10.57745/P0PXVN&amp;version=1.0 -->

    <owl:NamedIndividual rdf:about="https://entrepot.recherche.data.gouv.fr/file.xhtml?persistentId=doi:10.57745/P0PXVN&amp;version=1.0"/>
    


    <!-- https://entrepot.recherche.data.gouv.fr/file.xhtml?persistentId=doi:10.57745/Q6OT0J&amp;version=1.0 -->

    <owl:NamedIndividual rdf:about="https://entrepot.recherche.data.gouv.fr/file.xhtml?persistentId=doi:10.57745/Q6OT0J&amp;version=1.0"/>
    


    <!-- https://entrepot.recherche.data.gouv.fr/file.xhtml?persistentId=doi:10.57745/TRYLX1&amp;version=1.0 -->

    <owl:NamedIndividual rdf:about="https://entrepot.recherche.data.gouv.fr/file.xhtml?persistentId=doi:10.57745/TRYLX1&amp;version=1.0"/>
    


    <!-- https://geotrek.parcdesbauges.com/api/v2/ -->

    <owl:NamedIndividual rdf:about="https://geotrek.parcdesbauges.com/api/v2/"/>
    


    <!-- https://intforout.github.io/outdoorPressure#AltitudeRandoRoutesBauges2025 -->

    <owl:NamedIndividual rdf:about="https://intforout.github.io/outdoorPressure#AltitudeRandoRoutesBauges2025">
        <rdf:type rdf:resource="http://www.w3.org/ns/dcat#Dataset"/>
        <terms:issued rdf:datatype="http://www.w3.org/2001/XMLSchema#date">2025-05-01</terms:issued>
        <terms:language>fr-FR</terms:language>
        <terms:license rdf:resource="https://opendatacommons.org/licenses/odbl/"/>
        <terms:publisher rdf:resource="https://intforout.github.io/outdoorPressure#altituderando"/>
        <rdfs:comment xml:lang="en">A set of routes issued from altituderando.com in 2025 in the Bauges area.</rdfs:comment>
        <rdfs:label xml:lang="en">AltitudeRando Hiking Routes in the Bauges Massif (2025)</rdfs:label>
    </owl:NamedIndividual>
    


    <!-- https://intforout.github.io/outdoorPressure#BDTOPOSentiersBauges2025 -->

    <owl:NamedIndividual rdf:about="https://intforout.github.io/outdoorPressure#BDTOPOSentiersBauges2025">
        <rdf:type rdf:resource="http://www.w3.org/ns/dcat#Dataset"/>
        <geodata:represents rdf:resource="https://intforout.github.io/outdoorPressure#SentierDesBauges"/>
        <rdfs:comment xml:lang="fr">Classe=Tronçon de route, Nature=Sentier</rdfs:comment>
        <rdfs:comment xml:lang="en">This dataset is extracted from the BDTOPO database, under the Transportation theme, from the Road Segment feature class, applying a filter on the “nature” attribute corresponding to the value “trail”.</rdfs:comment>
        <rdfs:label xml:lang="en">Trails from the BDTOPO dataset in the Bauges Massif (2025 edition)</rdfs:label>
        <dcat:inSeries rdf:resource="http://purl.org/www.umr-lastig.fr/geodata#BD_TOPO_V3"/>
    </owl:NamedIndividual>
    


    <!-- https://intforout.github.io/outdoorPressure#BoisVincennes -->

    <owl:NamedIndividual rdf:about="https://intforout.github.io/outdoorPressure#BoisVincennes">
        <rdf:type rdf:resource="http://purl.org/dc/terms/Location"/>
        <rdfs:label xml:lang="en">Test area located in the Bois de Vincennes</rdfs:label>
        <rdfs:label xml:lang="fr">Zone de test dans le Bois de Vincennes</rdfs:label>
    </owl:NamedIndividual>
    


    <!-- https://intforout.github.io/outdoorPressure#CamptocampPoisBauges2025 -->

    <owl:NamedIndividual rdf:about="https://intforout.github.io/outdoorPressure#CamptocampPoisBauges2025">
        <rdf:type rdf:resource="http://www.w3.org/ns/dcat#Dataset"/>
        <terms:issued rdf:datatype="http://www.w3.org/2001/XMLSchema#date">2025-05-01</terms:issued>
        <terms:language>fr-FR</terms:language>
        <terms:license rdf:resource="https://opendatacommons.org/licenses/odbl/"/>
        <terms:publisher rdf:resource="https://intforout.github.io/outdoorPressure#camptocamp"/>
        <rdfs:comment xml:lang="en">A set of Waypoints issued from Camptocamp.org API.</rdfs:comment>
        <rdfs:label xml:lang="en">Camptocamp.org-waypoints</rdfs:label>
        <dcat:distribution rdf:resource="https://intforout.github.io/outdoorPressure#c2c-waypoint-geojson"/>
    </owl:NamedIndividual>
    


    <!-- https://intforout.github.io/outdoorPressure#CamptocampRoutesBauges2025 -->

    <owl:NamedIndividual rdf:about="https://intforout.github.io/outdoorPressure#CamptocampRoutesBauges2025">
        <rdf:type rdf:resource="http://www.w3.org/ns/dcat#Dataset"/>
        <terms:issued rdf:datatype="http://www.w3.org/2001/XMLSchema#date">2025-05-01</terms:issued>
        <terms:language>fr-FR</terms:language>
        <terms:license rdf:resource="https://opendatacommons.org/licenses/odbl/"/>
        <terms:publisher rdf:resource="https://intforout.github.io/outdoorPressure#camptocamp"/>
        <rdfs:comment xml:lang="en">A set of Routes issued from Camptocamp.org API.</rdfs:comment>
        <rdfs:label xml:lang="en">Camptocamp.org-routes</rdfs:label>
        <dcat:distribution rdf:resource="https://intforout.github.io/outdoorPressure#c2c-route-geojson"/>
    </owl:NamedIndividual>
    


    <!-- https://intforout.github.io/outdoorPressure#DeepFaune -->

    <owl:NamedIndividual rdf:about="https://intforout.github.io/outdoorPressure#DeepFaune">
        <rdf:type rdf:resource="http://www.w3.org/ns/prov#SoftwareAgent"/>
        <terms:identifier>DeepFaune</terms:identifier>
        <rdfs:label xml:lang="en">DeepFaune</rdfs:label>
    </owl:NamedIndividual>
    


    <!-- https://intforout.github.io/outdoorPressure#EcoCompteurCMBDataset -->

    <owl:NamedIndividual rdf:about="https://intforout.github.io/outdoorPressure#EcoCompteurCMBDataset">
        <rdf:type rdf:resource="http://www.w3.org/ns/dcat#Dataset"/>
        <rdfs:comment xml:lang="fr">12 éco-compteurs (issus de conventions avec CD et Communauté de Communes de la Vallée de Chamonix-Mont-Blanc (CCVCMB) avec les localisations de chaque éco-compteur. Ces éco-compteurs sont tous des Pyro-Evo</rdfs:comment>
        <rdfs:comment xml:lang="en">This dataset includes 12 eco-counters (implemented through agreements with the Departmental Council and the Chamonix-Mont-Blanc Valley Community of Communes (CCVCMB)), together with the geographic location of each device. All counters are Pyro-Evo units.</rdfs:comment>
        <rdfs:label xml:lang="en">Dataset derived from 12 CCVCMB eco-counters.</rdfs:label>
    </owl:NamedIndividual>
    


    <!-- https://intforout.github.io/outdoorPressure#EcoCompteurUTMBDataset -->

    <owl:NamedIndividual rdf:about="https://intforout.github.io/outdoorPressure#EcoCompteurUTMBDataset">
        <rdf:type rdf:resource="http://www.w3.org/ns/dcat#Dataset"/>
        <rdfs:comment xml:lang="fr">10 éco-compteurs UTMB (avec des propriétaires différents), utilisables uniquement par le GT représentativité du WP2 dans un premier temps. Sinon pas d&apos;autorisation. Certains de ces éco-compteurs sont uniquement piétons, d’autres distinguent piétons / cyclistes / voitures.</rdfs:comment>
        <rdfs:comment xml:lang="en">This dataset comprises 10 UTMB eco-counters (with different ownership). They are initially accessible solely to the WP2 Representativeness Working Group; no additional authorization is granted. Some counters record pedestrian traffic only, while others distinguish between pedestrians, cyclists, and motor vehicles.</rdfs:comment>
        <rdfs:label xml:lang="en">Dataset derived from 12 UTMB eco-counters.</rdfs:label>
    </owl:NamedIndividual>
    


    <!-- https://intforout.github.io/outdoorPressure#EntrepotRechercheIntForOut -->

    <owl:NamedIndividual rdf:about="https://intforout.github.io/outdoorPressure#EntrepotRechercheIntForOut">
        <rdf:type rdf:resource="http://www.w3.org/ns/dcat#Catalog"/>
        <rdfs:comment xml:lang="en">Dataverse dedicated to the IntForOut project. This catalog is integrated into the multidisciplinary Recherche Data Gouv data warehouse platform.</rdfs:comment>
        <rdfs:comment xml:lang="fr">Dataverse dédié au projet IntForOut. Ce catalogue est intégré dans la plateforme de l&apos;entrepôt pluridisciplinaire Recherche Data Gouv.</rdfs:comment>
        <rdfs:label xml:lang="en">Dataverse dedicated to the IntForOut project</rdfs:label>
        <dcat:dataset rdf:resource="https://intforout.github.io/outdoorPressure#MOUSLS"/>
        <dcat:dataset rdf:resource="https://intforout.github.io/outdoorPressure#MOUSLSGroundTruthDenseForestPath"/>
        <dcat:dataset rdf:resource="https://intforout.github.io/outdoorPressure#MOUSLSTracksMultiSensorsVincennesForest"/>
        <dcat:record rdf:resource="https://intforout.github.io/outdoorPressure#MetadataGroundTruthPathVincennesForest"/>
        <dcat:record rdf:resource="https://intforout.github.io/outdoorPressure#MetadataTracksMultiSensorsVincennesForest"/>
        <foaf:homePage>https://entrepot.recherche.data.gouv.fr/dataverse/intforout</foaf:homePage>
    </owl:NamedIndividual>
    


    <!-- https://intforout.github.io/outdoorPressure#GroundTruthDenseForestPath-csv -->

    <owl:NamedIndividual rdf:about="https://intforout.github.io/outdoorPressure#GroundTruthDenseForestPath-csv">
        <rdf:type rdf:resource="http://www.w3.org/ns/dcat#Distribution"/>
        <dcat:accessURL rdf:resource="https://entrepot.recherche.data.gouv.fr/file.xhtml?persistentId=doi:10.57745/P0PXVN&amp;version=1.0"/>
        <dcat:format>csv</dcat:format>
        <dcat:identifier>ground_truth_dense_forest_path.txt</dcat:identifier>
    </owl:NamedIndividual>
    


    <!-- https://intforout.github.io/outdoorPressure#HikersFootprintBoisVincennes -->

    <owl:NamedIndividual rdf:about="https://intforout.github.io/outdoorPressure#HikersFootprintBoisVincennes">
        <rdf:type rdf:resource="https://intforout.github.io/outdoorPressure#PopulationFootprint"/>
        <outdoorPressure:affords rdf:resource="https://intforout.github.io/outdoorPressure#HikingInBoisdeVincennes"/>
    </owl:NamedIndividual>
    


    <!-- https://intforout.github.io/outdoorPressure#HikingInBoisdeVincennes -->

    <owl:NamedIndividual rdf:about="https://intforout.github.io/outdoorPressure#HikingInBoisdeVincennes">
        <rdf:type rdf:resource="https://intforout.github.io/outdoorPressure#Hiking"/>
    </owl:NamedIndividual>
    


    <!-- https://intforout.github.io/outdoorPressure#HikingInLesBauges -->

    <owl:NamedIndividual rdf:about="https://intforout.github.io/outdoorPressure#HikingInLesBauges">
        <rdf:type rdf:resource="https://intforout.github.io/outdoorPressure#Hiking"/>
    </owl:NamedIndividual>
    


    <!-- https://intforout.github.io/outdoorPressure#HumanChamoisRealEncounters -->

    <owl:NamedIndividual rdf:about="https://intforout.github.io/outdoorPressure#HumanChamoisRealEncounters">
        <rdf:type rdf:resource="http://www.w3.org/ns/dcat#Dataset"/>
        <terms:issued rdf:datatype="http://www.w3.org/2001/XMLSchema#date">2025-04-25</terms:issued>
        <terms:language>English</terms:language>
        <terms:license>Licence Ouverte v2.0 (Etalab)</terms:license>
        <terms:publisher rdf:resource="http://purl.org/www.umr-lastig.fr/geodata#LASTIG"/>
        <rdfs:comment xml:lang="en">185 real encounters. The geometries are saved as WKT. Only included real encounters as they are likely enough to work with and potential encounters drastically increase amount of data, also they may need some explanation for why they have 2 different dates</rdfs:comment>
        <dcat:distribution rdf:resource="https://intforout.github.io/outdoorPressure#HumanChamoisRealEncounters-csv"/>
        <prov:wasAttributedTo rdf:resource="http://purl.org/www.umr-lastig.fr/geodata#jadawson"/>
    </owl:NamedIndividual>
    


    <!-- https://intforout.github.io/outdoorPressure#HumanChamoisRealEncounters-csv -->

    <owl:NamedIndividual rdf:about="https://intforout.github.io/outdoorPressure#HumanChamoisRealEncounters-csv">
        <rdf:type rdf:resource="http://www.w3.org/ns/dcat#Distribution"/>
        <dcat:format>csv</dcat:format>
        <dcat:identifier>human_chamois_real_encounters.csv</dcat:identifier>
    </owl:NamedIndividual>
    


    <!-- https://intforout.github.io/outdoorPressure#HumanOutdoorActivitiesBauges2014 -->

    <owl:NamedIndividual rdf:about="https://intforout.github.io/outdoorPressure#HumanOutdoorActivitiesBauges2014">
        <rdf:type rdf:resource="https://intforout.github.io/outdoorPressure#HumanActivity"/>
    </owl:NamedIndividual>
    


    <!-- https://intforout.github.io/outdoorPressure#HumanOutdoorActivitiesBauges2024 -->

    <owl:NamedIndividual rdf:about="https://intforout.github.io/outdoorPressure#HumanOutdoorActivitiesBauges2024">
        <rdf:type rdf:resource="https://intforout.github.io/outdoorPressure#HumanActivity"/>
    </owl:NamedIndividual>
    


    <!-- https://intforout.github.io/outdoorPressure#HumanOutdoorActivitiesBoisVincennes2022 -->

    <owl:NamedIndividual rdf:about="https://intforout.github.io/outdoorPressure#HumanOutdoorActivitiesBoisVincennes2022">
        <rdf:type rdf:resource="https://intforout.github.io/outdoorPressure#HumanActivity"/>
    </owl:NamedIndividual>
    


    <!-- https://intforout.github.io/outdoorPressure#HumanOutdoorActivitiesMontBlanc2024 -->

    <owl:NamedIndividual rdf:about="https://intforout.github.io/outdoorPressure#HumanOutdoorActivitiesMontBlanc2024">
        <rdf:type rdf:resource="https://intforout.github.io/outdoorPressure#HumanActivity"/>
    </owl:NamedIndividual>
    


    <!-- https://intforout.github.io/outdoorPressure#IntForOutDB -->

    <owl:NamedIndividual rdf:about="https://intforout.github.io/outdoorPressure#IntForOutDB">
        <rdf:type rdf:resource="http://purl.org/www.umr-lastig.fr/geodata#DataWarehouse"/>
        <terms:language>English</terms:language>
        <terms:publisher rdf:resource="http://purl.org/www.umr-lastig.fr/geodata#LIFAT"/>
        <rdfs:comment>Dataset associated with IntForOut ETL framework</rdfs:comment>
        <rdfs:label xml:lang="en">Dataset associated with IntForOut ETL framework</rdfs:label>
    </owl:NamedIndividual>
    


    <!-- https://intforout.github.io/outdoorPressure#JournalOfOutdoorRecreationAndTourismKerouantonEtAl2024 -->

    <owl:NamedIndividual rdf:about="https://intforout.github.io/outdoorPressure#JournalOfOutdoorRecreationAndTourismKerouantonEtAl2024">
        <rdf:type rdf:resource="http://purl.org/www.umr-lastig.fr/geodata#ScientificPaper"/>
        <terms:creator rdf:resource="http://purl.org/www.umr-lastig.fr/geodata#ljolivet"/>
        <terms:creator rdf:resource="https://intforout.github.io/outdoorPressure#aloison"/>
        <terms:creator>
            <rdf:Description>
                <rdf:type rdf:resource="http://www.w3.org/ns/prov#Person"/>
                <foaf:name>Colin Kerouanton</foaf:name>
            </rdf:Description>
        </terms:creator>
        <terms:creator>
            <rdf:Description>
                <rdf:type rdf:resource="http://www.w3.org/ns/prov#Person"/>
                <foaf:name>Clémence Perrin-Malterre</foaf:name>
            </rdf:Description>
        </terms:creator>
        <terms:publisher>Journal of Outdoor Recreation and Tourism</terms:publisher>
        <datacite:firstPage>100734</datacite:firstPage>
        <datacite:publicationYear>2024</datacite:publicationYear>
        <datacite:relatedIdentifier>10.1016/j.jort.2024.100734</datacite:relatedIdentifier>
        <datacite:relatedIdentifier>https://doi.org/10.1016/j.jort.2024.100734</datacite:relatedIdentifier>
        <datacite:resourceType rdf:resource="http://purl.org/spar/datacite/Journal"/>
        <datacite:subject>Outdoor recreation</datacite:subject>
        <datacite:subject>Pauses</datacite:subject>
        <datacite:subject>ST-DBSCAN</datacite:subject>
        <datacite:subject>Spatio-temporal pattern</datacite:subject>
        <datacite:subject>Time-geography</datacite:subject>
        <datacite:subject>global navigation satellite system</datacite:subject>
        <rdfs:label xml:lang="en">Eye-catching or breath-catching: Role and landscape attributes of pauses differs among hikers’ profile when rambling in a French mountainous area</rdfs:label>
        <prov:quotedAs rdf:resource="https://intforout.github.io/outdoorPressure#KerouantonSurvey20142015"/>
        <prov:quotedAs rdf:resource="https://intforout.github.io/outdoorPressure#KerouantonTrack20142015"/>
    </owl:NamedIndividual>
    


    <!-- https://intforout.github.io/outdoorPressure#JournalOfPeopleAndNatureMarchandEtAl2025 -->

    <owl:NamedIndividual rdf:about="https://intforout.github.io/outdoorPressure#JournalOfPeopleAndNatureMarchandEtAl2025">
        <rdf:type rdf:resource="http://purl.org/www.umr-lastig.fr/geodata#ScientificPaper"/>
        <terms:creator rdf:resource="https://intforout.github.io/outdoorPressure#mgarel"/>
        <terms:creator rdf:resource="https://intforout.github.io/outdoorPressure#pmarchand"/>
        <terms:creator>
            <rdf:Description>
                <rdf:type rdf:resource="http://www.w3.org/ns/prov#Person"/>
                <foaf:name>Nolwenn Risser</foaf:name>
            </rdf:Description>
        </terms:creator>
        <terms:creator>
            <rdf:Description>
                <rdf:type rdf:resource="http://www.w3.org/ns/prov#Person"/>
                <foaf:name>Elodie Petit</foaf:name>
            </rdf:Description>
        </terms:creator>
        <terms:isPartOf>Journal of People and Nature</terms:isPartOf>
        <datacite:firstPage>3002</datacite:firstPage>
        <datacite:lastPage>3016</datacite:lastPage>
        <datacite:number>11</datacite:number>
        <datacite:publicationYear>2025</datacite:publicationYear>
        <datacite:relatedIdentifier>10.1002/pan3.70151</datacite:relatedIdentifier>
        <datacite:relatedIdentifier>https://besjournals.onlinelibrary.wiley.com/doi/abs/10.1002/pan3.70151</datacite:relatedIdentifier>
        <datacite:resourceType rdf:resource="http://purl.org/spar/datacite/Journal"/>
        <datacite:subject>activity</datacite:subject>
        <datacite:subject>behaviour</datacite:subject>
        <datacite:subject>cycling races</datacite:subject>
        <datacite:subject>disturbance</datacite:subject>
        <datacite:subject>movements</datacite:subject>
        <datacite:subject>recreational ecology</datacite:subject>
        <datacite:subject>trail running</datacite:subject>
        <datacite:volume>7</datacite:volume>
        <rdfs:label xml:lang="en">Disturbance by massive sporting events in mountain areas: When and where matters for the protected Alpine ibex Capra ibex</rdfs:label>
        <prov:quotedAs rdf:resource="https://intforout.github.io/outdoorPressure#MarchandEtAl2025MSEPeopleNatureDataZenodo"/>
    </owl:NamedIndividual>
    


    <!-- https://intforout.github.io/outdoorPressure#KerouantonQuestionnaire20142015 -->

    <owl:NamedIndividual rdf:about="https://intforout.github.io/outdoorPressure#KerouantonQuestionnaire20142015">
        <rdf:type rdf:resource="http://www.w3.org/ns/dcat#Dataset"/>
        <rdfs:comment xml:lang="en">A set of answers issued from a questionnaire. Compleed with tracks</rdfs:comment>
        <rdfs:label xml:lang="en">Tracks issued from PhD of Colin Kerouanton</rdfs:label>
        <dcat:inSeries rdf:resource="https://intforout.github.io/outdoorPressure#KerouantonSurveyFieldCampaignTracksGNSS20142015"/>
        <prov:wasQuotedFrom rdf:resource="https://intforout.github.io/outdoorPressure#JournalOfOutdoorRecreationAndTourismKerouantonEtAl2024"/>
    </owl:NamedIndividual>
    


    <!-- https://intforout.github.io/outdoorPressure#KerouantonSurvey20142015 -->

    <owl:NamedIndividual rdf:about="https://intforout.github.io/outdoorPressure#KerouantonSurvey20142015">
        <rdf:type rdf:resource="https://intforout.github.io/outdoorPressure#Observation"/>
        <prov:endedAtTime rdf:datatype="http://www.w3.org/2001/XMLSchema#gYearMonth">2014-01</prov:endedAtTime>
        <prov:generated rdf:resource="https://intforout.github.io/outdoorPressure#KerouantonSurveyFieldCampaignTracksGNSS20142015"/>
        <prov:startedAtTime rdf:datatype="http://www.w3.org/2001/XMLSchema#gYearMonth">2015-12</prov:startedAtTime>
    </owl:NamedIndividual>
    


    <!-- https://intforout.github.io/outdoorPressure#KerouantonSurveyFieldCampaignTracksGNSS20142015 -->

    <owl:NamedIndividual rdf:about="https://intforout.github.io/outdoorPressure#KerouantonSurveyFieldCampaignTracksGNSS20142015">
        <rdf:type rdf:resource="http://www.w3.org/ns/dcat#DatasetSeries"/>
        <terms:issued rdf:datatype="http://www.w3.org/2001/XMLSchema#date">2015-08-31</terms:issued>
        <terms:language>French</terms:language>
        <terms:publisher>LECA et l’EDYTEM</terms:publisher>
        <terms:spatial rdf:resource="https://intforout.github.io/outdoorPressure#PNRDesBauges"/>
        <rdfs:comment xml:lang="fr">Questionnaires de campagnes de terrain ciblant la pratique de la randonnée dans le PNR du Massif des Bauges accompagnés de traces GNSS</rdfs:comment>
        <rdfs:label xml:lang="fr">Questionnaires de campagnes de terrain complétés par des traces GNSS</rdfs:label>
        <prov:wasQuotedFrom rdf:resource="https://intforout.github.io/outdoorPressure#JournalOfOutdoorRecreationAndTourismKerouantonEtAl2024"/>
    </owl:NamedIndividual>
    


    <!-- https://intforout.github.io/outdoorPressure#KerouantonTrack20142015 -->

    <owl:NamedIndividual rdf:about="https://intforout.github.io/outdoorPressure#KerouantonTrack20142015">
        <rdf:type rdf:resource="http://www.w3.org/ns/dcat#Dataset"/>
        <rdfs:comment xml:lang="en">A set of tracks. Compleed with questionnaires</rdfs:comment>
        <rdfs:label xml:lang="en">Tracks issued from PhD of Colin Kerouanton</rdfs:label>
        <dcat:inSeries rdf:resource="https://intforout.github.io/outdoorPressure#KerouantonSurveyFieldCampaignTracksGNSS20142015"/>
        <prov:wasQuotedFrom rdf:resource="https://intforout.github.io/outdoorPressure#JournalOfOutdoorRecreationAndTourismKerouantonEtAl2024"/>
    </owl:NamedIndividual>
    


    <!-- https://intforout.github.io/outdoorPressure#LIFAT -->

    <owl:NamedIndividual rdf:about="https://intforout.github.io/outdoorPressure#LIFAT">
        <rdf:type rdf:resource="http://www.w3.org/ns/prov#Organization"/>
        <foaf:name>Laboratoire d&apos;Informatique Fondamentale et Appliquée de Tours (LIFAT)</foaf:name>
    </owl:NamedIndividual>
    


    <!-- https://intforout.github.io/outdoorPressure#MOUSLS -->

    <owl:NamedIndividual rdf:about="https://intforout.github.io/outdoorPressure#MOUSLS">
        <rdf:type rdf:resource="http://www.w3.org/ns/dcat#DatasetSeries"/>
        <terms:bibliographicCitation>Raimond, Ana-Maria; Meneroux, Yann; Calloch, Paul; Labbé, Brice; Peseux, Lorine; Tertre, Franck; Clédat, Emmanuel, 2025, &quot;Multi-sensors and Ground Truth Tracks&quot;, https://doi.org/10.57745/MOUSLS, Recherche Data Gouv, V1</terms:bibliographicCitation>
        <terms:issued rdf:datatype="http://www.w3.org/2001/XMLSchema#date">2025-01-18</terms:issued>
        <terms:language>English</terms:language>
        <terms:license>Licence Ouverte v2.0 (Etalab)</terms:license>
        <terms:publisher rdf:resource="http://purl.org/www.umr-lastig.fr/geodata#LASTIG"/>
        <terms:spatial rdf:resource="https://intforout.github.io/outdoorPressure#BoisVincennes"/>
        <datacite:relatedIdentifier>https://doi.org/10.57745/MOUSLS</datacite:relatedIdentifier>
        <rdfs:comment xml:lang="en">The goal of this dataset is to provide in-situ ground truth data to validate an algorithm for fusing GNSS tracks. This is a dataset series composed by two linked datasets. The first was (file tracks_multi_sensors_vincennes_forest.gpkg) contains GNSS tracks and was collected by two researchers using a strict data collection protocol, following the same path at times precisely and at other times with slight deviations. The second (file ground_truth_dense_forest_path.txt) was collected by a group of students and represents ground truth data for the same path in dense forest. English (2025)</rdfs:comment>
        <rdfs:label xml:lang="en">MOUSLS: Multi-sensors and Ground Truth Tracks in Vincennes (2025)</rdfs:label>
        <prov:wasAttributedTo rdf:resource="http://purl.org/www.umr-lastig.fr/geodata#amraimond"/>
        <prov:wasAttributedTo rdf:resource="http://purl.org/www.umr-lastig.fr/geodata#ymeneroux"/>
        <prov:wasQuotedFrom rdf:resource="https://intforout.github.io/outdoorPressure#SIGSPATIAL24VanDammeEtAl2024"/>
    </owl:NamedIndividual>
    


    <!-- https://intforout.github.io/outdoorPressure#MOUSLSGroundTruthDenseForestPath -->

    <owl:NamedIndividual rdf:about="https://intforout.github.io/outdoorPressure#MOUSLSGroundTruthDenseForestPath">
        <rdf:type rdf:resource="http://www.w3.org/ns/dcat#Dataset"/>
        <rdfs:comment xml:lang="en">This dataset was collected on-site by a group of students using a defined methodology. It contains precise station locations along a real-world path through dense forest, after reordering in the south–north direction of travel. The goal of these reference data is to obtain a very precise ground truth in order to assess the accuracy of GNSS tracks produced by following exactly the same path with five sensors: a Garmin watch, a Polar watch, the Visorando mobile application, a Keymaza GPS, and a Ublox GPS.</rdfs:comment>
        <dcat:distribution rdf:resource="https://intforout.github.io/outdoorPressure#GroundTruthDenseForestPath-csv"/>
        <dcat:inSeries rdf:resource="https://intforout.github.io/outdoorPressure#MOUSLS"/>
    </owl:NamedIndividual>
    


    <!-- https://intforout.github.io/outdoorPressure#MOUSLSTracksMultiSensorsVincennesForest -->

    <owl:NamedIndividual rdf:about="https://intforout.github.io/outdoorPressure#MOUSLSTracksMultiSensorsVincennesForest">
        <rdf:type rdf:resource="http://www.w3.org/ns/dcat#Dataset"/>
        <geodata:represents rdf:resource="https://intforout.github.io/outdoorPressure#HumanOutdoorActivitiesBoisVincennes2022"/>
        <rdfs:comment xml:lang="en">This dataset was collected by two researchers by following the data colection protocol and using five sensors Garmin watch, Polar watch, Visorando mobile phone application, Keymaza GPS, Ublox GPS. The study area covers dense forect in Vincennes forest (Paris).</rdfs:comment>
        <dcat:distribution rdf:resource="https://intforout.github.io/outdoorPressure#TracksMultiSensorsVincennesForest-gpkg"/>
        <dcat:inSeries rdf:resource="https://intforout.github.io/outdoorPressure#MOUSLS"/>
    </owl:NamedIndividual>
    


    <!-- https://intforout.github.io/outdoorPressure#MarchandEtAl2025MSEPeopleNatureDataActExport -->

    <owl:NamedIndividual rdf:about="https://intforout.github.io/outdoorPressure#MarchandEtAl2025MSEPeopleNatureDataActExport">
        <rdf:type rdf:resource="http://www.w3.org/ns/dcat#Dataset"/>
        <terms:issued rdf:datatype="http://www.w3.org/2001/XMLSchema#date">2025-09-04</terms:issued>
        <terms:language>English</terms:language>
        <terms:license rdf:resource="https://creativecommons.org/licenses/by/4.0/"/>
        <terms:publisher>Office Français de la Biodiversité</terms:publisher>
        <rdfs:comment xml:lang="en">Activity data from gps collars</rdfs:comment>
        <rdfs:label xml:lang="fr">act-export</rdfs:label>
        <dcat:distribution rdf:resource="https://intforout.github.io/outdoorPressure#marchandetal-rdata"/>
        <dcat:inSeries rdf:resource="https://intforout.github.io/outdoorPressure#MarchandEtAl2025MSEPeopleNatureDataZenodo"/>
    </owl:NamedIndividual>
    


    <!-- https://intforout.github.io/outdoorPressure#MarchandEtAl2025MSEPeopleNatureDataLocsExport -->

    <owl:NamedIndividual rdf:about="https://intforout.github.io/outdoorPressure#MarchandEtAl2025MSEPeopleNatureDataLocsExport">
        <rdf:type rdf:resource="http://www.w3.org/ns/dcat#Dataset"/>
        <terms:issued rdf:datatype="http://www.w3.org/2001/XMLSchema#date">2025-09-04</terms:issued>
        <terms:language>English</terms:language>
        <terms:license rdf:resource="https://creativecommons.org/licenses/by/4.0/"/>
        <terms:publisher>Office Français de la Biodiversité</terms:publisher>
        <rdfs:comment xml:lang="en">GPS locations</rdfs:comment>
        <rdfs:label xml:lang="fr">locs-export</rdfs:label>
        <dcat:distribution rdf:resource="https://intforout.github.io/outdoorPressure#marchandetal-rdata"/>
        <dcat:inSeries rdf:resource="https://intforout.github.io/outdoorPressure#MarchandEtAl2025MSEPeopleNatureDataZenodo"/>
    </owl:NamedIndividual>
    


    <!-- https://intforout.github.io/outdoorPressure#MarchandEtAl2025MSEPeopleNatureDataZenodo -->

    <owl:NamedIndividual rdf:about="https://intforout.github.io/outdoorPressure#MarchandEtAl2025MSEPeopleNatureDataZenodo">
        <rdf:type rdf:resource="http://www.w3.org/ns/dcat#DatasetSeries"/>
        <terms:bibliographicCitation>Marchand, P., Risser, N., Petit, E. &amp; Garel, M. (2025). Data from: Disturbance by massive sporting events in mountain areas: when and where matters for the protected Alpine ibex Capra ibex [Data set]. Zenodo. https://doi.org/10.5281/zenodo.17052197</terms:bibliographicCitation>
        <terms:issued rdf:datatype="http://www.w3.org/2001/XMLSchema#date">2025-09-04</terms:issued>
        <terms:language>English</terms:language>
        <terms:license rdf:resource="https://creativecommons.org/licenses/by/4.0/"/>
        <terms:publisher>Office Français de la Biodiversité</terms:publisher>
        <terms:spatial rdf:resource="https://intforout.github.io/outdoorPressure#RNCFSBauges"/>
        <datacite:relatedIdentifier>https://doi.org/10.5281/zenodo.17052197</datacite:relatedIdentifier>
        <rdfs:comment xml:lang="en">These R data files contains the data needed to replicate the analyses presented in Marchand et al. 2025  - Disturbance by massive sporting events in mountain areas: when and where matters for the protected Alpine ibex Capra ibex, published in People &amp; Nature. &apos;locs_export&apos; contains gps locations, whereas &apos;act_export&apos; contains activity data from gps collars. See Methods for details.</rdfs:comment>
        <rdfs:label xml:lang="en">Data from: Disturbance by massive sporting events in mountain areas: when and where matters for the protected Alpine ibex Capra ibex</rdfs:label>
        <dcat:distribution rdf:resource="https://intforout.github.io/outdoorPressure#marchandetal-rdata"/>
        <prov:wasAttributedTo rdf:resource="http://purl.org/www.umr-lastig.fr/geodata#mgarel"/>
        <prov:wasAttributedTo rdf:resource="http://purl.org/www.umr-lastig.fr/geodata#pmarchand"/>
        <prov:wasQuotedFrom rdf:resource="https://intforout.github.io/outdoorPressure#JournalOfPeopleAndNatureMarchandEtAl2025"/>
    </owl:NamedIndividual>
    


    <!-- https://intforout.github.io/outdoorPressure#MassifDesBauges -->

    <owl:NamedIndividual rdf:about="https://intforout.github.io/outdoorPressure#MassifDesBauges">
        <rdf:type rdf:resource="https://intforout.github.io/outdoorPressure#ReservesNaturelles"/>
        <rdfs:comment xml:lang="fr">Massif des Bauges</rdfs:comment>
    </owl:NamedIndividual>
    


    <!-- https://intforout.github.io/outdoorPressure#MergedTrack -->

    <owl:NamedIndividual rdf:about="https://intforout.github.io/outdoorPressure#MergedTrack"/>
    


    <!-- https://intforout.github.io/outdoorPressure#MergedTracksVincennes2024 -->

    <owl:NamedIndividual rdf:about="https://intforout.github.io/outdoorPressure#MergedTracksVincennes2024">
        <rdf:type rdf:resource="http://www.w3.org/ns/dcat#Dataset"/>
        <geodata:represents rdf:resource="https://intforout.github.io/outdoorPressure#HikersFootprintBoisVincennes"/>
        <rdfs:comment xml:lang="en">Merged tracks generated with the Track collection from Vincennes in 2024 by the MIAA algorithm</rdfs:comment>
        <rdfs:label xml:lang="en">Merged tracks in Vincennes</rdfs:label>
        <prov:wasGeneratedBy rdf:resource="https://intforout.github.io/outdoorPressure#PopulationFootprintFromTracksCollection"/>
        <prov:wasQuotedFrom rdf:resource="https://intforout.github.io/outdoorPressure#SIGSPATIAL24VanDammeEtAl2024"/>
    </owl:NamedIndividual>
    


    <!-- https://intforout.github.io/outdoorPressure#MetadataGroundTruthPathVincennesForest -->

    <owl:NamedIndividual rdf:about="https://intforout.github.io/outdoorPressure#MetadataGroundTruthPathVincennesForest">
        <rdf:type rdf:resource="http://www.w3.org/ns/dcat#CatalogRecord"/>
        <rdfs:comment xml:lang="en">Associated metadata (ISO 19115/19139 XML format, includes station details, measurement uncertainties, and spatial extent)</rdfs:comment>
        <dcat:accessURL rdf:resource="https://entrepot.recherche.data.gouv.fr/file.xhtml?persistentId=doi:10.57745/TRYLX1&amp;version=1.0"/>
        <dcat:conformsTo rdf:resource="https://www.iso.org/fr/standard/53798.html"/>
        <dcat:format>xml</dcat:format>
        <dcat:identifier>Metadata_ground_truth_path_vincennes_forest.xml</dcat:identifier>
        <dcat:issued rdf:datatype="http://www.w3.org/2001/XMLSchema#date">2025-08-13</dcat:issued>
        <foaf:primaryTopic rdf:resource="https://intforout.github.io/outdoorPressure#MOUSLSGroundTruthDenseForestPath"/>
    </owl:NamedIndividual>
    


    <!-- https://intforout.github.io/outdoorPressure#MetadataTracksMultiSensorsVincennesForest -->

    <owl:NamedIndividual rdf:about="https://intforout.github.io/outdoorPressure#MetadataTracksMultiSensorsVincennesForest">
        <rdf:type rdf:resource="http://www.w3.org/ns/dcat#CatalogRecord"/>
        <rdfs:comment xml:lang="en">Associated metadata (ISO 19115/19139 XML format, contains spatial extent, attributes description, collection method, and quality information)</rdfs:comment>
        <dcat:accessURL rdf:resource="https://entrepot.recherche.data.gouv.fr/file.xhtml?persistentId=doi:10.57745/Q6OT0J&amp;version=1.0"/>
        <dcat:conformsTo rdf:resource="https://www.iso.org/fr/standard/53798.html"/>
        <dcat:format>xml</dcat:format>
        <dcat:identifier>Metadata_tracks_multi_sensors_vincennes_forest.xml</dcat:identifier>
        <dcat:issued rdf:datatype="http://www.w3.org/2001/XMLSchema#date">2025-08-13</dcat:issued>
        <foaf:primaryTopic rdf:resource="https://intforout.github.io/outdoorPressure#MOUSLSTracksMultiSensorsVincennesForest"/>
    </owl:NamedIndividual>
    


    <!-- https://intforout.github.io/outdoorPressure#Movebank -->

    <owl:NamedIndividual rdf:about="https://intforout.github.io/outdoorPressure#Movebank">
        <rdf:type rdf:resource="http://purl.org/www.umr-lastig.fr/geodata#DataWarehouse"/>
        <terms:language>English</terms:language>
        <rdfs:comment xml:lang="en">Movebank is coordinated by the Max Planck Institute of Animal Behavior, the North Carolina Museum of Natural Sciences, the Senckenberg Society for Nature Research, and the University of Konstanz. </rdfs:comment>
        <rdfs:label xml:lang="en">Movebank is a free, online database of animal tracking data</rdfs:label>
    </owl:NamedIndividual>
    


    <!-- https://intforout.github.io/outdoorPressure#OVExportBaugesGeoPackage -->

    <owl:NamedIndividual rdf:about="https://intforout.github.io/outdoorPressure#OVExportBaugesGeoPackage">
        <rdf:type rdf:resource="http://www.w3.org/ns/dcat#Distribution"/>
        <dcat:format>geopackage</dcat:format>
        <dcat:identifier>Export_RNCFS_0.gpkg</dcat:identifier>
    </owl:NamedIndividual>
    


    <!-- https://intforout.github.io/outdoorPressure#OVExportChamonixGeoPackage -->

    <owl:NamedIndividual rdf:about="https://intforout.github.io/outdoorPressure#OVExportChamonixGeoPackage">
        <rdf:type rdf:resource="http://www.w3.org/ns/dcat#Distribution"/>
        <dcat:format>geopackage</dcat:format>
        <dcat:identifier>Export_Chamonix_0.gpkg</dcat:identifier>
    </owl:NamedIndividual>
    


    <!-- https://intforout.github.io/outdoorPressure#OVExportLesHouchesGeoPackage -->

    <owl:NamedIndividual rdf:about="https://intforout.github.io/outdoorPressure#OVExportLesHouchesGeoPackage">
        <rdf:type rdf:resource="http://www.w3.org/ns/dcat#Distribution"/>
        <dcat:format>geopackage</dcat:format>
        <dcat:identifier>Export_Les_Houches_0.gpkg</dcat:identifier>
    </owl:NamedIndividual>
    


    <!-- https://intforout.github.io/outdoorPressure#OVExportServozGeoPackage -->

    <owl:NamedIndividual rdf:about="https://intforout.github.io/outdoorPressure#OVExportServozGeoPackage">
        <rdf:type rdf:resource="http://www.w3.org/ns/dcat#Distribution"/>
        <dcat:format>geopackage</dcat:format>
        <dcat:identifier>Export_Servoz_0.gpkg</dcat:identifier>
    </owl:NamedIndividual>
    


    <!-- https://intforout.github.io/outdoorPressure#OVExportVallorcineGeoPackage -->

    <owl:NamedIndividual rdf:about="https://intforout.github.io/outdoorPressure#OVExportVallorcineGeoPackage">
        <rdf:type rdf:resource="http://www.w3.org/ns/dcat#Distribution"/>
        <dcat:format>geopackage</dcat:format>
        <dcat:identifier>Export_Vallorcine_0.gpkg</dcat:identifier>
    </owl:NamedIndividual>
    


    <!-- https://intforout.github.io/outdoorPressure#OVRecreationalUserMapService -->

    <owl:NamedIndividual rdf:about="https://intforout.github.io/outdoorPressure#OVRecreationalUserMapService">
        <rdf:type rdf:resource="http://www.w3.org/ns/dcat#DataService"/>
        <geodata:represents rdf:resource="https://intforout.github.io/outdoorPressure#HumanOutdoorActivitiesBauges2024"/>
        <geodata:represents rdf:resource="https://intforout.github.io/outdoorPressure#HumanOutdoorActivitiesMontBlanc2024"/>
        <terms:publisher rdf:resource="https://intforout.github.io/outdoorPressure#prnsn"/>
        <terms:spatial rdf:resource="https://intforout.github.io/outdoorPressure#RNCFSBauges"/>
        <terms:spatial rdf:resource="https://intforout.github.io/outdoorPressure#ZoneEtudeMontBlanc"/>
        <rdfs:comment xml:lang="fr">Ce flux de données permet de visualiser dans l’application Outdoorvision les tracés agrégés des traces GPS issus de services et d’objets connectés des pratiquants de sports et loisirs de nature. L’agrégation des flux s’appuie uniquement sur les traces GPS et ne prend pas en compte les contraintes spatiales comme le réseau routier. Cela permet de visualiser de façon précise la pratique sportive, les trajets réalisés qui peuvent être hors sentier.</rdfs:comment>
        <rdfs:comment xml:lang="en">This data feed enables visualization in the Outdoorvision application of aggregated GPS tracks obtained from services and connected devices used by outdoor sports and recreational users. The aggregation is based exclusively on GPS traces and does not account for spatial constraints, such as the road network. It provides a precise representation of sports activity and the paths taken, including off-trail routes.</rdfs:comment>
        <rdfs:label xml:lang="en">Recreational User Map Service</rdfs:label>
        <rdfs:label xml:lang="fr">Service diffusant des cartes de flux des pratiquants outdoor</rdfs:label>
    </owl:NamedIndividual>
    


    <!-- https://intforout.github.io/outdoorPressure#OVTracksMontBlancBauges2024 -->

    <owl:NamedIndividual rdf:about="https://intforout.github.io/outdoorPressure#OVTracksMontBlancBauges2024">
        <rdf:type rdf:resource="http://www.w3.org/ns/dcat#Dataset"/>
        <geodata:represents rdf:resource="https://intforout.github.io/outdoorPressure#HumanOutdoorActivitiesBauges2024"/>
        <geodata:represents rdf:resource="https://intforout.github.io/outdoorPressure#HumanOutdoorActivitiesMontBlanc2024"/>
        <rdfs:comment xml:lang="en">A set of tracks issued from Outdoorvision. GPS traces from outdoorvison are cleaned and filtered</rdfs:comment>
        <terms:publisher rdf:resource="https://intforout.github.io/outdoorPressure#prnsn"/>
        <terms:spatial rdf:resource="https://intforout.github.io/outdoorPressure#RNCFSBauges"/>
        <terms:spatial rdf:resource="https://intforout.github.io/outdoorPressure#ZoneEtudeMontBlanc"/>
        <rdfs:comment xml:lang="en">A set of tracks issued from Outdoorvision. GPS traces from outdoorvison are cleaned and filtered</rdfs:comment>
        <rdfs:label xml:lang="en">OutdoorVision export in Bauges and Mont Blanc in 2024</rdfs:label>
        <dcat:distribution rdf:resource="https://intforout.github.io/outdoorPressure#OVExportBaugesGeoPackage"/>
        <dcat:distribution rdf:resource="https://intforout.github.io/outdoorPressure#OVExportChamonixGeoPackage"/>
        <dcat:distribution rdf:resource="https://intforout.github.io/outdoorPressure#OVExportLesHouchesGeoPackage"/>
        <dcat:distribution rdf:resource="https://intforout.github.io/outdoorPressure#OVExportServozGeoPackage"/>
        <dcat:distribution rdf:resource="https://intforout.github.io/outdoorPressure#OVExportVallorcineGeoPackage"/>
        <dcat:keyword xml:lang="en">GPS traces</dcat:keyword>
    </owl:NamedIndividual>
    


    <!-- https://intforout.github.io/outdoorPressure#PNRBPOIBauges2025 -->

    <owl:NamedIndividual rdf:about="https://intforout.github.io/outdoorPressure#PNRBPOIBauges2025">
        <rdf:type rdf:resource="http://www.w3.org/ns/dcat#Dataset"/>
        <terms:issued rdf:datatype="http://www.w3.org/2001/XMLSchema#date">2025-05-01</terms:issued>
        <terms:language>fr-FR</terms:language>
        <terms:license rdf:resource="https://www.etalab.gouv.fr/licence-ouverte-open-licence"/>
        <terms:publisher rdf:resource="https://intforout.github.io/outdoorPressure#parcdesbauges"/>
        <rdfs:comment xml:lang="en">A set of POIs issued from Parcdesbauges.com.</rdfs:comment>
        <rdfs:label xml:lang="fr">Parcdesbauges.com - POI</rdfs:label>
        <dcat:distribution rdf:resource="https://intforout.github.io/outdoorPressure#parcdesbauges-poi-geojson"/>
    </owl:NamedIndividual>
    


    <!-- https://intforout.github.io/outdoorPressure#PNRBRoutesBauges2025 -->

    <owl:NamedIndividual rdf:about="https://intforout.github.io/outdoorPressure#PNRBRoutesBauges2025">
        <rdf:type rdf:resource="http://www.w3.org/ns/dcat#Dataset"/>
        <terms:issued rdf:datatype="http://www.w3.org/2001/XMLSchema#date">2025-05-01</terms:issued>
        <terms:language>fr-FR</terms:language>
        <terms:license rdf:resource="https://www.etalab.gouv.fr/licence-ouverte-open-licence"/>
        <terms:publisher rdf:resource="https://intforout.github.io/outdoorPressure#parcdesbauges"/>
        <rdfs:comment xml:lang="en">A set of treks issued from Parcdesbauges.com.</rdfs:comment>
        <rdfs:label xml:lang="fr">Parcdesbauges.com - trek</rdfs:label>
        <dcat:distribution rdf:resource="https://intforout.github.io/outdoorPressure#parcdesbauges-trek-geojson"/>
    </owl:NamedIndividual>
    


    <!-- https://intforout.github.io/outdoorPressure#PNRBSensitiveAreaBauges2025 -->

    <owl:NamedIndividual rdf:about="https://intforout.github.io/outdoorPressure#PNRBSensitiveAreaBauges2025">
        <rdf:type rdf:resource="http://www.w3.org/ns/dcat#Dataset"/>
        <terms:issued rdf:datatype="http://www.w3.org/2001/XMLSchema#date">2025-05-01</terms:issued>
        <terms:language>fr-FR</terms:language>
        <terms:license rdf:resource="https://www.etalab.gouv.fr/licence-ouverte-open-licence"/>
        <terms:publisher rdf:resource="https://intforout.github.io/outdoorPressure#parcdesbauges"/>
        <rdfs:comment xml:lang="en">A set of sensitive area issued from Parcdesbauges.com.</rdfs:comment>
        <rdfs:label xml:lang="fr">Parcdesbauges.com - sensitivearea</rdfs:label>
        <dcat:distribution rdf:resource="https://intforout.github.io/outdoorPressure#parcdesbauges-sensitivearea-geojson"/>
    </owl:NamedIndividual>
    


    <!-- https://intforout.github.io/outdoorPressure#PNRDesBauges -->

    <owl:NamedIndividual rdf:about="https://intforout.github.io/outdoorPressure#PNRDesBauges">
        <rdf:type rdf:resource="http://purl.org/dc/terms/Location"/>
        <rdfs:comment xml:lang="fr">Le parc naturel régional du Massif des Bauges est une aire protégée</rdfs:comment>
        <rdfs:label>Parc naturel régional du Massif des Bauges</rdfs:label>
    </owl:NamedIndividual>
    


    <!-- https://intforout.github.io/outdoorPressure#PopulationFootprintFromTracksCollection -->

    <owl:NamedIndividual rdf:about="https://intforout.github.io/outdoorPressure#PopulationFootprintFromTracksCollection">
        <rdf:type rdf:resource="http://purl.org/www.umr-lastig.fr/geodata#Process"/>
        <rdfs:comment xml:lang="en">A modular and iterative aggregation algorithm (MIAA)</rdfs:comment>
        <rdfs:label xml:lang="en">Population footprint from a tracks collection</rdfs:label>
        <prov:endedAtTime rdf:datatype="http://www.w3.org/2001/XMLSchema#gYearMonth">2024-06</prov:endedAtTime>
        <prov:generated rdf:resource="https://intforout.github.io/outdoorPressure#MergedTracksVincennes2024"/>
        <prov:startedAtTime rdf:datatype="http://www.w3.org/2001/XMLSchema#gYearMonth">2024-05</prov:startedAtTime>
        <prov:used rdf:resource="https://intforout.github.io/outdoorPressure#MOUSLS"/>
        <prov:wasAssociatedWith rdf:resource="http://purl.org/www.umr-lastig.fr/geodata#Tracklib"/>
        <prov:wasAttributedTo rdf:resource="http://purl.org/www.umr-lastig.fr/geodata#mdvandamme"/>
    </owl:NamedIndividual>
    


    <!-- https://intforout.github.io/outdoorPressure#ProfilageOutdoorVision -->

    <owl:NamedIndividual rdf:about="https://intforout.github.io/outdoorPressure#ProfilageOutdoorVision">
        <rdf:type rdf:resource="http://purl.org/www.umr-lastig.fr/geodata#UserFeedback"/>
        <terms:creator rdf:resource="https://intforout.github.io/outdoorPressure#anaciri"/>
        <rdfs:comment xml:lang="fr">Profil des données outdoorvision dans un format PDF pour le projet IntForOut</rdfs:comment>
    </owl:NamedIndividual>
    


    <!-- https://intforout.github.io/outdoorPressure#QualityOfOVRecreationalUserMapService -->

    <owl:NamedIndividual rdf:about="https://intforout.github.io/outdoorPressure#QualityOfOVRecreationalUserMapService">
        <rdf:type rdf:resource="http://purl.org/www.umr-lastig.fr/geodata#UserFeedback"/>
        <geodata:target rdf:resource="https://intforout.github.io/outdoorPressure#OVRecreationalUserMapService"/>
        <terms:creator rdf:resource="http://purl.org/www.umr-lastig.fr/geodata#mdvandamme"/>
        <rdfs:comment xml:lang="en">Artifacts exist in dense urban areas above a certain zoom level. This is because the accuracy of GPS tracks is lower in these areas, making the spatial information displayed less relevant.</rdfs:comment>
    </owl:NamedIndividual>
    


    <!-- https://intforout.github.io/outdoorPressure#RNCFSBauges -->

    <owl:NamedIndividual rdf:about="https://intforout.github.io/outdoorPressure#RNCFSBauges">
        <rdf:type rdf:resource="http://purl.org/dc/terms/Location"/>
        <rdfs:comment xml:lang="fr">La Réserve de chasse et de faune sauvage des Bauges est située dans la partie Est du massif des Bauges et comprend la plupart de ses plus hauts sommets dont le point culminant de l’Arcalod (2217 m). D’une superficie de 5 200 hectares, elle s’étend sur 12 communes des départements de Haute-Savoie (26%) et de Savoie (74%).</rdfs:comment>
        <rdfs:label>La Réserve nationale de chasse et de faune sauvage des Bauges</rdfs:label>
    </owl:NamedIndividual>
    


    <!-- https://intforout.github.io/outdoorPressure#RefugesInfoPOIBauges2025 -->

    <owl:NamedIndividual rdf:about="https://intforout.github.io/outdoorPressure#RefugesInfoPOIBauges2025">
        <rdf:type rdf:resource="http://www.w3.org/ns/dcat#Dataset"/>
        <terms:issued rdf:datatype="http://www.w3.org/2001/XMLSchema#date">2025-05-01</terms:issued>
        <terms:language>fr-FR</terms:language>
        <terms:license rdf:resource="http://creativecommons.org/licenses/by-sa/2.0/deed.fr"/>
        <terms:publisher rdf:resource="https://intforout.github.io/outdoorPressure#refugesinfo"/>
        <rdfs:comment xml:lang="en">A set of Points issued from Refuges.info.</rdfs:comment>
        <rdfs:label xml:lang="en">Refuges.info - points</rdfs:label>
        <dcat:distribution rdf:resource="https://intforout.github.io/outdoorPressure#refugesinfo-points-geojson"/>
    </owl:NamedIndividual>
    


    <!-- https://intforout.github.io/outdoorPressure#ReplicabilityTrackCollectionAggregation -->

    <owl:NamedIndividual rdf:about="https://intforout.github.io/outdoorPressure#ReplicabilityTrackCollectionAggregation">
        <rdf:type rdf:resource="http://purl.org/www.umr-lastig.fr/geodata#UserFeedback"/>
        <geodata:target rdf:resource="https://intforout.github.io/outdoorPressure#OVTracksMontBlancBauges2024"/>
        <geodata:target rdf:resource="https://intforout.github.io/outdoorPressure#SIGSPATIAL24VanDammeEtAl2024"/>
        <terms:creator rdf:resource="http://purl.org/www.umr-lastig.fr/geodata#mdvandamme"/>
        <rdfs:comment xml:lang="en">The process proposed in this paper can probably be reproduced to generate HikersFootprint in Les Bauges and MontBlanc, using OutdoorVision data as an input</rdfs:comment>
    </owl:NamedIndividual>
    


    <!-- https://intforout.github.io/outdoorPressure#SIGSPATIAL24VanDammeEtAl2024 -->

    <owl:NamedIndividual rdf:about="https://intforout.github.io/outdoorPressure#SIGSPATIAL24VanDammeEtAl2024">
        <rdf:type rdf:resource="http://purl.org/www.umr-lastig.fr/geodata#ScientificPaper"/>
        <terms:creator rdf:resource="http://purl.org/www.umr-lastig.fr/geodata#amraimond"/>
        <terms:creator rdf:resource="http://purl.org/www.umr-lastig.fr/geodata#mdvandamme"/>
        <terms:creator rdf:resource="http://purl.org/www.umr-lastig.fr/geodata#ymeneroux"/>
        <terms:hasPart rdf:resource="https://intforout.github.io/outdoorPressure#MOUSLS"/>
        <terms:isPartOf>Proceedings of the 32nd ACM International Conference on Advances in Geographic Information Systems</terms:isPartOf>
        <terms:isPartOf>SIGSPATIAL &apos;24</terms:isPartOf>
        <terms:publisher>Association for Computing Machinery</terms:publisher>
        <terms:spatial>Atlanta, GA, USA</terms:spatial>
        <datacite:firstPage>633</datacite:firstPage>
        <datacite:lastPage>636</datacite:lastPage>
        <datacite:publicationYear>2024</datacite:publicationYear>
        <datacite:relatedIdentifier>10.1145/3678717.3691325</datacite:relatedIdentifier>
        <datacite:relatedIdentifier>https://doi.org/10.1145/3678717.3691325</datacite:relatedIdentifier>
        <datacite:resourceType rdf:resource="http://purl.org/spar/datacite/ConferenceProceeding"/>
        <datacite:subject>global navigation satellite system</datacite:subject>
        <datacite:subject>metrological analysis</datacite:subject>
        <datacite:subject>synthetic and real world trajectories</datacite:subject>
        <datacite:subject>trajectory aggregation</datacite:subject>
        <rdfs:label xml:lang="en">A metrological analysis of a modular and iterative aggregation algorithm of GNSS trajectories</rdfs:label>
        <prov:quotedAs rdf:resource="https://intforout.github.io/outdoorPressure#MOUSLS"/>
        <prov:quotedAs rdf:resource="https://intforout.github.io/outdoorPressure#MergedTracksVincennes2024"/>
        <prov:wasInfluencedBy rdf:resource="https://intforout.github.io/outdoorPressure#PopulationFootprintFromTracksCollection"/>
    </owl:NamedIndividual>
    


    <!-- https://intforout.github.io/outdoorPressure#SentierDesBauges -->

    <owl:NamedIndividual rdf:about="https://intforout.github.io/outdoorPressure#SentierDesBauges">
        <rdf:type rdf:resource="https://intforout.github.io/outdoorPressure#Sentier"/>
        <outdoorPressure:affords rdf:resource="https://intforout.github.io/outdoorPressure#HikingInLesBauges"/>
    </owl:NamedIndividual>
    


    <!-- https://intforout.github.io/outdoorPressure#SkiLiftCountersMontBlanc2008To2024 -->

    <owl:NamedIndividual rdf:about="https://intforout.github.io/outdoorPressure#SkiLiftCountersMontBlanc2008To2024">
        <rdf:type rdf:resource="http://www.w3.org/ns/dcat#Dataset"/>
        <geodata:represents rdf:resource="https://intforout.github.io/outdoorPressure#SkiLiftUsageMontBlanc2008To2024"/>
        <rdfs:comment xml:lang="en">Counting data for each ski lift, including their locations (start and end points), over a 10-year period (one file per year).</rdfs:comment>
        <rdfs:label xml:lang="en">Ski Lift Ridership Counts in the CMB Area.</rdfs:label>
    </owl:NamedIndividual>
    


    <!-- https://intforout.github.io/outdoorPressure#SkiLiftUsageMontBlanc2008To2024 -->

    <owl:NamedIndividual rdf:about="https://intforout.github.io/outdoorPressure#SkiLiftUsageMontBlanc2008To2024">
        <rdf:type rdf:resource="https://intforout.github.io/outdoorPressure#HumanActivity"/>
    </owl:NamedIndividual>
    


    <!-- https://intforout.github.io/outdoorPressure#Strava -->

    <owl:NamedIndividual rdf:about="https://intforout.github.io/outdoorPressure#Strava">
        <rdf:type rdf:resource="http://www.w3.org/ns/prov#Organization"/>
        <rdfs:comment xml:lang="en">american internet service for tracking physical exercise which incorporates social networking features. It tracks outdoor activities using GPS data, and other exercise types, including indoor activities. Strava records data for a user&apos;s activities, which can then be shared with the user&apos;s followers or shared publicly. If an activity is shared publicly, Strava automatically groups activities that occur at the same time and place (such as taking part in a marathon, sportive or group ride). An activity&apos;s recorded information may include a route summary, elevation (net and unidirectional), speed (average and maximum), timing (total and moving time), power and heart rate. Activities can be recorded using the mobile app or from devices manufactured by third parties like Garmin, Google Fit, Suunto, and Wahoo. Activities can also be entered manually via the Strava website and mobile app. (quoted from wikipedia)</rdfs:comment>
        <rdfs:seeAlso>https://www.wikidata.org/wiki/Q13884156</rdfs:seeAlso>
        <foaf:homePage>https://www.strava.com/about</foaf:homePage>
    </owl:NamedIndividual>
    


    <!-- https://intforout.github.io/outdoorPressure#StravaMetro -->

    <owl:NamedIndividual rdf:about="https://intforout.github.io/outdoorPressure#StravaMetro">
        <rdf:type rdf:resource="http://purl.org/www.umr-lastig.fr/geodata#DataWarehouse"/>
        <terms:language>English</terms:language>
        <terms:publisher rdf:resource="https://intforout.github.io/outdoorPressure#Strava"/>
        <rdfs:comment xml:lang="en">Aggregated and de-identified Strava data</rdfs:comment>
        <rdfs:label xml:lang="en">Strava Metro data set</rdfs:label>
        <rdfs:seeAlso>https://www.wikidata.org/wiki/Q114074281</rdfs:seeAlso>
    </owl:NamedIndividual>
    


    <!-- https://intforout.github.io/outdoorPressure#StravaMetroTracksMontBlanc2024 -->

    <owl:NamedIndividual rdf:about="https://intforout.github.io/outdoorPressure#StravaMetroTracksMontBlanc2024">
        <rdf:type rdf:resource="http://www.w3.org/ns/dcat#Dataset"/>
        <geodata:represents rdf:resource="https://intforout.github.io/outdoorPressure#HumanOutdoorActivitiesBauges2014"/>
        <dc:publisher rdf:resource="https://intforout.github.io/outdoorPressure#Strava"/>
    </owl:NamedIndividual>
    


    <!-- https://intforout.github.io/outdoorPressure#StravaRecreationalUserMapService -->

    <owl:NamedIndividual rdf:about="https://intforout.github.io/outdoorPressure#StravaRecreationalUserMapService">
        <rdf:type rdf:resource="http://www.w3.org/ns/dcat#DataService"/>
        <geodata:represents rdf:resource="https://intforout.github.io/outdoorPressure#HumanOutdoorActivitiesBauges2024"/>
        <geodata:represents rdf:resource="https://intforout.github.io/outdoorPressure#HumanOutdoorActivitiesMontBlanc2024"/>
        <terms:publisher rdf:resource="https://intforout.github.io/outdoorPressure#Strava"/>
        <rdfs:comment xml:lang="en">Displays the aggregated public activities recorded in Strava over the past year</rdfs:comment>
        <rdfs:comment xml:lang="fr">Montre les activités publiques agrégées au cours de l&apos;année passée dans Strava</rdfs:comment>
        <rdfs:label xml:lang="fr">Carte mondiale des activités Strava</rdfs:label>
        <rdfs:label xml:lang="en">Strava Global Heatmap</rdfs:label>
        <rdfs:seeAlso>https://www.wikidata.org/wiki/Q114074364</rdfs:seeAlso>
    </owl:NamedIndividual>
    


    <!-- https://intforout.github.io/outdoorPressure#StravaTracksBauges2014 -->

    <owl:NamedIndividual rdf:about="https://intforout.github.io/outdoorPressure#StravaTracksBauges2014">
        <rdf:type rdf:resource="http://www.w3.org/ns/dcat#Dataset"/>
        <geodata:represents rdf:resource="https://intforout.github.io/outdoorPressure#HumanOutdoorActivitiesBauges2014"/>
        <dc:publisher rdf:resource="https://intforout.github.io/outdoorPressure#Strava"/>
    </owl:NamedIndividual>
    


    <!-- https://intforout.github.io/outdoorPressure#TopometricSurveyGroundTruthPathVincennes2024 -->

    <owl:NamedIndividual rdf:about="https://intforout.github.io/outdoorPressure#TopometricSurveyGroundTruthPathVincennes2024">
        <rdf:type rdf:resource="https://intforout.github.io/outdoorPressure#Observation"/>
        <terms:creator rdf:resource="https://intforout.github.io/outdoorPressure#blabbe"/>
        <terms:creator rdf:resource="https://intforout.github.io/outdoorPressure#lpeseux"/>
        <terms:creator rdf:resource="https://intforout.github.io/outdoorPressure#pcalloch"/>
        <prov:endedAtTime rdf:datatype="http://www.w3.org/2001/XMLSchema#gYearMonth">2024-01-18</prov:endedAtTime>
        <prov:generated rdf:resource="https://intforout.github.io/outdoorPressure#MOUSLSGroundTruthDenseForestPath"/>
        <prov:startedAtTime rdf:datatype="http://www.w3.org/2001/XMLSchema#gYearMonth">2024-01-18</prov:startedAtTime>
        <prov:used rdf:resource="ttp://purl.org/www.umr-lastig.fr/geodata#LeicaTS16"/>
    </owl:NamedIndividual>
    


    <!-- https://intforout.github.io/outdoorPressure#TracksMultiSensorsVincennesForest-gpkg -->

    <owl:NamedIndividual rdf:about="https://intforout.github.io/outdoorPressure#TracksMultiSensorsVincennesForest-gpkg">
        <rdf:type rdf:resource="http://www.w3.org/ns/dcat#Distribution"/>
        <dcat:accessURL rdf:resource="https://entrepot.recherche.data.gouv.fr/file.xhtml?persistentId=doi:10.57745/NSMUWN&amp;version=1.0"/>
        <dcat:format>gpkg</dcat:format>
        <dcat:identifier>tracks_multi_sensors_vincennes_forest.gpkg</dcat:identifier>
    </owl:NamedIndividual>
    


    <!-- https://intforout.github.io/outdoorPressure#VisorandoRoutesBauges2025 -->

    <owl:NamedIndividual rdf:about="https://intforout.github.io/outdoorPressure#VisorandoRoutesBauges2025">
        <rdf:type rdf:resource="http://www.w3.org/ns/dcat#Dataset"/>
        <terms:issued rdf:datatype="http://www.w3.org/2001/XMLSchema#date">2025-05-01</terms:issued>
        <terms:language>fr-FR</terms:language>
        <terms:license rdf:resource="https://opendatacommons.org/licenses/odbl/"/>
        <terms:publisher rdf:resource="https://intforout.github.io/outdoorPressure#visorando"/>
        <rdfs:comment xml:lang="en">A set of routes issued from visorando.com.</rdfs:comment>
        <rdfs:label xml:lang="en">Visorando Hiking Routes in the Bauges Massif (2025)</rdfs:label>
    </owl:NamedIndividual>
    


    <!-- https://intforout.github.io/outdoorPressure#WildlifeMonitoringFromCameraTrapImage -->

    <owl:NamedIndividual rdf:about="https://intforout.github.io/outdoorPressure#WildlifeMonitoringFromCameraTrapImage">
        <rdf:type rdf:resource="http://purl.org/www.umr-lastig.fr/geodata#Process"/>
        <rdfs:comment xml:lang="en">Les données pièges-photos seront actualisées par Marjorie en janvier. A noter que les sorties DeepFaune étaient indiquées dans les données ouvertes et qu’elles ont été décalées dans la partie sous convention (à n’utiliser que dans le cadre du consortium, comme les autres données CREA-partenaires)</rdfs:comment>
        <prov:wasAssociatedWith rdf:resource="https://intforout.github.io/outdoorPressure#DeepFaune"/>
    </owl:NamedIndividual>
    


    <!-- https://intforout.github.io/outdoorPressure#ZoneEtudeMontBlanc -->

    <owl:NamedIndividual rdf:about="https://intforout.github.io/outdoorPressure#ZoneEtudeMontBlanc">
        <rdf:type rdf:resource="http://purl.org/dc/terms/Location"/>
        <rdfs:label>Massif du Mont Blanc, côté France</rdfs:label>
    </owl:NamedIndividual>
    


    <!-- https://intforout.github.io/outdoorPressure#aloison -->

    <owl:NamedIndividual rdf:about="https://intforout.github.io/outdoorPressure#aloison">
        <rdf:type rdf:resource="http://www.w3.org/ns/prov#Person"/>
        <foaf:name>Anne Loison</foaf:name>
    </owl:NamedIndividual>
    


    <!-- https://intforout.github.io/outdoorPressure#altituderando -->

    <owl:NamedIndividual rdf:about="https://intforout.github.io/outdoorPressure#altituderando">
        <rdf:type rdf:resource="http://www.w3.org/ns/prov#Organization"/>
        <foaf:homePage rdf:resource="https://www.altituderando.com"/>
        <foaf:name>Altituderando</foaf:name>
    </owl:NamedIndividual>
    


    <!-- https://intforout.github.io/outdoorPressure#anaciri -->

    <owl:NamedIndividual rdf:about="https://intforout.github.io/outdoorPressure#anaciri">
        <rdf:type rdf:resource="http://www.w3.org/ns/prov#Person"/>
        <foaf:name>Abdassalam Naciri</foaf:name>
    </owl:NamedIndividual>
    


    <!-- https://intforout.github.io/outdoorPressure#api-camptocamp -->

    <owl:NamedIndividual rdf:about="https://intforout.github.io/outdoorPressure#api-camptocamp">
        <rdf:type rdf:resource="http://www.w3.org/ns/dcat#DataService"/>
        <terms:license rdf:resource="https://opendatacommons.org/licenses/odbl/"/>
        <terms:publisher rdf:resource="https://intforout.github.io/outdoorPressure#camptocamp"/>
        <rdfs:comment xml:lang="fr">API du site collaboratif et interactif camptocamp.org. On peut y trouver des informations sur la montagne : conditions sur le terrain (manteau neigeux par exemple), descriptions de sommets, itinéraires de ski de randonnée ou grandes voies d’escalade par exemple, photographies, articles techniques ou récits de montagne. Certaines de ces informations sont modifiables par tout contributeur enregistré . Vous y trouverez aussi un forum qui vous permet d’échanger.</rdfs:comment>
        <rdfs:label xml:lang="en">API de Camptocamp.org (routes, waypoints, outings)</rdfs:label>
        <dcat:accessURL rdf:resource="https://api.camptocamp.org/"/>
        <dcat:servesDataset rdf:resource="https://intforout.github.io/outdoorPressure#CamptocampPoisBauges2025"/>
        <dcat:servesDataset rdf:resource="https://intforout.github.io/outdoorPressure#CamptocampRoutesBauges2025"/>
        <foaf:homePage rdf:resource="https://www.camptocamp.org/"/>
    </owl:NamedIndividual>
    


    <!-- https://intforout.github.io/outdoorPressure#api-parcdesbauges -->

    <owl:NamedIndividual rdf:about="https://intforout.github.io/outdoorPressure#api-parcdesbauges">
        <rdf:type rdf:resource="http://www.w3.org/ns/dcat#DataService"/>
        <terms:license rdf:resource="https://www.etalab.gouv.fr/licence-ouverte-open-licence"/>
        <terms:publisher rdf:resource="https://intforout.github.io/outdoorPressure#parcdesbauges"/>
        <rdfs:comment xml:lang="fr">L&apos;API du PNR Massif des Bauges met en valeur la randonnée pédestre, sentier et activités touristiques en offrant une pléthore de requêtes pour accéder données.</rdfs:comment>
        <rdfs:label xml:lang="en">API du PNR Massif des Bauges</rdfs:label>
        <dcat:accessURL rdf:resource="https://geotrek.parcdesbauges.com/api/v2/"/>
        <dcat:servesDataset rdf:resource="https://intforout.github.io/outdoorPressure#PNRBPOIBauges2025"/>
        <dcat:servesDataset rdf:resource="https://intforout.github.io/outdoorPressure#PNRBRoutesBauges2025"/>
        <dcat:servesDataset rdf:resource="https://intforout.github.io/outdoorPressure#PNRBSensitiveAreaBauges2025"/>
    </owl:NamedIndividual>
    


    <!-- https://intforout.github.io/outdoorPressure#api-refugesinfo -->

    <owl:NamedIndividual rdf:about="https://intforout.github.io/outdoorPressure#api-refugesinfo">
        <rdf:type rdf:resource="http://www.w3.org/ns/dcat#DataService"/>
        <terms:license rdf:resource="http://creativecommons.org/licenses/by-sa/2.0/deed.fr"/>
        <terms:publisher rdf:resource="https://intforout.github.io/outdoorPressure#refugesinfo"/>
        <rdfs:comment xml:lang="fr">L&apos;API de Refuges.info est un service web personnel et non commercial permettant de se renseigner sur les hébergements de montagnes destinés aux randonneurs. Elle permet de recevoir dans de nombreux formats une liste de points, des informations détaillées sur un point ou encore les résultats de requêtes spéciales telles que la recherche de points.</rdfs:comment>
        <rdfs:label xml:lang="en">API de Refuges.info (points)</rdfs:label>
        <dcat:accessURL rdf:resource="https://www.refuges.info/api/"/>
        <dcat:servesDataset rdf:resource="https://intforout.github.io/outdoorPressure#RefugesInfoPOIBauges2025"/>
    </owl:NamedIndividual>
    


    <!-- https://intforout.github.io/outdoorPressure#blabbe -->

    <owl:NamedIndividual rdf:about="https://intforout.github.io/outdoorPressure#blabbe">
        <rdf:type rdf:resource="http://www.w3.org/ns/prov#Person"/>
        <foaf:name>Brice Labbé</foaf:name>
    </owl:NamedIndividual>
    


    <!-- https://intforout.github.io/outdoorPressure#c2c-route-geojson -->

    <owl:NamedIndividual rdf:about="https://intforout.github.io/outdoorPressure#c2c-route-geojson">
        <rdf:type rdf:resource="http://www.w3.org/ns/dcat#Distribution"/>
        <dcat:accessService rdf:resource="https://intforout.github.io/outdoorPressure#api-camptocamp"/>
        <dcat:format>GeoJSON</dcat:format>
    </owl:NamedIndividual>
    


    <!-- https://intforout.github.io/outdoorPressure#c2c-waypoint-geojson -->

    <owl:NamedIndividual rdf:about="https://intforout.github.io/outdoorPressure#c2c-waypoint-geojson">
        <rdf:type rdf:resource="http://www.w3.org/ns/dcat#Distribution"/>
        <dcat:accessService rdf:resource="https://intforout.github.io/outdoorPressure#api-camptocamp"/>
        <dcat:format>GeoJSON</dcat:format>
    </owl:NamedIndividual>
    


    <!-- https://intforout.github.io/outdoorPressure#camptocamp -->

    <owl:NamedIndividual rdf:about="https://intforout.github.io/outdoorPressure#camptocamp">
        <rdf:type rdf:resource="http://www.w3.org/ns/prov#Organization"/>
        <foaf:homePage rdf:resource="https://www.camptocamp.org/"/>
        <foaf:name>Camptocamp Association</foaf:name>
    </owl:NamedIndividual>
    


    <!-- https://intforout.github.io/outdoorPressure#cirkwi -->

    <owl:NamedIndividual rdf:about="https://intforout.github.io/outdoorPressure#cirkwi">
        <rdf:type rdf:resource="http://www.w3.org/ns/prov#Organization"/>
        <foaf:homePage rdf:resource="https://www.cirkwi.com/"/>
        <foaf:name>Cirkwi</foaf:name>
    </owl:NamedIndividual>
    


    <!-- https://intforout.github.io/outdoorPressure#lpeseux -->

    <owl:NamedIndividual rdf:about="https://intforout.github.io/outdoorPressure#lpeseux">
        <rdf:type rdf:resource="http://www.w3.org/ns/prov#Person"/>
        <foaf:name>Lorine Peseux</foaf:name>
    </owl:NamedIndividual>
    


    <!-- https://intforout.github.io/outdoorPressure#marchandetal-rdata -->

    <owl:NamedIndividual rdf:about="https://intforout.github.io/outdoorPressure#marchandetal-rdata">
        <rdf:type rdf:resource="http://www.w3.org/ns/dcat#Distribution"/>
        <dcat:format>RData</dcat:format>
    </owl:NamedIndividual>
    


    <!-- https://intforout.github.io/outdoorPressure#mgarel -->

    <owl:NamedIndividual rdf:about="https://intforout.github.io/outdoorPressure#mgarel">
        <rdf:type rdf:resource="http://www.w3.org/ns/prov#Person"/>
        <foaf:name>Mathieu Garel</foaf:name>
    </owl:NamedIndividual>
    


    <!-- https://intforout.github.io/outdoorPressure#openstreetmap -->

    <owl:NamedIndividual rdf:about="https://intforout.github.io/outdoorPressure#openstreetmap">
        <rdf:type rdf:resource="http://www.w3.org/ns/prov#Organization"/>
        <foaf:homePage rdf:resource="https://www.openstreetmap.org"/>
        <foaf:name>OpenStreetMap (OSM)</foaf:name>
    </owl:NamedIndividual>
    


    <!-- https://intforout.github.io/outdoorPressure#outdoorvision -->

    <owl:NamedIndividual rdf:about="https://intforout.github.io/outdoorPressure#outdoorvision">
        <rdf:type rdf:resource="http://www.w3.org/ns/dcat#Catalog"/>
        <terms:publisher rdf:resource="https://intforout.github.io/outdoorPressure#prnsn"/>
        <rdfs:comment xml:lang="en">Outdoorvision https://outdoorvision.fr/; is a service to gather GPS tracks voluntarily shared by human during their outdoor activity through their accounts on their mobile device Garmin Connect™ / Polar Flow / Suunto APP (Appli Suunto) / Decathlon. The data are anonymized and published for a list of authorised users. It is offered by the French National Resource Centre for Ecological Transition and Outdoor Sports, a support mission of the Ministry of Sport. It results from a partnership between local authorities, sports federations and brands united around a non-profit programme.</rdfs:comment>
        <rdfs:label xml:lang="en">OutdoorVision Catalog</rdfs:label>
        <dcat:dataset rdf:resource="https://intforout.github.io/outdoorPressure#OVTracksMontBlancBauges2024"/>
        <dcat:service rdf:resource="https://intforout.github.io/outdoorPressure#OVRecreationalUserMapService"/>
        <foaf:homePage>https://outdoorvision.fr/</foaf:homePage>
    </owl:NamedIndividual>
    


    <!-- https://intforout.github.io/outdoorPressure#parcdesbauges -->

    <owl:NamedIndividual rdf:about="https://intforout.github.io/outdoorPressure#parcdesbauges">
        <rdf:type rdf:resource="http://www.w3.org/ns/prov#Organization"/>
        <foaf:homePage rdf:resource="https://parcdesbauges.com"/>
        <foaf:name>Parc Naturel Régional du Massif des Bauges</foaf:name>
    </owl:NamedIndividual>
    


    <!-- https://intforout.github.io/outdoorPressure#parcdesbauges-poi-geojson -->

    <owl:NamedIndividual rdf:about="https://intforout.github.io/outdoorPressure#parcdesbauges-poi-geojson">
        <rdf:type rdf:resource="http://www.w3.org/ns/dcat#Distribution"/>
        <dcat:accessService rdf:resource="https://intforout.github.io/outdoorPressure#api-parcdesbauges"/>
        <dcat:format>GeoJSON</dcat:format>
    </owl:NamedIndividual>
    


    <!-- https://intforout.github.io/outdoorPressure#parcdesbauges-sensitivearea-geojson -->

    <owl:NamedIndividual rdf:about="https://intforout.github.io/outdoorPressure#parcdesbauges-sensitivearea-geojson">
        <rdf:type rdf:resource="http://www.w3.org/ns/dcat#Distribution"/>
        <dcat:accessService rdf:resource="https://intforout.github.io/outdoorPressure#api-parcdesbauges"/>
        <dcat:format>GeoJSON</dcat:format>
    </owl:NamedIndividual>
    


    <!-- https://intforout.github.io/outdoorPressure#parcdesbauges-trek-geojson -->

    <owl:NamedIndividual rdf:about="https://intforout.github.io/outdoorPressure#parcdesbauges-trek-geojson">
        <rdf:type rdf:resource="http://www.w3.org/ns/dcat#Distribution"/>
        <dcat:accessService rdf:resource="https://intforout.github.io/outdoorPressure#api-parcdesbauges"/>
        <dcat:format>GeoJSON</dcat:format>
    </owl:NamedIndividual>
    


    <!-- https://intforout.github.io/outdoorPressure#pcalloch -->

    <owl:NamedIndividual rdf:about="https://intforout.github.io/outdoorPressure#pcalloch">
        <rdf:type rdf:resource="http://www.w3.org/ns/prov#Person"/>
        <foaf:name>Paul Calloch</foaf:name>
    </owl:NamedIndividual>
    


    <!-- https://intforout.github.io/outdoorPressure#pmarchand -->

    <owl:NamedIndividual rdf:about="https://intforout.github.io/outdoorPressure#pmarchand">
        <rdf:type rdf:resource="http://www.w3.org/ns/prov#Person"/>
        <foaf:name>Pascal Marchand</foaf:name>
    </owl:NamedIndividual>
    


    <!-- https://intforout.github.io/outdoorPressure#prnsn -->

    <owl:NamedIndividual rdf:about="https://intforout.github.io/outdoorPressure#prnsn">
        <rdf:type rdf:resource="http://www.w3.org/ns/prov#Organization"/>
        <rdfs:label>Pôle ressources national sports de nature (PRNSN)</rdfs:label>
    </owl:NamedIndividual>
    


    <!-- https://intforout.github.io/outdoorPressure#refugesinfo -->

    <owl:NamedIndividual rdf:about="https://intforout.github.io/outdoorPressure#refugesinfo">
        <rdf:type rdf:resource="http://www.w3.org/ns/prov#Organization"/>
        <foaf:homePage rdf:resource="https://www.refuges.info/"/>
        <foaf:name>Refuges.info</foaf:name>
    </owl:NamedIndividual>
    


    <!-- https://intforout.github.io/outdoorPressure#refugesinfo-points-geojson -->

    <owl:NamedIndividual rdf:about="https://intforout.github.io/outdoorPressure#refugesinfo-points-geojson">
        <rdf:type rdf:resource="http://www.w3.org/ns/dcat#Distribution"/>
        <dcat:accessService rdf:resource="https://intforout.github.io/outdoorPressure#api-refugesinfo"/>
        <dcat:format>GeoJSON</dcat:format>
    </owl:NamedIndividual>
    


    <!-- https://intforout.github.io/outdoorPressure#visorando -->

    <owl:NamedIndividual rdf:about="https://intforout.github.io/outdoorPressure#visorando">
        <rdf:type rdf:resource="http://www.w3.org/ns/prov#Organization"/>
        <foaf:homePage rdf:resource="https://www.visorando.com/"/>
        <foaf:name>Visorando</foaf:name>
    </owl:NamedIndividual>
    


    <!-- https://www.refuges.info/api/ -->

    <owl:NamedIndividual rdf:about="https://www.refuges.info/api/"/>
    


    <!-- 
    ///////////////////////////////////////////////////////////////////////////////////////
    //
    // Annotations
    //
    ///////////////////////////////////////////////////////////////////////////////////////
     -->

    <rdf:Description rdf:about="https://intforout.github.io/outdoorPressure#MergedTrack">
        <rdfs:comment xml:lang="en">A merged trace represents the best geometric representation of a set of traces following exactly the same route, defined from an origin point to a destination (Van Damme et al., 2024).</rdfs:comment>
        <rdfs:comment xml:lang="fr">La trace fusionnée est la meilleure représentation géométrique d’un ensemble de traces suivant exactement le même trajet, défini d un point d origine à une destination (Van Damme et al., 2024).</rdfs:comment>
    </rdf:Description>
</rdf:RDF>



<!-- Generated by the OWL API (version 4.5.29.2024-05-13T12:11:03Z) https://github.com/owlcs/owlapi -->

