@prefix : <https://intforout.github.io/outdoorPressure#> .
@prefix owl: <http://www.w3.org/2002/07/owl#> .
@prefix rdf: <http://www.w3.org/1999/02/22-rdf-syntax-ns#> .
@prefix xml: <http://www.w3.org/XML/1998/namespace> .
@prefix xsd: <http://www.w3.org/2001/XMLSchema#> .
@prefix rdfs: <http://www.w3.org/2000/01/rdf-schema#> .
@base <https://intforout.github.io/outdoorPressure#> .

<https://intforout.github.io/outdoorPressure> rdf:type owl:Ontology ;
                                               owl:imports <http://purl.org/www.umr-lastig.fr/geodata> ;
                                               <http://creativecommons.org/ns#licence> <http://creativecommons.org/licenses/by/4.0/> ;
                                               <http://purl.org/dc/elements/1.1/creator> "Bénédicte Bucher" ,
                                                                                         "Marie-Dominique Van Damme" ;
                                               <http://purl.org/dc/elements/1.1/title> "Mountain outdoor pressure KG"@en ;
                                               rdfs:comment "Sets of classes, properties and instances useful to study and mitigate ecological pressure generated by human outdoor activities in mountain"@en ;
                                               rdfs:label "Mountain outdoor pressure knowledge graph"@en .

#################################################################
#    Annotation properties
#################################################################

###  http://creativecommons.org/ns#licence
<http://creativecommons.org/ns#licence> rdf:type owl:AnnotationProperty .


###  http://purl.org/dc/elements/1.1/creator
<http://purl.org/dc/elements/1.1/creator> rdf:type owl:AnnotationProperty .


###  http://purl.org/dc/elements/1.1/description
<http://purl.org/dc/elements/1.1/description> rdf:type owl:AnnotationProperty .


###  http://purl.org/dc/elements/1.1/publisher
<http://purl.org/dc/elements/1.1/publisher> rdf:type owl:AnnotationProperty .


###  http://purl.org/dc/elements/1.1/title
<http://purl.org/dc/elements/1.1/title> rdf:type owl:AnnotationProperty .


###  http://purl.org/dc/terms/bibliographicCitation
<http://purl.org/dc/terms/bibliographicCitation> rdf:type owl:AnnotationProperty .


###  http://purl.org/dc/terms/conformsTo
<http://purl.org/dc/terms/conformsTo> rdf:type owl:AnnotationProperty .


###  http://purl.org/dc/terms/creator
<http://purl.org/dc/terms/creator> rdf:type owl:AnnotationProperty .


###  http://purl.org/dc/terms/hasPart
<http://purl.org/dc/terms/hasPart> rdf:type owl:AnnotationProperty .


###  http://purl.org/dc/terms/identifier
<http://purl.org/dc/terms/identifier> rdf:type owl:AnnotationProperty .


###  http://purl.org/dc/terms/isPartOf
<http://purl.org/dc/terms/isPartOf> rdf:type owl:AnnotationProperty .


###  http://purl.org/dc/terms/issued
<http://purl.org/dc/terms/issued> rdf:type owl:AnnotationProperty .


###  http://purl.org/dc/terms/language
<http://purl.org/dc/terms/language> rdf:type owl:AnnotationProperty .


###  http://purl.org/dc/terms/license
<http://purl.org/dc/terms/license> rdf:type owl:AnnotationProperty .


###  http://purl.org/dc/terms/publisher
<http://purl.org/dc/terms/publisher> rdf:type owl:AnnotationProperty .


###  http://purl.org/dc/terms/spatial
<http://purl.org/dc/terms/spatial> rdf:type owl:AnnotationProperty .


###  http://purl.org/dc/terms/type
<http://purl.org/dc/terms/type> rdf:type owl:AnnotationProperty .


###  http://purl.org/spar/datacite/firstPage
<http://purl.org/spar/datacite/firstPage> rdf:type owl:AnnotationProperty .


###  http://purl.org/spar/datacite/lastPage
<http://purl.org/spar/datacite/lastPage> rdf:type owl:AnnotationProperty .


###  http://purl.org/spar/datacite/number
<http://purl.org/spar/datacite/number> rdf:type owl:AnnotationProperty .


###  http://purl.org/spar/datacite/publicationYear
<http://purl.org/spar/datacite/publicationYear> rdf:type owl:AnnotationProperty .


###  http://purl.org/spar/datacite/relatedIdentifier
<http://purl.org/spar/datacite/relatedIdentifier> rdf:type owl:AnnotationProperty .


###  http://purl.org/spar/datacite/resourceType
<http://purl.org/spar/datacite/resourceType> rdf:type owl:AnnotationProperty .


###  http://purl.org/spar/datacite/subject
<http://purl.org/spar/datacite/subject> rdf:type owl:AnnotationProperty .


###  http://purl.org/spar/datacite/volume
<http://purl.org/spar/datacite/volume> rdf:type owl:AnnotationProperty .


###  http://purl.org/www.umr-lastig.fr/geodata#target
<http://purl.org/www.umr-lastig.fr/geodata#target> rdf:type owl:AnnotationProperty .


###  http://schema.org/address
<http://schema.org/address> rdf:type owl:AnnotationProperty .


###  http://www.w3.org/1999/02/22-rdf-syntax-ns#comment
rdf:comment rdf:type owl:AnnotationProperty .


###  http://www.w3.org/2000/01/rdf-schema#description
rdfs:description rdf:type owl:AnnotationProperty .


###  http://www.w3.org/ns/dcat#accessService
<http://www.w3.org/ns/dcat#accessService> rdf:type owl:AnnotationProperty .


###  http://www.w3.org/ns/dcat#accessURL
<http://www.w3.org/ns/dcat#accessURL> rdf:type owl:AnnotationProperty .


###  http://www.w3.org/ns/dcat#conformsTo
<http://www.w3.org/ns/dcat#conformsTo> rdf:type owl:AnnotationProperty .


###  http://www.w3.org/ns/dcat#dataset
<http://www.w3.org/ns/dcat#dataset> rdf:type owl:AnnotationProperty .


###  http://www.w3.org/ns/dcat#format
<http://www.w3.org/ns/dcat#format> rdf:type owl:AnnotationProperty .


###  http://www.w3.org/ns/dcat#hasPart
<http://www.w3.org/ns/dcat#hasPart> rdf:type owl:AnnotationProperty .


###  http://www.w3.org/ns/dcat#identifier
<http://www.w3.org/ns/dcat#identifier> rdf:type owl:AnnotationProperty .


###  http://www.w3.org/ns/dcat#isPartOf
<http://www.w3.org/ns/dcat#isPartOf> rdf:type owl:AnnotationProperty .


###  http://www.w3.org/ns/dcat#issued
<http://www.w3.org/ns/dcat#issued> rdf:type owl:AnnotationProperty .


###  http://www.w3.org/ns/dcat#keyword
<http://www.w3.org/ns/dcat#keyword> rdf:type owl:AnnotationProperty .


###  http://www.w3.org/ns/dcat#record
<http://www.w3.org/ns/dcat#record> rdf:type owl:AnnotationProperty .


###  http://www.w3.org/ns/dcat#servesDataset
<http://www.w3.org/ns/dcat#servesDataset> rdf:type owl:AnnotationProperty .


###  http://www.w3.org/ns/dcat#service
<http://www.w3.org/ns/dcat#service> rdf:type owl:AnnotationProperty .


###  http://www.w3.org/ns/dcat#theme
<http://www.w3.org/ns/dcat#theme> rdf:type owl:AnnotationProperty .


###  http://www.w3.org/ns/prov#endedAtTime
<http://www.w3.org/ns/prov#endedAtTime> rdf:type owl:AnnotationProperty .


###  http://www.w3.org/ns/prov#generated
<http://www.w3.org/ns/prov#generated> rdf:type owl:AnnotationProperty .


###  http://www.w3.org/ns/prov#quotedAs
<http://www.w3.org/ns/prov#quotedAs> rdf:type owl:AnnotationProperty .


###  http://www.w3.org/ns/prov#startedAtTime
<http://www.w3.org/ns/prov#startedAtTime> rdf:type owl:AnnotationProperty .


###  http://www.w3.org/ns/prov#used
<http://www.w3.org/ns/prov#used> rdf:type owl:AnnotationProperty .


###  http://www.w3.org/ns/prov#wasAssociatedWith
<http://www.w3.org/ns/prov#wasAssociatedWith> rdf:type owl:AnnotationProperty .


###  http://www.w3.org/ns/prov#wasAttributedTo
<http://www.w3.org/ns/prov#wasAttributedTo> rdf:type owl:AnnotationProperty .


###  http://www.w3.org/ns/prov#wasGeneratedBy
<http://www.w3.org/ns/prov#wasGeneratedBy> rdf:type owl:AnnotationProperty .


###  http://www.w3.org/ns/prov#wasInfluencedBy
<http://www.w3.org/ns/prov#wasInfluencedBy> rdf:type owl:AnnotationProperty .


###  http://www.w3.org/ns/prov#wasQuotedFrom
<http://www.w3.org/ns/prov#wasQuotedFrom> rdf:type owl:AnnotationProperty .


###  http://xmlns.com/foaf/0.1/homePage
<http://xmlns.com/foaf/0.1/homePage> rdf:type owl:AnnotationProperty .


###  http://xmlns.com/foaf/0.1/name
<http://xmlns.com/foaf/0.1/name> rdf:type owl:AnnotationProperty .


###  http://xmlns.com/foaf/0.1/primaryTopic
<http://xmlns.com/foaf/0.1/primaryTopic> rdf:type owl:AnnotationProperty .


#################################################################
#    Datatypes
#################################################################

###  http://www.w3.org/2001/XMLSchema#date
xsd:date rdf:type rdfs:Datatype .


###  http://www.w3.org/2001/XMLSchema#gYearMonth
xsd:gYearMonth rdf:type rdfs:Datatype .


###  xsd:date
<xsd:date> rdf:type rdfs:Datatype .


#################################################################
#    Object Properties
#################################################################

###  https://intforout.github.io/outdoorPressure#affords
:affords rdf:type owl:ObjectProperty ;
         rdfs:domain :LandEntity ;
         rdfs:range :Activity ;
         rdfs:comment "Capacity of a place, or land, to support a given activity, effectively or potentially"@en .


###  https://intforout.github.io/outdoorPressure#hasProfile
:hasProfile rdf:type owl:ObjectProperty ;
            rdfs:domain <http://www.w3.org/ns/dcat#Dataset> ;
            rdfs:range <http://purl.org/dc/terms/URI> ;
            rdfs:comment "Profilage de la source -ou du jeu- partagé sous forme d'un document référencé par une URL"@en .


###  https://intforout.github.io/outdoorPressure#locatedIn
:locatedIn rdf:type owl:ObjectProperty ;
           rdfs:domain :Population ;
           rdfs:range :LandEntity .


#################################################################
#    Classes
#################################################################

###  http://purl.org/dc/terms/URI
<http://purl.org/dc/terms/URI> rdf:type owl:Class .


###  https://intforout.github.io/outdoorPressure#Activity
:Activity rdf:type owl:Class ;
          rdfs:comment "Activity of a living creature, different from prov:Activity in the sense that the purpose of the Activity is not to yield an output."@en ;
          rdfs:label "Activity of a living creature"@en .


###  https://intforout.github.io/outdoorPressure#AireCampingCar
:AireCampingCar rdf:type owl:Class ;
                rdfs:subClassOf :LandEntity .


###  https://intforout.github.io/outdoorPressure#AireDeDetente
:AireDeDetente rdf:type owl:Class ;
               rdfs:subClassOf :LandEntity .


###  https://intforout.github.io/outdoorPressure#AireProtegee
:AireProtegee rdf:type owl:Class ;
              rdfs:subClassOf :LandEntity ;
              rdfs:comment "Une aire protégée (AP) (de l'anglais protected area, PA) est, selon la définition de l'Union internationale pour la conservation de la nature (UICN), « un espace géographique clairement défini, reconnu, consacré et géré, par tout moyen efficace, juridique ou autre, afin d'assurer à long terme la conservation de la nature, des services écosystémiques et des valeurs culturelles qui lui sont associés »"@fr ;
              rdfs:label "Aire protégée"@fr .


###  https://intforout.github.io/outdoorPressure#AnimalActivity
:AnimalActivity rdf:type owl:Class ;
                rdfs:subClassOf :Activity .


###  https://intforout.github.io/outdoorPressure#AnimalTrack
:AnimalTrack rdf:type owl:Class ;
             rdfs:subClassOf :Track ;
             rdfs:comment "An animal trace is a digital trace corresponding to the path left by an animal tracked using an interoperable connected device and following a defined data collection protocol."@en ,
                          "La trace animale est une trace numérique correspondant à la trace laissée par un animal suivi au moyen d un dispositif connecté interopérable et selon un protocole de collecte défini."@fr .


###  https://intforout.github.io/outdoorPressure#Cycling
:Cycling rdf:type owl:Class ;
         rdfs:subClassOf :HumanActivity .


###  https://intforout.github.io/outdoorPressure#EncounteringZone
:EncounteringZone rdf:type owl:Class ;
                  rdfs:subClassOf :LandEntity ;
                  rdfs:comment "Area where different activities of different creatures take place, which can potentially imply a conflict of land use rather than harmonious land sharing."@en ;
                  rdfs:label "Encountering zone"@en .


###  https://intforout.github.io/outdoorPressure#FastHiking
:FastHiking rdf:type owl:Class ;
            rdfs:subClassOf :Hiking ;
            rdfs:comment """Le Fast hiking est une randonnée rapide qui se pratique à allure soutenue en toute autonomie sur un parcours présentant du dénivelé et/ou des difficultés techniques.
	        Il s’agit d’une discipline plus sportive et plus dynamique que la randonnée classique."""@fr .


###  https://intforout.github.io/outdoorPressure#FilteredTrack
:FilteredTrack rdf:type owl:Class ;
               rdfs:subClassOf :Track ;
               rdfs:comment "Filtered traces represent a set of unstructured traces assumed to follow the network and used for a specific case study. They result from a user-defined filtering process (spatial, temporal, activity type, etc.)."@en ,
                            "Les traces filtrées représentent un ensemble de traces non structurées, présumées suivre le réseau et utilisées pour un cas d étude spécifique. Elles résultent d un processus de filtrage défini par l utilisateur (spatial, temporel, type d activité, etc.)."@fr .


###  https://intforout.github.io/outdoorPressure#Hiking
:Hiking rdf:type owl:Class ;
        rdfs:subClassOf :HumanActivity ;
        rdfs:comment "activité de plein air consistant à se promener de façon ludique ou sportive"@fr ;
        rdfs:label "Hiking"@en ,
                   "Randonnée pédestre"@fr .


###  https://intforout.github.io/outdoorPressure#HumanActivity
:HumanActivity rdf:type owl:Class ;
               rdfs:subClassOf :Activity ;
               rdfs:comment "Human activity taking place outdoor"@en .


###  https://intforout.github.io/outdoorPressure#HumanTrack
:HumanTrack rdf:type owl:Class ;
            rdfs:subClassOf :Track ;
            rdfs:comment "A human trace is a digital trace corresponding to the path left by a person during outdoor activities using interoperable connected devices (GPS watches, apps, smartphones)."@en ,
                         "La trace humaine est une trace numérique correspondant à la trace laissée par un humain lors d une activité de plein air, à l aide de dispositifs connectés interopérables (montres GPS, applications, smartphones)."@fr .


###  https://intforout.github.io/outdoorPressure#LandEntity
:LandEntity rdf:type owl:Class ;
            rdfs:comment "An entity located in land : an area, a land, a parcel, a footprint, an observation."@en .


###  https://intforout.github.io/outdoorPressure#Landmark
:Landmark rdf:type owl:Class ;
          rdfs:subClassOf :LandEntity .


###  https://intforout.github.io/outdoorPressure#LivingCreature
:LivingCreature rdf:type owl:Class ;
                rdfs:comment "Living creature, animal or human" .


###  https://intforout.github.io/outdoorPressure#MergedAccurateTrack
:MergedAccurateTrack rdf:type owl:Class ;
                     rdfs:subClassOf :MergedTrack ;
                     rdfs:comment "An accurate merged trace is a merged trace that optimizes a quality criterion Q with respect to the ground truth GT (Van Damme et al., 2024)."@en ,
                                  "La trace fusionnée exacte est une trace fusionnée qui optimise un critère de qualité Q par rapport à la vérité terrain VT (Van Damme et al., 2024)."@fr .


###  https://intforout.github.io/outdoorPressure#MergedTrack
:MergedTrack rdf:type owl:Class ;
             rdfs:subClassOf :Track .


###  https://intforout.github.io/outdoorPressure#NamedRoute
:NamedRoute rdf:type owl:Class ;
            rdfs:subClassOf :Route ;
            rdfs:comment """A named route is a known route with a name and a detailed linear geometry, listed in an authoritative or collaborative database (e.g., Visorando). 
	            Example: “Le chemin du Roy”."""@en ,
                         """Un itinéraire nommé est un itinéraire connu ayant un titre et une géométrie linéraire détaillée,  répertorié dans une base de données d autorité ou collaborative (par ex. Visorando). 
	            Exemple : « Le chemin du Roy »."""@fr .


###  https://intforout.github.io/outdoorPressure#Observation
:Observation rdf:type owl:Class ;
             rdfs:subClassOf :Activity ;
             rdfs:comment """An observation is an act associated with a discrete time instant or period through which a number, term or
	other symbol is assigned to a phenomenon.""" ;
             rdfs:label "Observation or SurveyProcess" .


###  https://intforout.github.io/outdoorPressure#PlandEau
:PlandEau rdf:type owl:Class ;
          rdfs:subClassOf :LandEntity .


###  https://intforout.github.io/outdoorPressure#Population
:Population rdf:type owl:Class ;
            rdfs:comment "Ensemble of individuals of a species in an land entity."@en ;
            rdfs:seeAlso "http://www.wikidata.org/entity/Q2625603" .


###  https://intforout.github.io/outdoorPressure#PopulationFootprint
:PopulationFootprint rdf:type owl:Class ;
                     rdfs:subClassOf :LandEntity .


###  https://intforout.github.io/outdoorPressure#ReservesNaturelles
:ReservesNaturelles rdf:type owl:Class ;
                    rdfs:subClassOf :LandEntity ;
                    rdfs:comment "Zone naturelle sensible où l'environnement est vulnérable à certaines activités humaines. Créé en 2018 et imaginé par la Ligue de Protection des Oiseaux Isère, introduit dans les api des services des parcs régionaux et nationaux. Ce concept permet d'introduire les zones réglementaires et les zones sensibles, de renseigner les zones d’arrêtés de protection du biotope : emplacement, période de régulation, description associée, espèce, typologie de pratique, etc.." ;
                    rdfs:label "Réserves naturelles" .


###  https://intforout.github.io/outdoorPressure#ResilientRoute
:ResilientRoute rdf:type owl:Class ;
                rdfs:subClassOf :Route ;
                rdfs:comment "A resilient itinerary is a route that minimizes its environmental impact, exerting no pressure on wildlife or vegetation."@en ,
                             "Un itinéraire résilient est un itinéraire qui n exerce pas de pression sur la faune et la flore."@fr .


###  https://intforout.github.io/outdoorPressure#Route
:Route rdf:type owl:Class ;
       rdfs:subClassOf :LandEntity ;
       rdfs:comment "A route represents a path to follow, which may rely (or not) on a physical support such as a road network (Teulade-Denantes et al., 2015). It is characterized by an origin, a destination, a set of waypoints, and a descriptive element."@en ,
                    "Un itinéraire représente un trajet à suivre qui s appuie (ou non) sur un support physique défini par un réseau routier (Teulade-Denantes et al., 2015). Il est caractérisé par une origine, une destination, un ensemble de points de passage et une description."@fr .


###  https://intforout.github.io/outdoorPressure#SensitiveArea
:SensitiveArea rdf:type owl:Class ;
               rdfs:subClassOf :LandEntity ;
               rdfs:comment "Zone naturelle sensible où l'environnement est vulnérable à certaines activités humaines. Créé en 2018 et imaginé par la Ligue de Protection des Oiseaux Isère, introduit dans les api des services des parcs régionaux et nationaux. Ce concept permet d'introduire les zones réglementaires et les zones sensibles, de renseigner les zones d’arrêtés de protection du biotope : emplacement, période de régulation, description associée, espèce, typologie de pratique, etc.." .


###  https://intforout.github.io/outdoorPressure#Sentier
:Sentier rdf:type owl:Class ;
         rdfs:subClassOf :LandEntity .


###  https://intforout.github.io/outdoorPressure#Track
:Track rdf:type owl:Class ;
       rdfs:comment "A track is defined as an ordered set of points, each characterized by a position (x, y) and a timestamp (Van Damme et al., 2024)."@en ,
                    "La trace est définie par un ensemble de points ordonnés, chaque point étant caractérisé par une position (x, y) et un temps (timestamp) (Van Damme et al., 2024). C'est un résultat d'une procédure : soit d'une Observation par un Sensor, capteur gps porté par un objet mobile (Platform), soit d'un retraitement d'une trace brute, soit d'une simulation."@fr .


###  https://intforout.github.io/outdoorPressure#Trajectory
:Trajectory rdf:type owl:Class ;
            rdfs:subClassOf :LandEntity .


#################################################################
#    Individuals
#################################################################

###  http://purl.org/www.umr-lastig.fr/geodata#BD_TOPO_V3
<http://purl.org/www.umr-lastig.fr/geodata#BD_TOPO_V3> rdf:type owl:NamedIndividual ,
                                                                <http://www.w3.org/ns/dcat#DatasetSeries> ;
                                                       <http://schema.org/alternateName> "BD TOPO® description vectorielle 3D (" ;
                                                       <http://schema.org/creator> <http://njh.me/contact.geoservices@ign.fr> ;
                                                       <http://schema.org/dateCreated> "2002-12-15"^^<http://schema.org/Date> ;
                                                       <http://schema.org/datePublished> "2025-06-15"^^<http://schema.org/Date> ;
                                                       <http://schema.org/description> """La BD TOPO® version 3.5 contient une description vectorielle 3D (structurée en objets) des éléments du territoire et de ses infrastructures, de précision métrique.

	    Les objets de la BD TOPO® sont structurés en thèmes : 
	     - l'administratif ; 
	     - le bâti ; 
	     - l'hydrographie ; 
	     - les lieux nommés ; 
	     - l'occupation du sol ; 
	     - les services et activités ; 
	     - le transport ; 
	     - les zones réglementées. 

	    Le processus de production 3D permet de fournir l'altimétrie des objets, ainsi que la hauteur des bâtiments. 

	    Le relief est décrit sous forme de modèles numériques de terrain (MNT). 

	    Depuis la version 3.0, tous les objets possèdent un identifiant unique et stable dans le temps.

	    Le produit **BDTOPO® Express** est l’édition hebdomadaire de la BDTOPO® si vous avez besoin de travailler sur de la donnée topographique à haute fréquence (disponible depuis mai 2025). 

	    Le produit **Différentiel BD TOPO®** contient les différences géométriques et sémantiques sur l'ensemble du contenu BD TOPO® entre deux éditions trimestrielles successives BD TOPO®. 

	    Plus précisément, l'édition N du Différentiel BD TOPO® en vigueur contient tout objet de la BD TOPO® dont la date de modification, la date de création ou la date de suppression en base est postérieure à la date de prédiffusion de la précédente édition trimestrielle (N-1), équivalent à une activité de mise à jour par l'IGN d'une durée de 3 mois.""" ;
                                                       <http://schema.org/encodingFormat> "GPKG" ,
                                                                                          "PostGreSQL" ,
                                                                                          "SHP" ,
                                                                                          "TMS" ,
                                                                                          "WFS" ,
                                                                                          "WMS" ,
                                                                                          "WMTS" ;
                                                       <http://schema.org/keywords> "Altitude" ,
                                                                                    "Bâtiments" ,
                                                                                    "Dénominations géographiques" ,
                                                                                    "Hydrographie" ,
                                                                                    "Mobilité" ,
                                                                                    "Réseaux de transport" ,
                                                                                    "activités" ,
                                                                                    "données ouvertes" ,
                                                                                    "eau" ,
                                                                                    "forêts" ,
                                                                                    "haies" ,
                                                                                    "routes" ,
                                                                                    "toponymie" ,
                                                                                    "transports" ,
                                                                                    "végétation" ;
                                                       <http://schema.org/name> "BD TOPO®" ;
                                                       rdfs:comment "BD TOPO covers whole French territory, is captured at scale 1/ 10 000, exists since 1990 and aims to provide reference data for mapping and spatial analysis."@en ;
                                                       rdfs:label "BD TOPO® V3."@en ;
                                                       <http://www.w3.org/ns/dcat#language> "fr-FR" ;
                                                       <http://www.w3.org/ns/dcat#title> "BD TOPO® V3. La BD TOPO® permet de couvrir de manière cohérente l'ensemble des entités géographiques et administratives du territoire national. La BD TOPO® fournit une information de référence à tous les acteurs de la gestion, de l'aménagement et de l'observation du territoire pour analyser, situer, représenter des données dans leur réalité géographique"@fr .


###  http://purl.org/www.umr-lastig.fr/geodata#CameraTrapSurveyCMB20242025
<http://purl.org/www.umr-lastig.fr/geodata#CameraTrapSurveyCMB20242025> rdf:type owl:NamedIndividual ,
                                                                                 :Observation ;
                                                                        <http://www.w3.org/ns/prov#generated> :EcoCompteurCMBDataset ;
                                                                        <http://www.w3.org/ns/prov#used> <ttp://purl.org/www.umr-lastig.fr/geodata#PyroEvo> ;
                                                                        rdfs:comment "Including the locations of each eco-counter."@en ;
                                                                        rdfs:label "Camera trap survey from Chamonix Community of Communes in 2024-2025."@en ;
                                                                        <http://www.w3.org/ns/prov#endedAtTime> "2024-02"^^xsd:gYearMonth ;
                                                                        <http://www.w3.org/ns/prov#startedAtTime> "2025-11"^^xsd:gYearMonth .


###  http://purl.org/www.umr-lastig.fr/geodata#mgarel
<http://purl.org/www.umr-lastig.fr/geodata#mgarel> rdf:type owl:NamedIndividual .


###  http://purl.org/www.umr-lastig.fr/geodata#pmarchand
<http://purl.org/www.umr-lastig.fr/geodata#pmarchand> rdf:type owl:NamedIndividual .


###  https://api.camptocamp.org/
<https://api.camptocamp.org/> rdf:type owl:NamedIndividual .


###  https://entrepot.recherche.data.gouv.fr/file.xhtml?persistentId=doi:10.57745/NSMUWN&version=1.0
<https://entrepot.recherche.data.gouv.fr/file.xhtml?persistentId=doi:10.57745/NSMUWN&version=1.0> rdf:type owl:NamedIndividual .


###  https://entrepot.recherche.data.gouv.fr/file.xhtml?persistentId=doi:10.57745/P0PXVN&version=1.0
<https://entrepot.recherche.data.gouv.fr/file.xhtml?persistentId=doi:10.57745/P0PXVN&version=1.0> rdf:type owl:NamedIndividual .


###  https://entrepot.recherche.data.gouv.fr/file.xhtml?persistentId=doi:10.57745/Q6OT0J&version=1.0
<https://entrepot.recherche.data.gouv.fr/file.xhtml?persistentId=doi:10.57745/Q6OT0J&version=1.0> rdf:type owl:NamedIndividual .


###  https://entrepot.recherche.data.gouv.fr/file.xhtml?persistentId=doi:10.57745/TRYLX1&version=1.0
<https://entrepot.recherche.data.gouv.fr/file.xhtml?persistentId=doi:10.57745/TRYLX1&version=1.0> rdf:type owl:NamedIndividual .


###  https://geotrek.parcdesbauges.com/api/v2/
<https://geotrek.parcdesbauges.com/api/v2/> rdf:type owl:NamedIndividual .


###  https://intforout.github.io/outdoorPressure#AltitudeRandoRoutesBauges2025
:AltitudeRandoRoutesBauges2025 rdf:type owl:NamedIndividual ,
                                        <http://www.w3.org/ns/dcat#Dataset> ;
                               <http://purl.org/dc/terms/issued> "2025-05-01"^^xsd:date ;
                               <http://purl.org/dc/terms/language> "fr-FR" ;
                               <http://purl.org/dc/terms/license> <https://opendatacommons.org/licenses/odbl/> ;
                               <http://purl.org/dc/terms/publisher> :altituderando ;
                               rdfs:comment "A set of routes issued from altituderando.com in 2025 in the Bauges area."@en ;
                               rdfs:label "AltitudeRando Hiking Routes in the Bauges Massif (2025)"@en .


###  https://intforout.github.io/outdoorPressure#BDTOPOSentiersBauges2025
:BDTOPOSentiersBauges2025 rdf:type owl:NamedIndividual ,
                                   <http://www.w3.org/ns/dcat#Dataset> ;
                          <http://purl.org/www.umr-lastig.fr/geodata#represents> :SentierDesBauges ;
                          <http://www.w3.org/ns/dcat#inSeries> <http://purl.org/www.umr-lastig.fr/geodata#BD_TOPO_V3> ;
                          rdfs:comment "Classe=Tronçon de route, Nature=Sentier"@fr ,
                                       "This dataset is extracted from the BDTOPO database, under the Transportation theme, from the Road Segment feature class, applying a filter on the “nature” attribute corresponding to the value “trail”."@en ;
                          rdfs:label "Trails from the BDTOPO dataset in the Bauges Massif (2025 edition)"@en .


###  https://intforout.github.io/outdoorPressure#BoisVincennes
:BoisVincennes rdf:type owl:NamedIndividual ,
                        <http://purl.org/dc/terms/Location> ;
               rdfs:label "Test area located in the Bois de Vincennes"@en ,
                          "Zone de test dans le Bois de Vincennes"@fr .


###  https://intforout.github.io/outdoorPressure#CamptocampPoisBauges2025
:CamptocampPoisBauges2025 rdf:type owl:NamedIndividual ,
                                   <http://www.w3.org/ns/dcat#Dataset> ;
                          <http://www.w3.org/ns/dcat#distribution> :c2c-waypoint-geojson ;
                          <http://purl.org/dc/terms/issued> "2025-05-01"^^xsd:date ;
                          <http://purl.org/dc/terms/language> "fr-FR" ;
                          <http://purl.org/dc/terms/license> <https://opendatacommons.org/licenses/odbl/> ;
                          <http://purl.org/dc/terms/publisher> :camptocamp ;
                          rdfs:comment "A set of Waypoints issued from Camptocamp.org API."@en ;
                          rdfs:label "Camptocamp.org-waypoints"@en .


###  https://intforout.github.io/outdoorPressure#CamptocampRoutesBauges2025
:CamptocampRoutesBauges2025 rdf:type owl:NamedIndividual ,
                                     <http://www.w3.org/ns/dcat#Dataset> ;
                            <http://www.w3.org/ns/dcat#distribution> :c2c-route-geojson ;
                            <http://purl.org/dc/terms/issued> "2025-05-01"^^xsd:date ;
                            <http://purl.org/dc/terms/language> "fr-FR" ;
                            <http://purl.org/dc/terms/license> <https://opendatacommons.org/licenses/odbl/> ;
                            <http://purl.org/dc/terms/publisher> :camptocamp ;
                            rdfs:comment "A set of Routes issued from Camptocamp.org API."@en ;
                            rdfs:label "Camptocamp.org-routes"@en .


###  https://intforout.github.io/outdoorPressure#DeepFaune
:DeepFaune rdf:type owl:NamedIndividual ,
                    <http://www.w3.org/ns/prov#SoftwareAgent> ;
           <http://purl.org/dc/terms/identifier> "DeepFaune" ;
           rdfs:label "DeepFaune"@en .


###  https://intforout.github.io/outdoorPressure#EcoCompteurCMBDataset
:EcoCompteurCMBDataset rdf:type owl:NamedIndividual ,
                                <http://www.w3.org/ns/dcat#Dataset> ;
                       rdfs:comment "12 éco-compteurs (issus de conventions avec CD et Communauté de Communes de la Vallée de Chamonix-Mont-Blanc (CCVCMB) avec les localisations de chaque éco-compteur. Ces éco-compteurs sont tous des Pyro-Evo"@fr ,
                                    "This dataset includes 12 eco-counters (implemented through agreements with the Departmental Council and the Chamonix-Mont-Blanc Valley Community of Communes (CCVCMB)), together with the geographic location of each device. All counters are Pyro-Evo units."@en ;
                       rdfs:label "Dataset derived from 12 CCVCMB eco-counters."@en .


###  https://intforout.github.io/outdoorPressure#EcoCompteurUTMBDataset
:EcoCompteurUTMBDataset rdf:type owl:NamedIndividual ,
                                 <http://www.w3.org/ns/dcat#Dataset> ;
                        rdfs:comment "10 éco-compteurs UTMB (avec des propriétaires différents), utilisables uniquement par le GT représentativité du WP2 dans un premier temps. Sinon pas d'autorisation. Certains de ces éco-compteurs sont uniquement piétons, d’autres distinguent piétons / cyclistes / voitures."@fr ,
                                     "This dataset comprises 10 UTMB eco-counters (with different ownership). They are initially accessible solely to the WP2 Representativeness Working Group; no additional authorization is granted. Some counters record pedestrian traffic only, while others distinguish between pedestrians, cyclists, and motor vehicles."@en ;
                        rdfs:label "Dataset derived from 12 UTMB eco-counters."@en .


###  https://intforout.github.io/outdoorPressure#EntrepotRechercheIntForOut
:EntrepotRechercheIntForOut rdf:type owl:NamedIndividual ,
                                     <http://www.w3.org/ns/dcat#Catalog> ;
                            <http://www.w3.org/ns/dcat#dataset> :MOUSLS ,
                                                                :MOUSLSGroundTruthDenseForestPath ,
                                                                :MOUSLSTracksMultiSensorsVincennesForest ;
                            <http://www.w3.org/ns/dcat#record> :MetadataGroundTruthPathVincennesForest ,
                                                               :MetadataTracksMultiSensorsVincennesForest ;
                            rdfs:comment "Dataverse dedicated to the IntForOut project. This catalog is integrated into the multidisciplinary Recherche Data Gouv data warehouse platform."@en ,
                                         "Dataverse dédié au projet IntForOut. Ce catalogue est intégré dans la plateforme de l'entrepôt pluridisciplinaire Recherche Data Gouv."@fr ;
                            rdfs:label "Dataverse dedicated to the IntForOut project"@en ;
                            <http://xmlns.com/foaf/0.1/homePage> "https://entrepot.recherche.data.gouv.fr/dataverse/intforout" .


###  https://intforout.github.io/outdoorPressure#GroundTruthDenseForestPath-csv
:GroundTruthDenseForestPath-csv rdf:type owl:NamedIndividual ,
                                         <http://www.w3.org/ns/dcat#Distribution> ;
                                <http://www.w3.org/ns/dcat#accessURL> <https://entrepot.recherche.data.gouv.fr/file.xhtml?persistentId=doi:10.57745/P0PXVN&version=1.0> ;
                                <http://www.w3.org/ns/dcat#format> "csv" ;
                                <http://www.w3.org/ns/dcat#identifier> "ground_truth_dense_forest_path.txt" .


###  https://intforout.github.io/outdoorPressure#HikersFootprintBoisVincennes
:HikersFootprintBoisVincennes rdf:type owl:NamedIndividual ,
                                       :PopulationFootprint ;
                              :affords :HikingInBoisdeVincennes .


###  https://intforout.github.io/outdoorPressure#HikingInBoisdeVincennes
:HikingInBoisdeVincennes rdf:type owl:NamedIndividual ,
                                  :Hiking .


###  https://intforout.github.io/outdoorPressure#HikingInLesBauges
:HikingInLesBauges rdf:type owl:NamedIndividual ,
                            :Hiking .


###  https://intforout.github.io/outdoorPressure#HumanChamoisRealEncounters
:HumanChamoisRealEncounters rdf:type owl:NamedIndividual ,
                                     <http://www.w3.org/ns/dcat#Dataset> ;
                            <http://www.w3.org/ns/dcat#distribution> :HumanChamoisRealEncounters-csv ;
                            <http://www.w3.org/ns/prov#wasAttributedTo> <http://purl.org/www.umr-lastig.fr/geodata#jadawson> ;
                            <http://purl.org/dc/terms/issued> "2025-04-25"^^xsd:date ;
                            <http://purl.org/dc/terms/language> "English" ;
                            <http://purl.org/dc/terms/license> "Licence Ouverte v2.0 (Etalab)" ;
                            <http://purl.org/dc/terms/publisher> <http://purl.org/www.umr-lastig.fr/geodata#LASTIG> ;
                            rdfs:comment "185 real encounters. The geometries are saved as WKT. Only included real encounters as they are likely enough to work with and potential encounters drastically increase amount of data, also they may need some explanation for why they have 2 different dates"@en .


###  https://intforout.github.io/outdoorPressure#HumanChamoisRealEncounters-csv
:HumanChamoisRealEncounters-csv rdf:type owl:NamedIndividual ,
                                         <http://www.w3.org/ns/dcat#Distribution> ;
                                <http://www.w3.org/ns/dcat#format> "csv" ;
                                <http://www.w3.org/ns/dcat#identifier> "human_chamois_real_encounters.csv" .


###  https://intforout.github.io/outdoorPressure#HumanOutdoorActivitiesBauges2014
:HumanOutdoorActivitiesBauges2014 rdf:type owl:NamedIndividual ,
                                           :HumanActivity .


###  https://intforout.github.io/outdoorPressure#HumanOutdoorActivitiesBauges2024
:HumanOutdoorActivitiesBauges2024 rdf:type owl:NamedIndividual ,
                                           :HumanActivity .


###  https://intforout.github.io/outdoorPressure#HumanOutdoorActivitiesBoisVincennes2022
:HumanOutdoorActivitiesBoisVincennes2022 rdf:type owl:NamedIndividual ,
                                                  :HumanActivity .


###  https://intforout.github.io/outdoorPressure#HumanOutdoorActivitiesMontBlanc2024
:HumanOutdoorActivitiesMontBlanc2024 rdf:type owl:NamedIndividual ,
                                              :HumanActivity .


###  https://intforout.github.io/outdoorPressure#IntForOutDB
:IntForOutDB rdf:type owl:NamedIndividual ,
                      <http://purl.org/www.umr-lastig.fr/geodata#DataWarehouse> ;
             <http://purl.org/dc/terms/language> "English" ;
             <http://purl.org/dc/terms/publisher> <http://purl.org/www.umr-lastig.fr/geodata#LIFAT> ;
             rdfs:comment "Dataset associated with IntForOut ETL framework" ;
             rdfs:label "Dataset associated with IntForOut ETL framework"@en .


###  https://intforout.github.io/outdoorPressure#JournalOfOutdoorRecreationAndTourismKerouantonEtAl2024
:JournalOfOutdoorRecreationAndTourismKerouantonEtAl2024 rdf:type owl:NamedIndividual ,
                                                                 <http://purl.org/www.umr-lastig.fr/geodata#ScientificPaper> ;
                                                        <http://purl.org/dc/terms/creator> <http://purl.org/www.umr-lastig.fr/geodata#ljolivet> ,
                                                                                           :aloison ,
                                                                                           _:genid1 ,
                                                                                           _:genid2 ;
                                                        <http://purl.org/dc/terms/publisher> "Journal of Outdoor Recreation and Tourism" ;
                                                        <http://purl.org/spar/datacite/firstPage> "100734" ;
                                                        <http://purl.org/spar/datacite/publicationYear> "2024" ;
                                                        <http://purl.org/spar/datacite/relatedIdentifier> "10.1016/j.jort.2024.100734" ,
                                                                                                          "https://doi.org/10.1016/j.jort.2024.100734" ;
                                                        <http://purl.org/spar/datacite/resourceType> <http://purl.org/spar/datacite/Journal> ;
                                                        <http://purl.org/spar/datacite/subject> "Outdoor recreation" ,
                                                                                                "Pauses" ,
                                                                                                "ST-DBSCAN" ,
                                                                                                "Spatio-temporal pattern" ,
                                                                                                "Time-geography" ,
                                                                                                "global navigation satellite system" ;
                                                        rdfs:label "Eye-catching or breath-catching: Role and landscape attributes of pauses differs among hikers’ profile when rambling in a French mountainous area"@en ;
                                                        <http://www.w3.org/ns/prov#quotedAs> :KerouantonSurvey20142015 ,
                                                                                             :KerouantonTrack20142015 .

_:genid1 rdf:type <http://www.w3.org/ns/prov#Person> ;
          <http://xmlns.com/foaf/0.1/name> "Colin Kerouanton" .

_:genid2 rdf:type <http://www.w3.org/ns/prov#Person> ;
          <http://xmlns.com/foaf/0.1/name> "Clémence Perrin-Malterre" .


###  https://intforout.github.io/outdoorPressure#JournalOfPeopleAndNatureMarchandEtAl2025
:JournalOfPeopleAndNatureMarchandEtAl2025 rdf:type owl:NamedIndividual ,
                                                   <http://purl.org/www.umr-lastig.fr/geodata#ScientificPaper> ;
                                          <http://purl.org/dc/terms/creator> :mgarel ,
                                                                             :pmarchand ,
                                                                             _:genid3 ,
                                                                             _:genid4 ;
                                          <http://purl.org/dc/terms/isPartOf> "Journal of People and Nature" ;
                                          <http://purl.org/spar/datacite/firstPage> "3002" ;
                                          <http://purl.org/spar/datacite/lastPage> "3016" ;
                                          <http://purl.org/spar/datacite/number> "11" ;
                                          <http://purl.org/spar/datacite/publicationYear> "2025" ;
                                          <http://purl.org/spar/datacite/relatedIdentifier> "10.1002/pan3.70151" ,
                                                                                            "https://besjournals.onlinelibrary.wiley.com/doi/abs/10.1002/pan3.70151" ;
                                          <http://purl.org/spar/datacite/resourceType> <http://purl.org/spar/datacite/Journal> ;
                                          <http://purl.org/spar/datacite/subject> "activity" ,
                                                                                  "behaviour" ,
                                                                                  "cycling races" ,
                                                                                  "disturbance" ,
                                                                                  "movements" ,
                                                                                  "recreational ecology" ,
                                                                                  "trail running" ;
                                          <http://purl.org/spar/datacite/volume> "7" ;
                                          rdfs:label "Disturbance by massive sporting events in mountain areas: When and where matters for the protected Alpine ibex Capra ibex"@en ;
                                          <http://www.w3.org/ns/prov#quotedAs> :MarchandEtAl2025MSEPeopleNatureDataZenodo .

_:genid3 rdf:type <http://www.w3.org/ns/prov#Person> ;
          <http://xmlns.com/foaf/0.1/name> "Nolwenn Risser" .

_:genid4 rdf:type <http://www.w3.org/ns/prov#Person> ;
          <http://xmlns.com/foaf/0.1/name> "Elodie Petit" .


###  https://intforout.github.io/outdoorPressure#KerouantonQuestionnaire20142015
:KerouantonQuestionnaire20142015 rdf:type owl:NamedIndividual ,
                                          <http://www.w3.org/ns/dcat#Dataset> ;
                                 <http://www.w3.org/ns/dcat#inSeries> :KerouantonSurveyFieldCampaignTracksGNSS20142015 ;
                                 <http://www.w3.org/ns/prov#wasQuotedFrom> :JournalOfOutdoorRecreationAndTourismKerouantonEtAl2024 ;
                                 rdfs:comment "A set of answers issued from a questionnaire. Compleed with tracks"@en ;
                                 rdfs:label "Tracks issued from PhD of Colin Kerouanton"@en .


###  https://intforout.github.io/outdoorPressure#KerouantonSurvey20142015
:KerouantonSurvey20142015 rdf:type owl:NamedIndividual ,
                                   :Observation ;
                          <http://www.w3.org/ns/prov#generated> :KerouantonSurveyFieldCampaignTracksGNSS20142015 ;
                          <http://www.w3.org/ns/prov#endedAtTime> "2014-01"^^xsd:gYearMonth ;
                          <http://www.w3.org/ns/prov#startedAtTime> "2015-12"^^xsd:gYearMonth .


###  https://intforout.github.io/outdoorPressure#KerouantonSurveyFieldCampaignTracksGNSS20142015
:KerouantonSurveyFieldCampaignTracksGNSS20142015 rdf:type owl:NamedIndividual ,
                                                          <http://www.w3.org/ns/dcat#DatasetSeries> ;
                                                 <http://www.w3.org/ns/prov#wasQuotedFrom> :JournalOfOutdoorRecreationAndTourismKerouantonEtAl2024 ;
                                                 <http://purl.org/dc/terms/issued> "2015-08-31"^^xsd:date ;
                                                 <http://purl.org/dc/terms/language> "French" ;
                                                 <http://purl.org/dc/terms/publisher> "LECA et l’EDYTEM" ;
                                                 <http://purl.org/dc/terms/spatial> :PNRDesBauges ;
                                                 rdfs:comment "Questionnaires de campagnes de terrain ciblant la pratique de la randonnée dans le PNR du Massif des Bauges accompagnés de traces GNSS"@fr ;
                                                 rdfs:label "Questionnaires de campagnes de terrain complétés par des traces GNSS"@fr .


###  https://intforout.github.io/outdoorPressure#KerouantonTrack20142015
:KerouantonTrack20142015 rdf:type owl:NamedIndividual ,
                                  <http://www.w3.org/ns/dcat#Dataset> ;
                         <http://www.w3.org/ns/dcat#inSeries> :KerouantonSurveyFieldCampaignTracksGNSS20142015 ;
                         <http://www.w3.org/ns/prov#wasQuotedFrom> :JournalOfOutdoorRecreationAndTourismKerouantonEtAl2024 ;
                         rdfs:comment "A set of tracks. Compleed with questionnaires"@en ;
                         rdfs:label "Tracks issued from PhD of Colin Kerouanton"@en .


###  https://intforout.github.io/outdoorPressure#LIFAT
:LIFAT rdf:type owl:NamedIndividual ,
                <http://www.w3.org/ns/prov#Organization> ;
       <http://xmlns.com/foaf/0.1/name> "Laboratoire d'Informatique Fondamentale et Appliquée de Tours (LIFAT)" .


###  https://intforout.github.io/outdoorPressure#MOUSLS
:MOUSLS rdf:type owl:NamedIndividual ,
                 <http://www.w3.org/ns/dcat#DatasetSeries> ;
        <http://www.w3.org/ns/prov#wasAttributedTo> <http://purl.org/www.umr-lastig.fr/geodata#amraimond> ,
                                                    <http://purl.org/www.umr-lastig.fr/geodata#ymeneroux> ;
        <http://www.w3.org/ns/prov#wasQuotedFrom> :SIGSPATIAL24VanDammeEtAl2024 ;
        <http://purl.org/dc/terms/bibliographicCitation> "Raimond, Ana-Maria; Meneroux, Yann; Calloch, Paul; Labbé, Brice; Peseux, Lorine; Tertre, Franck; Clédat, Emmanuel, 2025, \"Multi-sensors and Ground Truth Tracks\", https://doi.org/10.57745/MOUSLS, Recherche Data Gouv, V1" ;
        <http://purl.org/dc/terms/issued> "2025-01-18"^^xsd:date ;
        <http://purl.org/dc/terms/language> "English" ;
        <http://purl.org/dc/terms/license> "Licence Ouverte v2.0 (Etalab)" ;
        <http://purl.org/dc/terms/publisher> <http://purl.org/www.umr-lastig.fr/geodata#LASTIG> ;
        <http://purl.org/dc/terms/spatial> :BoisVincennes ;
        <http://purl.org/spar/datacite/relatedIdentifier> "https://doi.org/10.57745/MOUSLS" ;
        rdfs:comment "The goal of this dataset is to provide in-situ ground truth data to validate an algorithm for fusing GNSS tracks. This is a dataset series composed by two linked datasets. The first was (file tracks_multi_sensors_vincennes_forest.gpkg) contains GNSS tracks and was collected by two researchers using a strict data collection protocol, following the same path at times precisely and at other times with slight deviations. The second (file ground_truth_dense_forest_path.txt) was collected by a group of students and represents ground truth data for the same path in dense forest. English (2025)"@en ;
        rdfs:label "MOUSLS: Multi-sensors and Ground Truth Tracks in Vincennes (2025)"@en .


###  https://intforout.github.io/outdoorPressure#MOUSLSGroundTruthDenseForestPath
:MOUSLSGroundTruthDenseForestPath rdf:type owl:NamedIndividual ,
                                           <http://www.w3.org/ns/dcat#Dataset> ;
                                  <http://www.w3.org/ns/dcat#distribution> :GroundTruthDenseForestPath-csv ;
                                  <http://www.w3.org/ns/dcat#inSeries> :MOUSLS ;
                                  rdfs:comment "This dataset was collected on-site by a group of students using a defined methodology. It contains precise station locations along a real-world path through dense forest, after reordering in the south–north direction of travel. The goal of these reference data is to obtain a very precise ground truth in order to assess the accuracy of GNSS tracks produced by following exactly the same path with five sensors: a Garmin watch, a Polar watch, the Visorando mobile application, a Keymaza GPS, and a Ublox GPS."@en .


###  https://intforout.github.io/outdoorPressure#MOUSLSTracksMultiSensorsVincennesForest
:MOUSLSTracksMultiSensorsVincennesForest rdf:type owl:NamedIndividual ,
                                                  <http://www.w3.org/ns/dcat#Dataset> ;
                                         <http://purl.org/www.umr-lastig.fr/geodata#represents> :HumanOutdoorActivitiesBoisVincennes2022 ;
                                         <http://www.w3.org/ns/dcat#distribution> :TracksMultiSensorsVincennesForest-gpkg ;
                                         <http://www.w3.org/ns/dcat#inSeries> :MOUSLS ;
                                         rdfs:comment "This dataset was collected by two researchers by following the data colection protocol and using five sensors Garmin watch, Polar watch, Visorando mobile phone application, Keymaza GPS, Ublox GPS. The study area covers dense forect in Vincennes forest (Paris)."@en .


###  https://intforout.github.io/outdoorPressure#MarchandEtAl2025MSEPeopleNatureDataActExport
:MarchandEtAl2025MSEPeopleNatureDataActExport rdf:type owl:NamedIndividual ,
                                                       <http://www.w3.org/ns/dcat#Dataset> ;
                                              <http://www.w3.org/ns/dcat#distribution> :marchandetal-rdata ;
                                              <http://www.w3.org/ns/dcat#inSeries> :MarchandEtAl2025MSEPeopleNatureDataZenodo ;
                                              <http://purl.org/dc/terms/issued> "2025-09-04"^^xsd:date ;
                                              <http://purl.org/dc/terms/language> "English" ;
                                              <http://purl.org/dc/terms/license> <https://creativecommons.org/licenses/by/4.0/> ;
                                              <http://purl.org/dc/terms/publisher> "Office Français de la Biodiversité" ;
                                              rdfs:comment "Activity data from gps collars"@en ;
                                              rdfs:label "act-export"@fr .


###  https://intforout.github.io/outdoorPressure#MarchandEtAl2025MSEPeopleNatureDataLocsExport
:MarchandEtAl2025MSEPeopleNatureDataLocsExport rdf:type owl:NamedIndividual ,
                                                        <http://www.w3.org/ns/dcat#Dataset> ;
                                               <http://www.w3.org/ns/dcat#distribution> :marchandetal-rdata ;
                                               <http://www.w3.org/ns/dcat#inSeries> :MarchandEtAl2025MSEPeopleNatureDataZenodo ;
                                               <http://purl.org/dc/terms/issued> "2025-09-04"^^xsd:date ;
                                               <http://purl.org/dc/terms/language> "English" ;
                                               <http://purl.org/dc/terms/license> <https://creativecommons.org/licenses/by/4.0/> ;
                                               <http://purl.org/dc/terms/publisher> "Office Français de la Biodiversité" ;
                                               rdfs:comment "GPS locations"@en ;
                                               rdfs:label "locs-export"@fr .


###  https://intforout.github.io/outdoorPressure#MarchandEtAl2025MSEPeopleNatureDataZenodo
:MarchandEtAl2025MSEPeopleNatureDataZenodo rdf:type owl:NamedIndividual ,
                                                    <http://www.w3.org/ns/dcat#DatasetSeries> ;
                                           <http://www.w3.org/ns/dcat#distribution> :marchandetal-rdata ;
                                           <http://www.w3.org/ns/prov#wasAttributedTo> <http://purl.org/www.umr-lastig.fr/geodata#mgarel> ,
                                                                                       <http://purl.org/www.umr-lastig.fr/geodata#pmarchand> ;
                                           <http://www.w3.org/ns/prov#wasQuotedFrom> :JournalOfPeopleAndNatureMarchandEtAl2025 ;
                                           <http://purl.org/dc/terms/bibliographicCitation> "Marchand, P., Risser, N., Petit, E. & Garel, M. (2025). Data from: Disturbance by massive sporting events in mountain areas: when and where matters for the protected Alpine ibex Capra ibex [Data set]. Zenodo. https://doi.org/10.5281/zenodo.17052197" ;
                                           <http://purl.org/dc/terms/issued> "2025-09-04"^^xsd:date ;
                                           <http://purl.org/dc/terms/language> "English" ;
                                           <http://purl.org/dc/terms/license> <https://creativecommons.org/licenses/by/4.0/> ;
                                           <http://purl.org/dc/terms/publisher> "Office Français de la Biodiversité" ;
                                           <http://purl.org/dc/terms/spatial> :RNCFSBauges ;
                                           <http://purl.org/spar/datacite/relatedIdentifier> "https://doi.org/10.5281/zenodo.17052197" ;
                                           rdfs:comment "These R data files contains the data needed to replicate the analyses presented in Marchand et al. 2025  - Disturbance by massive sporting events in mountain areas: when and where matters for the protected Alpine ibex Capra ibex, published in People & Nature. 'locs_export' contains gps locations, whereas 'act_export' contains activity data from gps collars. See Methods for details."@en ;
                                           rdfs:label "Data from: Disturbance by massive sporting events in mountain areas: when and where matters for the protected Alpine ibex Capra ibex"@en .


###  https://intforout.github.io/outdoorPressure#MassifDesBauges
:MassifDesBauges rdf:type owl:NamedIndividual ,
                          :ReservesNaturelles ;
                 rdfs:comment "Massif des Bauges"@fr .


###  https://intforout.github.io/outdoorPressure#MergedTrack
:MergedTrack rdf:type owl:NamedIndividual .


###  https://intforout.github.io/outdoorPressure#MergedTracksVincennes2024
:MergedTracksVincennes2024 rdf:type owl:NamedIndividual ,
                                    <http://www.w3.org/ns/dcat#Dataset> ;
                           <http://purl.org/www.umr-lastig.fr/geodata#represents> :HikersFootprintBoisVincennes ;
                           <http://www.w3.org/ns/prov#wasGeneratedBy> :PopulationFootprintFromTracksCollection ;
                           <http://www.w3.org/ns/prov#wasQuotedFrom> :SIGSPATIAL24VanDammeEtAl2024 ;
                           rdfs:comment "Merged tracks generated with the Track collection from Vincennes in 2024 by the MIAA algorithm"@en ;
                           rdfs:label "Merged tracks in Vincennes"@en .


###  https://intforout.github.io/outdoorPressure#MetadataGroundTruthPathVincennesForest
:MetadataGroundTruthPathVincennesForest rdf:type owl:NamedIndividual ,
                                                 <http://www.w3.org/ns/dcat#CatalogRecord> ;
                                        <http://www.w3.org/ns/dcat#accessURL> <https://entrepot.recherche.data.gouv.fr/file.xhtml?persistentId=doi:10.57745/TRYLX1&version=1.0> ;
                                        <http://xmlns.com/foaf/0.1/primaryTopic> :MOUSLSGroundTruthDenseForestPath ;
                                        rdfs:comment "Associated metadata (ISO 19115/19139 XML format, includes station details, measurement uncertainties, and spatial extent)"@en ;
                                        <http://www.w3.org/ns/dcat#conformsTo> <https://www.iso.org/fr/standard/53798.html> ;
                                        <http://www.w3.org/ns/dcat#format> "xml" ;
                                        <http://www.w3.org/ns/dcat#identifier> "Metadata_ground_truth_path_vincennes_forest.xml" ;
                                        <http://www.w3.org/ns/dcat#issued> "2025-08-13"^^xsd:date .


###  https://intforout.github.io/outdoorPressure#MetadataTracksMultiSensorsVincennesForest
:MetadataTracksMultiSensorsVincennesForest rdf:type owl:NamedIndividual ,
                                                    <http://www.w3.org/ns/dcat#CatalogRecord> ;
                                           <http://www.w3.org/ns/dcat#accessURL> <https://entrepot.recherche.data.gouv.fr/file.xhtml?persistentId=doi:10.57745/Q6OT0J&version=1.0> ;
                                           <http://xmlns.com/foaf/0.1/primaryTopic> :MOUSLSTracksMultiSensorsVincennesForest ;
                                           rdfs:comment "Associated metadata (ISO 19115/19139 XML format, contains spatial extent, attributes description, collection method, and quality information)"@en ;
                                           <http://www.w3.org/ns/dcat#conformsTo> <https://www.iso.org/fr/standard/53798.html> ;
                                           <http://www.w3.org/ns/dcat#format> "xml" ;
                                           <http://www.w3.org/ns/dcat#identifier> "Metadata_tracks_multi_sensors_vincennes_forest.xml" ;
                                           <http://www.w3.org/ns/dcat#issued> "2025-08-13"^^xsd:date .


###  https://intforout.github.io/outdoorPressure#Movebank
:Movebank rdf:type owl:NamedIndividual ,
                   <http://purl.org/www.umr-lastig.fr/geodata#DataWarehouse> ;
          <http://purl.org/dc/terms/language> "English" ;
          rdfs:comment "Movebank is coordinated by the Max Planck Institute of Animal Behavior, the North Carolina Museum of Natural Sciences, the Senckenberg Society for Nature Research, and the University of Konstanz. "@en ;
          rdfs:label "Movebank is a free, online database of animal tracking data"@en .


###  https://intforout.github.io/outdoorPressure#OVExportBaugesGeoPackage
:OVExportBaugesGeoPackage rdf:type owl:NamedIndividual ,
                                   <http://www.w3.org/ns/dcat#Distribution> ;
                          <http://www.w3.org/ns/dcat#format> "geopackage" ;
                          <http://www.w3.org/ns/dcat#identifier> "Export_RNCFS_0.gpkg" .


###  https://intforout.github.io/outdoorPressure#OVExportChamonixGeoPackage
:OVExportChamonixGeoPackage rdf:type owl:NamedIndividual ,
                                     <http://www.w3.org/ns/dcat#Distribution> ;
                            <http://www.w3.org/ns/dcat#format> "geopackage" ;
                            <http://www.w3.org/ns/dcat#identifier> "Export_Chamonix_0.gpkg" .


###  https://intforout.github.io/outdoorPressure#OVExportLesHouchesGeoPackage
:OVExportLesHouchesGeoPackage rdf:type owl:NamedIndividual ,
                                       <http://www.w3.org/ns/dcat#Distribution> ;
                              <http://www.w3.org/ns/dcat#format> "geopackage" ;
                              <http://www.w3.org/ns/dcat#identifier> "Export_Les_Houches_0.gpkg" .


###  https://intforout.github.io/outdoorPressure#OVExportServozGeoPackage
:OVExportServozGeoPackage rdf:type owl:NamedIndividual ,
                                   <http://www.w3.org/ns/dcat#Distribution> ;
                          <http://www.w3.org/ns/dcat#format> "geopackage" ;
                          <http://www.w3.org/ns/dcat#identifier> "Export_Servoz_0.gpkg" .


###  https://intforout.github.io/outdoorPressure#OVExportVallorcineGeoPackage
:OVExportVallorcineGeoPackage rdf:type owl:NamedIndividual ,
                                       <http://www.w3.org/ns/dcat#Distribution> ;
                              <http://www.w3.org/ns/dcat#format> "geopackage" ;
                              <http://www.w3.org/ns/dcat#identifier> "Export_Vallorcine_0.gpkg" .


###  https://intforout.github.io/outdoorPressure#OVRecreationalUserMapService
:OVRecreationalUserMapService rdf:type owl:NamedIndividual ,
                                       <http://www.w3.org/ns/dcat#DataService> ;
                              <http://purl.org/www.umr-lastig.fr/geodata#represents> :HumanOutdoorActivitiesBauges2024 ,
                                                                                     :HumanOutdoorActivitiesMontBlanc2024 ;
                              <http://purl.org/dc/terms/publisher> :prnsn ;
                              <http://purl.org/dc/terms/spatial> :RNCFSBauges ,
                                                                 :ZoneEtudeMontBlanc ;
                              rdfs:comment "Ce flux de données permet de visualiser dans l’application Outdoorvision les tracés agrégés des traces GPS issus de services et d’objets connectés des pratiquants de sports et loisirs de nature. L’agrégation des flux s’appuie uniquement sur les traces GPS et ne prend pas en compte les contraintes spatiales comme le réseau routier. Cela permet de visualiser de façon précise la pratique sportive, les trajets réalisés qui peuvent être hors sentier."@fr ,
                                           "This data feed enables visualization in the Outdoorvision application of aggregated GPS tracks obtained from services and connected devices used by outdoor sports and recreational users. The aggregation is based exclusively on GPS traces and does not account for spatial constraints, such as the road network. It provides a precise representation of sports activity and the paths taken, including off-trail routes."@en ;
                              rdfs:label "Recreational User Map Service"@en ,
                                         "Service diffusant des cartes de flux des pratiquants outdoor"@fr .


###  https://intforout.github.io/outdoorPressure#OVTracksMontBlancBauges2024
:OVTracksMontBlancBauges2024 rdf:type owl:NamedIndividual ,
                                      <http://www.w3.org/ns/dcat#Dataset> ;
                             <http://purl.org/www.umr-lastig.fr/geodata#represents> :HumanOutdoorActivitiesBauges2024 ,
                                                                                    :HumanOutdoorActivitiesMontBlanc2024 ;
                             <http://www.w3.org/ns/dcat#distribution> :OVExportBaugesGeoPackage ,
                                                                      :OVExportChamonixGeoPackage ,
                                                                      :OVExportLesHouchesGeoPackage ,
                                                                      :OVExportServozGeoPackage ,
                                                                      :OVExportVallorcineGeoPackage ;
                             <http://purl.org/dc/terms/publisher> :prnsn ;
                             <http://purl.org/dc/terms/spatial> :RNCFSBauges ,
                                                                :ZoneEtudeMontBlanc ;
                             rdfs:comment "A set of tracks issued from Outdoorvision. GPS traces from outdoorvison are cleaned and filtered"@en ;
                             rdfs:label "OutdoorVision export in Bauges and Mont Blanc in 2024"@en ;
                             <http://www.w3.org/ns/dcat#keyword> "GPS traces"@en .


###  https://intforout.github.io/outdoorPressure#PNRBPOIBauges2025
:PNRBPOIBauges2025 rdf:type owl:NamedIndividual ,
                            <http://www.w3.org/ns/dcat#Dataset> ;
                   <http://www.w3.org/ns/dcat#distribution> :parcdesbauges-poi-geojson ;
                   <http://purl.org/dc/terms/issued> "2025-05-01"^^xsd:date ;
                   <http://purl.org/dc/terms/language> "fr-FR" ;
                   <http://purl.org/dc/terms/license> <https://www.etalab.gouv.fr/licence-ouverte-open-licence> ;
                   <http://purl.org/dc/terms/publisher> :parcdesbauges ;
                   rdfs:comment "A set of POIs issued from Parcdesbauges.com."@en ;
                   rdfs:label "Parcdesbauges.com - POI"@fr .


###  https://intforout.github.io/outdoorPressure#PNRBRoutesBauges2025
:PNRBRoutesBauges2025 rdf:type owl:NamedIndividual ,
                               <http://www.w3.org/ns/dcat#Dataset> ;
                      <http://www.w3.org/ns/dcat#distribution> :parcdesbauges-trek-geojson ;
                      <http://purl.org/dc/terms/issued> "2025-05-01"^^xsd:date ;
                      <http://purl.org/dc/terms/language> "fr-FR" ;
                      <http://purl.org/dc/terms/license> <https://www.etalab.gouv.fr/licence-ouverte-open-licence> ;
                      <http://purl.org/dc/terms/publisher> :parcdesbauges ;
                      rdfs:comment "A set of treks issued from Parcdesbauges.com."@en ;
                      rdfs:label "Parcdesbauges.com - trek"@fr .


###  https://intforout.github.io/outdoorPressure#PNRBSensitiveAreaBauges2025
:PNRBSensitiveAreaBauges2025 rdf:type owl:NamedIndividual ,
                                      <http://www.w3.org/ns/dcat#Dataset> ;
                             <http://www.w3.org/ns/dcat#distribution> :parcdesbauges-sensitivearea-geojson ;
                             <http://purl.org/dc/terms/issued> "2025-05-01"^^xsd:date ;
                             <http://purl.org/dc/terms/language> "fr-FR" ;
                             <http://purl.org/dc/terms/license> <https://www.etalab.gouv.fr/licence-ouverte-open-licence> ;
                             <http://purl.org/dc/terms/publisher> :parcdesbauges ;
                             rdfs:comment "A set of sensitive area issued from Parcdesbauges.com."@en ;
                             rdfs:label "Parcdesbauges.com - sensitivearea"@fr .


###  https://intforout.github.io/outdoorPressure#PNRDesBauges
:PNRDesBauges rdf:type owl:NamedIndividual ,
                       <http://purl.org/dc/terms/Location> ;
              rdfs:comment "Le parc naturel régional du Massif des Bauges est une aire protégée"@fr ;
              rdfs:label "Parc naturel régional du Massif des Bauges" .


###  https://intforout.github.io/outdoorPressure#PopulationFootprintFromTracksCollection
:PopulationFootprintFromTracksCollection rdf:type owl:NamedIndividual ,
                                                  <http://purl.org/www.umr-lastig.fr/geodata#Process> ;
                                         <http://www.w3.org/ns/prov#generated> :MergedTracksVincennes2024 ;
                                         <http://www.w3.org/ns/prov#used> :MOUSLS ;
                                         <http://www.w3.org/ns/prov#wasAssociatedWith> <http://purl.org/www.umr-lastig.fr/geodata#Tracklib> ;
                                         <http://www.w3.org/ns/prov#wasAttributedTo> <http://purl.org/www.umr-lastig.fr/geodata#mdvandamme> ;
                                         rdfs:comment "A modular and iterative aggregation algorithm (MIAA)"@en ;
                                         rdfs:label "Population footprint from a tracks collection"@en ;
                                         <http://www.w3.org/ns/prov#endedAtTime> "2024-06"^^xsd:gYearMonth ;
                                         <http://www.w3.org/ns/prov#startedAtTime> "2024-05"^^xsd:gYearMonth .


###  https://intforout.github.io/outdoorPressure#ProfilageOutdoorVision
:ProfilageOutdoorVision rdf:type owl:NamedIndividual ,
                                 <http://purl.org/www.umr-lastig.fr/geodata#UserFeedback> ;
                        <http://purl.org/dc/terms/creator> :anaciri ;
                        rdfs:comment "Profil des données outdoorvision dans un format PDF pour le projet IntForOut"@fr .


###  https://intforout.github.io/outdoorPressure#QualityOfOVRecreationalUserMapService
:QualityOfOVRecreationalUserMapService rdf:type owl:NamedIndividual ,
                                                <http://purl.org/www.umr-lastig.fr/geodata#UserFeedback> ;
                                       <http://purl.org/www.umr-lastig.fr/geodata#target> :OVRecreationalUserMapService ;
                                       <http://purl.org/dc/terms/creator> <http://purl.org/www.umr-lastig.fr/geodata#mdvandamme> ;
                                       rdfs:comment "Artifacts exist in dense urban areas above a certain zoom level. This is because the accuracy of GPS tracks is lower in these areas, making the spatial information displayed less relevant."@en .


###  https://intforout.github.io/outdoorPressure#RNCFSBauges
:RNCFSBauges rdf:type owl:NamedIndividual ,
                      <http://purl.org/dc/terms/Location> ;
             rdfs:comment "La Réserve de chasse et de faune sauvage des Bauges est située dans la partie Est du massif des Bauges et comprend la plupart de ses plus hauts sommets dont le point culminant de l’Arcalod (2217 m). D’une superficie de 5 200 hectares, elle s’étend sur 12 communes des départements de Haute-Savoie (26%) et de Savoie (74%)."@fr ;
             rdfs:label "La Réserve nationale de chasse et de faune sauvage des Bauges" .


###  https://intforout.github.io/outdoorPressure#RefugesInfoPOIBauges2025
:RefugesInfoPOIBauges2025 rdf:type owl:NamedIndividual ,
                                   <http://www.w3.org/ns/dcat#Dataset> ;
                          <http://www.w3.org/ns/dcat#distribution> :refugesinfo-points-geojson ;
                          <http://purl.org/dc/terms/issued> "2025-05-01"^^xsd:date ;
                          <http://purl.org/dc/terms/language> "fr-FR" ;
                          <http://purl.org/dc/terms/license> <http://creativecommons.org/licenses/by-sa/2.0/deed.fr> ;
                          <http://purl.org/dc/terms/publisher> :refugesinfo ;
                          rdfs:comment "A set of Points issued from Refuges.info."@en ;
                          rdfs:label "Refuges.info - points"@en .


###  https://intforout.github.io/outdoorPressure#ReplicabiliteTrackCollectionFusion
:ReplicabiliteTrackCollectionFusion rdf:type owl:NamedIndividual ,
                                             <http://purl.org/www.umr-lastig.fr/geodata#UserFeedback> ;
                                    <http://purl.org/www.umr-lastig.fr/geodata#target> :OVTracksMontBlancBauges2024 ,
                                                                                       :SIGSPATIAL24VanDammeEtAl2024 ;
                                    <http://purl.org/dc/terms/creator> <http://purl.org/www.umr-lastig.fr/geodata#mdvandamme> ;
                                    rdfs:comment "The process proposed in this paper can probably be reproduced to generate HikersFootprint in Les Bauges and MontBlanc, using OutdoorVision data as an input"@en .


###  https://intforout.github.io/outdoorPressure#SIGSPATIAL24VanDammeEtAl2024
:SIGSPATIAL24VanDammeEtAl2024 rdf:type owl:NamedIndividual ,
                                       <http://purl.org/www.umr-lastig.fr/geodata#ScientificPaper> ;
                              <http://purl.org/dc/terms/hasPart> :MOUSLS ;
                              <http://www.w3.org/ns/prov#wasInfluencedBy> :PopulationFootprintFromTracksCollection ;
                              <http://purl.org/dc/terms/creator> <http://purl.org/www.umr-lastig.fr/geodata#amraimond> ,
                                                                 <http://purl.org/www.umr-lastig.fr/geodata#mdvandamme> ,
                                                                 <http://purl.org/www.umr-lastig.fr/geodata#ymeneroux> ;
                              <http://purl.org/dc/terms/isPartOf> "Proceedings of the 32nd ACM International Conference on Advances in Geographic Information Systems" ,
                                                                  "SIGSPATIAL '24" ;
                              <http://purl.org/dc/terms/publisher> "Association for Computing Machinery" ;
                              <http://purl.org/dc/terms/spatial> "Atlanta, GA, USA" ;
                              <http://purl.org/spar/datacite/firstPage> "633" ;
                              <http://purl.org/spar/datacite/lastPage> "636" ;
                              <http://purl.org/spar/datacite/publicationYear> "2024" ;
                              <http://purl.org/spar/datacite/relatedIdentifier> "10.1145/3678717.3691325" ,
                                                                                "https://doi.org/10.1145/3678717.3691325" ;
                              <http://purl.org/spar/datacite/resourceType> <http://purl.org/spar/datacite/ConferenceProceeding> ;
                              <http://purl.org/spar/datacite/subject> "global navigation satellite system" ,
                                                                      "metrological analysis" ,
                                                                      "synthetic and real world trajectories" ,
                                                                      "trajectory aggregation" ;
                              rdfs:label "A metrological analysis of a modular and iterative aggregation algorithm of GNSS trajectories"@en ;
                              <http://www.w3.org/ns/prov#quotedAs> :MOUSLS ,
                                                                   :MergedTracksVincennes2024 .


###  https://intforout.github.io/outdoorPressure#SentierDesBauges
:SentierDesBauges rdf:type owl:NamedIndividual ,
                           :Sentier ;
                  :affords :HikingInLesBauges .


###  https://intforout.github.io/outdoorPressure#SkiLiftCountersMontBlanc2008To2024
:SkiLiftCountersMontBlanc2008To2024 rdf:type owl:NamedIndividual ,
                                             <http://www.w3.org/ns/dcat#Dataset> ;
                                    <http://purl.org/www.umr-lastig.fr/geodata#represents> :SkiLiftUsageMontBlanc2008To2024 ;
                                    rdfs:comment "Counting data for each ski lift, including their locations (start and end points), over a 10-year period (one file per year)."@en ;
                                    rdfs:label "Ski Lift Ridership Counts in the CMB Area."@en .


###  https://intforout.github.io/outdoorPressure#SkiLiftUsageMontBlanc2008To2024
:SkiLiftUsageMontBlanc2008To2024 rdf:type owl:NamedIndividual ,
                                          :HumanActivity .


###  https://intforout.github.io/outdoorPressure#Strava
:Strava rdf:type owl:NamedIndividual ,
                 <http://www.w3.org/ns/prov#Organization> ;
        rdfs:comment "american internet service for tracking physical exercise which incorporates social networking features. It tracks outdoor activities using GPS data, and other exercise types, including indoor activities. Strava records data for a user's activities, which can then be shared with the user's followers or shared publicly. If an activity is shared publicly, Strava automatically groups activities that occur at the same time and place (such as taking part in a marathon, sportive or group ride). An activity's recorded information may include a route summary, elevation (net and unidirectional), speed (average and maximum), timing (total and moving time), power and heart rate. Activities can be recorded using the mobile app or from devices manufactured by third parties like Garmin, Google Fit, Suunto, and Wahoo. Activities can also be entered manually via the Strava website and mobile app. (quoted from wikipedia)"@en ;
        rdfs:seeAlso "https://www.wikidata.org/wiki/Q13884156" ;
        <http://xmlns.com/foaf/0.1/homePage> "https://www.strava.com/about" .


###  https://intforout.github.io/outdoorPressure#StravaMetro
:StravaMetro rdf:type owl:NamedIndividual ,
                      <http://purl.org/www.umr-lastig.fr/geodata#DataWarehouse> ;
             <http://purl.org/dc/terms/language> "English" ;
             <http://purl.org/dc/terms/publisher> :Strava ;
             rdfs:comment "Aggregated and de-identified Strava data"@en ;
             rdfs:label "Strava Metro data set"@en ;
             rdfs:seeAlso "https://www.wikidata.org/wiki/Q114074281" .


###  https://intforout.github.io/outdoorPressure#StravaMetroTracksMontBlanc2024
:StravaMetroTracksMontBlanc2024 rdf:type owl:NamedIndividual ,
                                         <http://www.w3.org/ns/dcat#Dataset> ;
                                <http://purl.org/www.umr-lastig.fr/geodata#represents> :HumanOutdoorActivitiesBauges2014 ;
                                <http://purl.org/dc/elements/1.1/publisher> :Strava .


###  https://intforout.github.io/outdoorPressure#StravaRecreationalUserMapService
:StravaRecreationalUserMapService rdf:type owl:NamedIndividual ,
                                           <http://www.w3.org/ns/dcat#DataService> ;
                                  <http://purl.org/www.umr-lastig.fr/geodata#represents> :HumanOutdoorActivitiesBauges2024 ,
                                                                                         :HumanOutdoorActivitiesMontBlanc2024 ;
                                  <http://purl.org/dc/terms/publisher> :Strava ;
                                  rdfs:comment "Displays the aggregated public activities recorded in Strava over the past year"@en ,
                                               "Montre les activités publiques agrégées au cours de l'année passée dans Strava"@fr ;
                                  rdfs:label "Carte mondiale des activités Strava"@fr ,
                                             "Strava Global Heatmap"@en ;
                                  rdfs:seeAlso "https://www.wikidata.org/wiki/Q114074364" .


###  https://intforout.github.io/outdoorPressure#StravaTracksBauges2014
:StravaTracksBauges2014 rdf:type owl:NamedIndividual ,
                                 <http://www.w3.org/ns/dcat#Dataset> ;
                        <http://purl.org/www.umr-lastig.fr/geodata#represents> :HumanOutdoorActivitiesBauges2014 ;
                        <http://purl.org/dc/elements/1.1/publisher> :Strava .


###  https://intforout.github.io/outdoorPressure#TopometricSurveyGroundTruthPathVincennes2024
:TopometricSurveyGroundTruthPathVincennes2024 rdf:type owl:NamedIndividual ,
                                                       :Observation ;
                                              <http://www.w3.org/ns/prov#generated> :MOUSLSGroundTruthDenseForestPath ;
                                              <http://www.w3.org/ns/prov#used> <ttp://purl.org/www.umr-lastig.fr/geodata#LeicaTS16> ;
                                              <http://purl.org/dc/terms/creator> :blabbe ,
                                                                                 :lpeseux ,
                                                                                 :pcalloch ;
                                              <http://www.w3.org/ns/prov#endedAtTime> "2024-01-18"^^xsd:gYearMonth ;
                                              <http://www.w3.org/ns/prov#startedAtTime> "2024-01-18"^^xsd:gYearMonth .


###  https://intforout.github.io/outdoorPressure#TracksMultiSensorsVincennesForest-gpkg
:TracksMultiSensorsVincennesForest-gpkg rdf:type owl:NamedIndividual ,
                                                 <http://www.w3.org/ns/dcat#Distribution> ;
                                        <http://www.w3.org/ns/dcat#accessURL> <https://entrepot.recherche.data.gouv.fr/file.xhtml?persistentId=doi:10.57745/NSMUWN&version=1.0> ;
                                        <http://www.w3.org/ns/dcat#format> "gpkg" ;
                                        <http://www.w3.org/ns/dcat#identifier> "tracks_multi_sensors_vincennes_forest.gpkg" .


###  https://intforout.github.io/outdoorPressure#VisorandoRoutesBauges2025
:VisorandoRoutesBauges2025 rdf:type owl:NamedIndividual ,
                                    <http://www.w3.org/ns/dcat#Dataset> ;
                           <http://purl.org/dc/terms/issued> "2025-05-01"^^xsd:date ;
                           <http://purl.org/dc/terms/language> "fr-FR" ;
                           <http://purl.org/dc/terms/license> <https://opendatacommons.org/licenses/odbl/> ;
                           <http://purl.org/dc/terms/publisher> :visorando ;
                           rdfs:comment "A set of routes issued from visorando.com."@en ;
                           rdfs:label "Visorando Hiking Routes in the Bauges Massif (2025)"@en .


###  https://intforout.github.io/outdoorPressure#WildlifeMonitoringFromCameraTrapImage
:WildlifeMonitoringFromCameraTrapImage rdf:type owl:NamedIndividual ,
                                                <http://purl.org/www.umr-lastig.fr/geodata#Process> ;
                                       <http://www.w3.org/ns/prov#wasAssociatedWith> :DeepFaune ;
                                       rdfs:comment "Les données pièges-photos seront actualisées par Marjorie en janvier. A noter que les sorties DeepFaune étaient indiquées dans les données ouvertes et qu’elles ont été décalées dans la partie sous convention (à n’utiliser que dans le cadre du consortium, comme les autres données CREA-partenaires)"@en .


###  https://intforout.github.io/outdoorPressure#ZoneEtudeMontBlanc
:ZoneEtudeMontBlanc rdf:type owl:NamedIndividual ,
                             <http://purl.org/dc/terms/Location> ;
                    rdfs:label "Massif du Mont Blanc, côté France" .


###  https://intforout.github.io/outdoorPressure#aloison
:aloison rdf:type owl:NamedIndividual ,
                  <http://www.w3.org/ns/prov#Person> ;
         <http://xmlns.com/foaf/0.1/name> "Anne Loison" .


###  https://intforout.github.io/outdoorPressure#altituderando
:altituderando rdf:type owl:NamedIndividual ,
                        <http://www.w3.org/ns/prov#Organization> ;
               <http://xmlns.com/foaf/0.1/homePage> <https://www.altituderando.com> ;
               <http://xmlns.com/foaf/0.1/name> "Altituderando" .


###  https://intforout.github.io/outdoorPressure#anaciri
:anaciri rdf:type owl:NamedIndividual ,
                  <http://www.w3.org/ns/prov#Person> ;
         <http://xmlns.com/foaf/0.1/name> "Abdassalam Naciri" .


###  https://intforout.github.io/outdoorPressure#api-camptocamp
:api-camptocamp rdf:type owl:NamedIndividual ,
                         <http://www.w3.org/ns/dcat#DataService> ;
                <http://www.w3.org/ns/dcat#accessURL> <https://api.camptocamp.org/> ;
                <http://www.w3.org/ns/dcat#servesDataset> :CamptocampPoisBauges2025 ,
                                                          :CamptocampRoutesBauges2025 ;
                <http://purl.org/dc/terms/license> <https://opendatacommons.org/licenses/odbl/> ;
                <http://purl.org/dc/terms/publisher> :camptocamp ;
                rdfs:comment "API du site collaboratif et interactif camptocamp.org. On peut y trouver des informations sur la montagne : conditions sur le terrain (manteau neigeux par exemple), descriptions de sommets, itinéraires de ski de randonnée ou grandes voies d’escalade par exemple, photographies, articles techniques ou récits de montagne. Certaines de ces informations sont modifiables par tout contributeur enregistré . Vous y trouverez aussi un forum qui vous permet d’échanger."@fr ;
                rdfs:label "API de Camptocamp.org (routes, waypoints, outings)"@en ;
                <http://xmlns.com/foaf/0.1/homePage> <https://www.camptocamp.org/> .


###  https://intforout.github.io/outdoorPressure#api-parcdesbauges
:api-parcdesbauges rdf:type owl:NamedIndividual ,
                            <http://www.w3.org/ns/dcat#DataService> ;
                   <http://www.w3.org/ns/dcat#accessURL> <https://geotrek.parcdesbauges.com/api/v2/> ;
                   <http://www.w3.org/ns/dcat#servesDataset> :PNRBPOIBauges2025 ,
                                                             :PNRBRoutesBauges2025 ,
                                                             :PNRBSensitiveAreaBauges2025 ;
                   <http://purl.org/dc/terms/license> <https://www.etalab.gouv.fr/licence-ouverte-open-licence> ;
                   <http://purl.org/dc/terms/publisher> :parcdesbauges ;
                   rdfs:comment "L'API du PNR Massif des Bauges met en valeur la randonnée pédestre, sentier et activités touristiques en offrant une pléthore de requêtes pour accéder données."@fr ;
                   rdfs:label "API du PNR Massif des Bauges"@en .


###  https://intforout.github.io/outdoorPressure#api-refugesinfo
:api-refugesinfo rdf:type owl:NamedIndividual ,
                          <http://www.w3.org/ns/dcat#DataService> ;
                 <http://www.w3.org/ns/dcat#accessURL> <https://www.refuges.info/api/> ;
                 <http://www.w3.org/ns/dcat#servesDataset> :RefugesInfoPOIBauges2025 ;
                 <http://purl.org/dc/terms/license> <http://creativecommons.org/licenses/by-sa/2.0/deed.fr> ;
                 <http://purl.org/dc/terms/publisher> :refugesinfo ;
                 rdfs:comment "L'API de Refuges.info est un service web personnel et non commercial permettant de se renseigner sur les hébergements de montagnes destinés aux randonneurs. Elle permet de recevoir dans de nombreux formats une liste de points, des informations détaillées sur un point ou encore les résultats de requêtes spéciales telles que la recherche de points."@fr ;
                 rdfs:label "API de Refuges.info (points)"@en .


###  https://intforout.github.io/outdoorPressure#blabbe
:blabbe rdf:type owl:NamedIndividual ,
                 <http://www.w3.org/ns/prov#Person> ;
        <http://xmlns.com/foaf/0.1/name> "Brice Labbé" .


###  https://intforout.github.io/outdoorPressure#c2c-route-geojson
:c2c-route-geojson rdf:type owl:NamedIndividual ,
                            <http://www.w3.org/ns/dcat#Distribution> ;
                   <http://www.w3.org/ns/dcat#accessService> :api-camptocamp ;
                   <http://www.w3.org/ns/dcat#format> "GeoJSON" .


###  https://intforout.github.io/outdoorPressure#c2c-waypoint-geojson
:c2c-waypoint-geojson rdf:type owl:NamedIndividual ,
                               <http://www.w3.org/ns/dcat#Distribution> ;
                      <http://www.w3.org/ns/dcat#accessService> :api-camptocamp ;
                      <http://www.w3.org/ns/dcat#format> "GeoJSON" .


###  https://intforout.github.io/outdoorPressure#camptocamp
:camptocamp rdf:type owl:NamedIndividual ,
                     <http://www.w3.org/ns/prov#Organization> ;
            <http://xmlns.com/foaf/0.1/homePage> <https://www.camptocamp.org/> ;
            <http://xmlns.com/foaf/0.1/name> "Camptocamp Association" .


###  https://intforout.github.io/outdoorPressure#cirkwi
:cirkwi rdf:type owl:NamedIndividual ,
                 <http://www.w3.org/ns/prov#Organization> ;
        <http://xmlns.com/foaf/0.1/homePage> <https://www.cirkwi.com/> ;
        <http://xmlns.com/foaf/0.1/name> "Cirkwi" .


###  https://intforout.github.io/outdoorPressure#lpeseux
:lpeseux rdf:type owl:NamedIndividual ,
                  <http://www.w3.org/ns/prov#Person> ;
         <http://xmlns.com/foaf/0.1/name> "Lorine Peseux" .


###  https://intforout.github.io/outdoorPressure#marchandetal-rdata
:marchandetal-rdata rdf:type owl:NamedIndividual ,
                             <http://www.w3.org/ns/dcat#Distribution> ;
                    <http://www.w3.org/ns/dcat#format> "RData" .


###  https://intforout.github.io/outdoorPressure#mgarel
:mgarel rdf:type owl:NamedIndividual ,
                 <http://www.w3.org/ns/prov#Person> ;
        <http://xmlns.com/foaf/0.1/name> "Mathieu Garel" .


###  https://intforout.github.io/outdoorPressure#openstreetmap
:openstreetmap rdf:type owl:NamedIndividual ,
                        <http://www.w3.org/ns/prov#Organization> ;
               <http://xmlns.com/foaf/0.1/homePage> <https://www.openstreetmap.org> ;
               <http://xmlns.com/foaf/0.1/name> "OpenStreetMap (OSM)" .


###  https://intforout.github.io/outdoorPressure#outdoorvision
:outdoorvision rdf:type owl:NamedIndividual ,
                        <http://www.w3.org/ns/dcat#Catalog> ;
               <http://www.w3.org/ns/dcat#dataset> :OVTracksMontBlancBauges2024 ;
               <http://www.w3.org/ns/dcat#service> :OVRecreationalUserMapService ;
               <http://purl.org/dc/terms/publisher> :prnsn ;
               rdfs:comment "Outdoorvision https://outdoorvision.fr/; is a service to gather GPS tracks voluntarily shared by human during their outdoor activity through their accounts on their mobile device Garmin Connect™ / Polar Flow / Suunto APP (Appli Suunto) / Decathlon. The data are anonymized and published for a list of authorised users. It is offered by the French National Resource Centre for Ecological Transition and Outdoor Sports, a support mission of the Ministry of Sport. It results from a partnership between local authorities, sports federations and brands united around a non-profit programme."@en ;
               rdfs:label "OutdoorVision Catalog"@en ;
               <http://xmlns.com/foaf/0.1/homePage> "https://outdoorvision.fr/" .


###  https://intforout.github.io/outdoorPressure#parcdesbauges
:parcdesbauges rdf:type owl:NamedIndividual ,
                        <http://www.w3.org/ns/prov#Organization> ;
               <http://xmlns.com/foaf/0.1/homePage> <https://parcdesbauges.com> ;
               <http://xmlns.com/foaf/0.1/name> "Parc Naturel Régional du Massif des Bauges" .


###  https://intforout.github.io/outdoorPressure#parcdesbauges-poi-geojson
:parcdesbauges-poi-geojson rdf:type owl:NamedIndividual ,
                                    <http://www.w3.org/ns/dcat#Distribution> ;
                           <http://www.w3.org/ns/dcat#accessService> :api-parcdesbauges ;
                           <http://www.w3.org/ns/dcat#format> "GeoJSON" .


###  https://intforout.github.io/outdoorPressure#parcdesbauges-sensitivearea-geojson
:parcdesbauges-sensitivearea-geojson rdf:type owl:NamedIndividual ,
                                              <http://www.w3.org/ns/dcat#Distribution> ;
                                     <http://www.w3.org/ns/dcat#accessService> :api-parcdesbauges ;
                                     <http://www.w3.org/ns/dcat#format> "GeoJSON" .


###  https://intforout.github.io/outdoorPressure#parcdesbauges-trek-geojson
:parcdesbauges-trek-geojson rdf:type owl:NamedIndividual ,
                                     <http://www.w3.org/ns/dcat#Distribution> ;
                            <http://www.w3.org/ns/dcat#accessService> :api-parcdesbauges ;
                            <http://www.w3.org/ns/dcat#format> "GeoJSON" .


###  https://intforout.github.io/outdoorPressure#pcalloch
:pcalloch rdf:type owl:NamedIndividual ,
                   <http://www.w3.org/ns/prov#Person> ;
          <http://xmlns.com/foaf/0.1/name> "Paul Calloch" .


###  https://intforout.github.io/outdoorPressure#pmarchand
:pmarchand rdf:type owl:NamedIndividual ,
                    <http://www.w3.org/ns/prov#Person> ;
           <http://xmlns.com/foaf/0.1/name> "Pascal Marchand" .


###  https://intforout.github.io/outdoorPressure#prnsn
:prnsn rdf:type owl:NamedIndividual ,
                <http://www.w3.org/ns/prov#Organization> ;
       rdfs:label "Pôle ressources national sports de nature (PRNSN)" .


###  https://intforout.github.io/outdoorPressure#refugesinfo
:refugesinfo rdf:type owl:NamedIndividual ,
                      <http://www.w3.org/ns/prov#Organization> ;
             <http://xmlns.com/foaf/0.1/homePage> <https://www.refuges.info/> ;
             <http://xmlns.com/foaf/0.1/name> "Refuges.info" .


###  https://intforout.github.io/outdoorPressure#refugesinfo-points-geojson
:refugesinfo-points-geojson rdf:type owl:NamedIndividual ,
                                     <http://www.w3.org/ns/dcat#Distribution> ;
                            <http://www.w3.org/ns/dcat#accessService> :api-refugesinfo ;
                            <http://www.w3.org/ns/dcat#format> "GeoJSON" .


###  https://intforout.github.io/outdoorPressure#visorando
:visorando rdf:type owl:NamedIndividual ,
                    <http://www.w3.org/ns/prov#Organization> ;
           <http://xmlns.com/foaf/0.1/homePage> <https://www.visorando.com/> ;
           <http://xmlns.com/foaf/0.1/name> "Visorando" .


###  https://www.refuges.info/api/
<https://www.refuges.info/api/> rdf:type owl:NamedIndividual .


#################################################################
#    Annotations
#################################################################

:MergedTrack rdfs:comment "A merged trace represents the best geometric representation of a set of traces following exactly the same route, defined from an origin point to a destination (Van Damme et al., 2024)."@en ,
                          "La trace fusionnée est la meilleure représentation géométrique d’un ensemble de traces suivant exactement le même trajet, défini d un point d origine à une destination (Van Damme et al., 2024)."@fr .


###  Generated by the OWL API (version 5.1.18) https://github.com/owlcs/owlapi/
